@prefix rel-av:  <http://onto.fel.cvut.cz/ontologies/reliability/aviation-profile/> .
@prefix rdf:  <http://www.w3.org/1999/02/22-rdf-syntax-ns#> .
@prefix owl:  <http://www.w3.org/2002/07/owl#> .
@prefix rel:  <http://onto.fel.cvut.cz/ontologies/reliability/> .
@prefix rdfs:  <http://www.w3.org/2000/01/rdf-schema#> .
@prefix ata:  <http://onto.fel.cvut.cz/voc/ata-100/> .

rel-av:  rdf:type       owl:Ontology ;
        owl:versionIRI  rel-av:v0.1 .
@prefix rel-av:  <http://onto.fel.cvut.cz/ontologies/reliability/aviation-profile/> .
@prefix owl:  <http://www.w3.org/2002/07/owl#> .
@prefix rdf:  <http://www.w3.org/1999/02/22-rdf-syntax-ns#> .
@prefix xsd:  <http://www.w3.org/2001/XMLSchema#> .
@prefix rel:  <http://onto.fel.cvut.cz/ontologies/reliability/> .
@prefix rdfs:  <http://www.w3.org/2000/01/rdf-schema#> .
@prefix ata:  <http://onto.fel.cvut.cz/voc/ata-100/> .

ata:ata-53-80  rdf:type  owl:Class ;
        rdfs:label       "[AS REQUIRED]" ;
        rdfs:subClassOf  rel:Component ;
        ata:has-id       "5380" .

ata:ata-61-40  rdf:type  owl:Class ;
        rdfs:comment     "That portion of the system used to indicate operation or activation of propeller/propulsor systems. Includes items such as light, switches, wiring etc." ;
        rdfs:label       "INDICATING" ;
        rdfs:subClassOf  rel:Component ;
        ata:has-id       "6140" .

ata:ata-74-20  rdf:type  owl:Class ;
        rdfs:comment     "That portion of the system that conducts high or low voltage electricity from the electrical power supply to the spark plugs or igniters. Includes wiring between magneto and distributors in those systems where they are separate units. Includes items such as ignition harness, high tension leads, coils used in \"low tension\" systems, spark plugs igniters, etc." ;
        rdfs:label       "DISTRIBUTION" ;
        rdfs:subClassOf  rel:Component ;
        ata:has-id       "7420" .

ata:ata-46-50  rdf:type  owl:Class ;
        rdfs:comment     "That portion of the onboard information system that supports other functions, as defined by the user, that cannot be related to the flight deck, passenger cabin, or maintenance." ;
        rdfs:label       "MISCELLANEOUS INFORMATION SYSTEMS" ;
        rdfs:subClassOf  rel:Component ;
        ata:has-id       "4650" .

ata:ata-49  rdf:type     owl:Class ;
        rdfs:comment     "Those airborne power plants (engines) which are installed on the aircraft for the purpose of generating and supplying a single type or combination of auxiliary electric, hydraulic, pneumatic or other power. Includes power and drive section, fuel, ignition and control systems; also wiring, indicators, plumbing, valves, and ducts up to the power unit. Does not include generators, alternators, hydraulic pumps, etc. or their connecting systems which supply and deliver power to their respective aircraft systems." ;
        rdfs:label       "AIRBORNE AUXILIARY POWER" ;
        rdfs:subClassOf  rel:Component .

_:b0    rdf:type            owl:Restriction ;
        owl:onProperty      rel:hasComponent ;
        owl:someValuesFrom  ata:ata-49-20 .

ata:ata-49  rdfs:subClassOf  _:b0 .

_:b1    rdf:type            owl:Restriction ;
        owl:onProperty      rel:hasComponent ;
        owl:someValuesFrom  ata:ata-49-30 .

ata:ata-49  rdfs:subClassOf  _:b1 .

_:b2    rdf:type            owl:Restriction ;
        owl:onProperty      rel:hasComponent ;
        owl:someValuesFrom  ata:ata-49-50 .

ata:ata-49  rdfs:subClassOf  _:b2 .

_:b3    rdf:type            owl:Restriction ;
        owl:onProperty      rel:hasComponent ;
        owl:someValuesFrom  ata:ata-49-10 .

ata:ata-49  rdfs:subClassOf  _:b3 .

_:b4    rdf:type            owl:Restriction ;
        owl:onProperty      rel:hasComponent ;
        owl:someValuesFrom  ata:ata-49-60 .

ata:ata-49  rdfs:subClassOf  _:b4 .

_:b5    rdf:type            owl:Restriction ;
        owl:onProperty      rel:hasComponent ;
        owl:someValuesFrom  ata:ata-49-40 .

ata:ata-49  rdfs:subClassOf  _:b5 .

_:b6    rdf:type            owl:Restriction ;
        owl:onProperty      rel:hasComponent ;
        owl:someValuesFrom  ata:ata-49-70 .

ata:ata-49  rdfs:subClassOf  _:b6 .

_:b7    rdf:type            owl:Restriction ;
        owl:onProperty      rel:hasComponent ;
        owl:someValuesFrom  ata:ata-49-90 .

ata:ata-49  rdfs:subClassOf  _:b7 .

_:b8    rdf:type            owl:Restriction ;
        owl:onProperty      rel:hasComponent ;
        owl:someValuesFrom  ata:ata-49-80 .

ata:ata-49  rdfs:subClassOf  _:b8 ;
        rel:hasComponent  ata:ata-49-60 ;
        rel:hasComponent  ata:ata-49-20 ;
        rel:hasComponent  ata:ata-49-80 ;
        rel:hasComponent  ata:ata-49-90 ;
        rel:hasComponent  ata:ata-49-70 ;
        rel:hasComponent  ata:ata-49-30 ;
        rel:hasComponent  ata:ata-49-40 ;
        rel:hasComponent  ata:ata-49-50 ;
        rel:hasComponent  ata:ata-49-10 ;
        ata:has-id        "49" .

ata:ata-51-80  rdf:type  owl:Class ;
        rdfs:comment     "Topics concerning the electrical bonding of aircraft structure as well as electrical bonding of subsystems to aircraft structure." ;
        rdfs:label       "ELECTRICAL BONDING" ;
        rdfs:subClassOf  rel:Component ;
        ata:has-id       "5180" .

<http://onto.fel.cvut.cz/voc/ata-100/ata-72(T)-20>
        rdf:type         owl:Class ;
        rdfs:comment     "The section of the engine through which air enters the compressor section. Includes items such as guide vanes, shrouds, cases, etc." ;
        rdfs:label       "AIR INLET SECTION" ;
        rdfs:subClassOf  rel:Component ;
        ata:has-id       "72(T)20" .

ata:ata-77-40  rdf:type  owl:Class ;
        rdfs:comment     "That portion of the system which as an integrated concept receives several/all engine operating parameters and transmits this to a central processor for crew presentation. Includes items such as display units, transmitters, receivers, computers, etc." ;
        rdfs:label       "INTEGRATED ENGINE INSTRUMENT SYSTEMS" ;
        rdfs:subClassOf  rel:Component ;
        ata:has-id       "7740" .

ata:ata-31-70  rdf:type  owl:Class ;
        rdfs:comment     "Those systems and components used for collating and computing data from unrelated systems and transmitting same automatically. Includes ASDAR systems and components." ;
        rdfs:label       "AUTOMATIC DATA REPORTING SYSTEMS" ;
        rdfs:subClassOf  rel:Component ;
        ata:has-id       "3170" .

ata:ata-63  rdf:type     owl:Class ;
        rdfs:comment     "Includes all components transmitting power to the rotor(s): engine coupling components, drive shaft(s), clutch and free wheel units, gear box(es), its (their) components, systems and securing elements." ;
        rdfs:label       "MAIN ROTOR DRIVE(S)" ;
        rdfs:subClassOf  rel:Component .

_:b9    rdf:type            owl:Restriction ;
        owl:onProperty      rel:hasComponent ;
        owl:someValuesFrom  ata:ata-63-10 .

ata:ata-63  rdfs:subClassOf  _:b9 .

_:b10   rdf:type            owl:Restriction ;
        owl:onProperty      rel:hasComponent ;
        owl:someValuesFrom  ata:ata-63-20 .

ata:ata-63  rdfs:subClassOf  _:b10 .

_:b11   rdf:type            owl:Restriction ;
        owl:onProperty      rel:hasComponent ;
        owl:someValuesFrom  ata:ata-63-40 .

ata:ata-63  rdfs:subClassOf  _:b11 .

_:b12   rdf:type            owl:Restriction ;
        owl:onProperty      rel:hasComponent ;
        owl:someValuesFrom  ata:ata-63-30 .

ata:ata-63  rdfs:subClassOf  _:b12 ;
        rel:hasComponent  ata:ata-63-20 ;
        rel:hasComponent  ata:ata-63-40 ;
        rel:hasComponent  ata:ata-63-10 ;
        rel:hasComponent  ata:ata-63-30 ;
        ata:has-id        "63" .

ata:ata-49-70  rdf:type  owl:Class ;
        rdfs:comment     "For definitions see Chapter 77." ;
        rdfs:label       "INDICATING" ;
        rdfs:subClassOf  rel:Component ;
        ata:has-id       "4970" .

ata:ata-28-20  rdf:type  owl:Class ;
        rdfs:comment     "That portion of the system which is used to distribute fuel from the filler connector to the storage system and from the storage system to and including the power plant fuel quick disconnect. Includes items such as plumbing, pumps, valves, controls, etc." ;
        rdfs:label       "DISTRIBUTION - DRAIN VALVES" ;
        rdfs:subClassOf  rel:Component ;
        ata:has-id       "2820" .

ata:ata-31  rdf:type     owl:Class ;
        rdfs:comment     "Pictorial coverage of all instruments, instrument panels and controls. Procedural coverage of those systems which give visual or aural warning of conditions in unrelated systems. Units which record, store or compute data from unrelated systems. Includes systems/units which integrate indicating instruments into a central display system and instruments not related to any specific system." ;
        rdfs:label       "INDICATING / RECORDING SYSTEMS" ;
        rdfs:subClassOf  rel:Component .

_:b13   rdf:type            owl:Restriction ;
        owl:onProperty      rel:hasComponent ;
        owl:someValuesFrom  ata:ata-31-50 .

ata:ata-31  rdfs:subClassOf  _:b13 .

_:b14   rdf:type            owl:Restriction ;
        owl:onProperty      rel:hasComponent ;
        owl:someValuesFrom  ata:ata-31-60 .

ata:ata-31  rdfs:subClassOf  _:b14 .

_:b15   rdf:type            owl:Restriction ;
        owl:onProperty      rel:hasComponent ;
        owl:someValuesFrom  ata:ata-31-20 .

ata:ata-31  rdfs:subClassOf  _:b15 .

_:b16   rdf:type            owl:Restriction ;
        owl:onProperty      rel:hasComponent ;
        owl:someValuesFrom  ata:ata-31-10 .

ata:ata-31  rdfs:subClassOf  _:b16 .

_:b17   rdf:type            owl:Restriction ;
        owl:onProperty      rel:hasComponent ;
        owl:someValuesFrom  ata:ata-31-30 .

ata:ata-31  rdfs:subClassOf  _:b17 .

_:b18   rdf:type            owl:Restriction ;
        owl:onProperty      rel:hasComponent ;
        owl:someValuesFrom  ata:ata-31-70 .

ata:ata-31  rdfs:subClassOf  _:b18 .

_:b19   rdf:type            owl:Restriction ;
        owl:onProperty      rel:hasComponent ;
        owl:someValuesFrom  ata:ata-31-40 .

ata:ata-31  rdfs:subClassOf  _:b19 ;
        rel:hasComponent  ata:ata-31-10 ;
        rel:hasComponent  ata:ata-31-50 ;
        rel:hasComponent  ata:ata-31-20 ;
        rel:hasComponent  ata:ata-31-30 ;
        rel:hasComponent  ata:ata-31-60 ;
        rel:hasComponent  ata:ata-31-40 ;
        rel:hasComponent  ata:ata-31-70 ;
        ata:has-id        "31" .

ata:ata-75-40  rdf:type  owl:Class ;
        rdfs:comment     "That portion of the system which is used to indicate temperature, pressure, control positions, etc. of the air systems. Includes items such as transmitters, indicators, wiring, etc." ;
        rdfs:label       "INDICATING" ;
        rdfs:subClassOf  rel:Component ;
        ata:has-id       "7540" .

ata:ata-41-10  rdf:type  owl:Class ;
        rdfs:comment     "That portion of the system which stores water solely for the purpose of providing airship ballast. Includes removable tanks (bladder cells), interconnecting balance pipes, filler valves, etc." ;
        rdfs:label       "STORAGE" ;
        rdfs:subClassOf  rel:Component ;
        ata:has-id       "4110" .

ata:ata-26-20  rdf:type  owl:Class ;
        rdfs:comment     "That portion of those fixed or portable systems which is used to extinguish fire." ;
        rdfs:label       "EXTINGUISHING" ;
        rdfs:subClassOf  rel:Component ;
        ata:has-id       "2620" .

ata:ata-45-70  rdf:type  owl:Class ;
        rdfs:comment     "Central Maintenance System interfaces with Power Plant, and identification of maintenance functions related to Power Plant. NOTE: Subsystem/Section Code is selected to match applicable system interface. For example, 45 -21-XX would identify all air conditioning monitoring and testing provided by the Central Maintenance System, and would provide directions for using the Central Maintenance System to execute those maintenance functions. Detailed testing not capable of coverage in Chapter 45 would be appropriately cross referenced and would be provided in Chapter 21. Similarly, 45 -32-XX would identify landing gear monitoring and testing provided by the Central Maintenance System. 45 -45 -XX would identify the Central Maintenance System itself." ;
        rdfs:label       "CMS / POWER PLANT" ;
        rdfs:subClassOf  rel:Component ;
        ata:has-id       "4570" .

ata:ata-57-10  rdf:type  owl:Class ;
        rdfs:comment     "Wing Skins, primary structure, fillets, and fairings of the center wing, and attach / attached fittings." ;
        rdfs:label       "CENTER" ;
        rdfs:subClassOf  rel:Component ;
        ata:has-id       "5710" .

ata:ata-24-20  rdf:type  owl:Class ;
        rdfs:comment     "That portion of the systems used to generate, regulate, control, and indicate AC electrical power. Includes items such as inverters, AC generators/alternators, control and regulating components, indicating systems, etc., all wiring to but not including main busses." ;
        rdfs:label       "AC GENERATION" ;
        rdfs:subClassOf  rel:Component ;
        ata:has-id       "2420" .

ata:ata-76  rdf:type     owl:Class ;
        rdfs:comment     "Those controls which govern operation of the engine. Includes units and components which are interconnected for emergency shutdown. For turbo-prop engines, includes linkages and controls to the coordinator or equivalent to the propeller governor, fuel control unit or other units being controlled. For reciprocating engine, include controls for blowers. Does not include units or components which are specifically included in other chapters." ;
        rdfs:label       "ENGINE CONTROLS" ;
        rdfs:subClassOf  rel:Component .

_:b20   rdf:type            owl:Restriction ;
        owl:onProperty      rel:hasComponent ;
        owl:someValuesFrom  ata:ata-76-20 .

ata:ata-76  rdfs:subClassOf  _:b20 .

_:b21   rdf:type            owl:Restriction ;
        owl:onProperty      rel:hasComponent ;
        owl:someValuesFrom  ata:ata-76-10 .

ata:ata-76  rdfs:subClassOf  _:b21 ;
        rel:hasComponent  ata:ata-76-20 ;
        rel:hasComponent  ata:ata-76-10 ;
        ata:has-id        "76" .

ata:ata-55-10  rdf:type  owl:Class ;
        rdfs:comment     "The horizontal airfoil of the tail or nose section to which the elevator is attached. Includes items such as spars, ribs, stringers, skins, access covers, tips, attach / attached fittings, etc." ;
        rdfs:label       "HORIZONTAL STABILIZER / STABILATOR OR CANARD" ;
        rdfs:subClassOf  rel:Component ;
        ata:has-id       "5510" .

ata:ata-22-20  rdf:type  owl:Class ;
        rdfs:comment     "That portion of the system that automatically maintains safe flight conditions by correcting for effects of speed and out -of-trim conditions by such means as automatic trim, mach trim or speed stability and mach feel. This includes sensing, computing, actuating, indicating, internal monitoring, and warning devices, etc." ;
        rdfs:label       "SPEED - ATTITUDE CORRECTION" ;
        rdfs:subClassOf  rel:Component ;
        ata:has-id       "2220" .

ata:ata-27-40  rdf:type  owl:Class ;
        rdfs:comment     "That portion of the system which controls the position and movement of the horizontal stabilizer/canard. Includes items such as control handle, cables, jackscrews, motors, warning systems, linkages, control surfaces, position indicators, etc." ;
        rdfs:label       "HORIZONTAL STABILIZER / STABILATOR" ;
        rdfs:subClassOf  rel:Component ;
        ata:has-id       "2740" .

ata:ata-53-10  rdf:type  owl:Class ;
        rdfs:comment     "Fuselage Sections Skins, main structure, secondary structure, and fairings of the complete fuselage with any structural differences grouped together and highlighted by fuselage section location. The section locations shall be defined by manufacturing joints or other suitable demarcations in sequence from front to rear. Does not include movable partitions covered in Chapter 25 nor the functional and maintenance aspects of variable aerodynamic fairings covered in Chapter 27." ;
        rdfs:label       "MAIN FRAME" ;
        rdfs:subClassOf  rel:Component ;
        ata:has-id       "5310" .

ata:ata-25-40  rdf:type  owl:Class ;
        rdfs:comment     "The toilet and dressing room areas containing wash basins, dressing tables, and water closet. Includes items such as mirrors, seats, cabinets, dispensing equipment, electrical outlets, wiring, etc. Wash basins and water closets are included in Chapter 38." ;
        rdfs:label       "LAVATORIES" ;
        rdfs:subClassOf  rel:Component ;
        ata:has-id       "2540" .

ata:ata-38-20  rdf:type  owl:Class ;
        rdfs:comment     "That portion of the system which is used to store and deliver wash water which is not potable." ;
        rdfs:label       "WASH" ;
        rdfs:subClassOf  rel:Component ;
        ata:has-id       "3820" .

ata:ata-45-05  rdf:type  owl:Class ;
        rdfs:comment     "Central Maintenance System interfaces with General Aircraft systems and identification of maintenance functions related to Aircraft General." ;
        rdfs:label       "CMS / AIRCRAFT GENERAL" ;
        rdfs:subClassOf  rel:Component ;
        ata:has-id       "4505" .

<http://onto.fel.cvut.cz/voc/ata-100/ata-72(T)-60>
        rdf:type         owl:Class ;
        rdfs:comment     "The mechanical power take-offs to drive accessories. Includes items such as engine-mounted gear boxes, gears, seals, pumps, etc. Does not include remotely installed gear boxes which are covered in Chapter 83." ;
        rdfs:label       "ACCESSORY DRIVES" ;
        rdfs:subClassOf  rel:Component ;
        ata:has-id       "72(T)60" .

ata:ata-71-20  rdf:type  owl:Class ;
        rdfs:comment     "The frame work, either of build-up construction or forgings which support the engine and attach it to the nacelle or pylon. Includes items such as engine mounts, vibration dampeners, support links, mounting bolts, etc." ;
        rdfs:label       "MOUNTS" ;
        rdfs:subClassOf  rel:Component ;
        ata:has-id       "7120" .

ata:ata-57  rdf:type     owl:Class ;
        rdfs:comment     "Center wing and outer wing structural units and associated components and members which support the aircraft in flight. Includes spars, skin, ribs, stringers, clamshells, scuppers, etc., and integral fuel tank structure of the flaps, slats, ailerons or elevons (complete with tabs), spoilers, and wing folding system." ;
        rdfs:label       "WINGS" ;
        rdfs:subClassOf  rel:Component .

_:b22   rdf:type            owl:Restriction ;
        owl:onProperty      rel:hasComponent ;
        owl:someValuesFrom  ata:ata-57-60 .

ata:ata-57  rdfs:subClassOf  _:b22 .

_:b23   rdf:type            owl:Restriction ;
        owl:onProperty      rel:hasComponent ;
        owl:someValuesFrom  ata:ata-57-20 .

ata:ata-57  rdfs:subClassOf  _:b23 .

_:b24   rdf:type            owl:Restriction ;
        owl:onProperty      rel:hasComponent ;
        owl:someValuesFrom  ata:ata-57-50 .

ata:ata-57  rdfs:subClassOf  _:b24 .

_:b25   rdf:type            owl:Restriction ;
        owl:onProperty      rel:hasComponent ;
        owl:someValuesFrom  ata:ata-57-70 .

ata:ata-57  rdfs:subClassOf  _:b25 .

_:b26   rdf:type            owl:Restriction ;
        owl:onProperty      rel:hasComponent ;
        owl:someValuesFrom  ata:ata-57-90 .

ata:ata-57  rdfs:subClassOf  _:b26 .

_:b27   rdf:type            owl:Restriction ;
        owl:onProperty      rel:hasComponent ;
        owl:someValuesFrom  ata:ata-57-30 .

ata:ata-57  rdfs:subClassOf  _:b27 .

_:b28   rdf:type            owl:Restriction ;
        owl:onProperty      rel:hasComponent ;
        owl:someValuesFrom  ata:ata-57-80 .

ata:ata-57  rdfs:subClassOf  _:b28 .

_:b29   rdf:type            owl:Restriction ;
        owl:onProperty      rel:hasComponent ;
        owl:someValuesFrom  ata:ata-57-40 .

ata:ata-57  rdfs:subClassOf  _:b29 .

_:b30   rdf:type            owl:Restriction ;
        owl:onProperty      rel:hasComponent ;
        owl:someValuesFrom  ata:ata-57-10 .

ata:ata-57  rdfs:subClassOf  _:b30 ;
        rel:hasComponent  ata:ata-57-50 ;
        rel:hasComponent  ata:ata-57-60 ;
        rel:hasComponent  ata:ata-57-20 ;
        rel:hasComponent  ata:ata-57-10 ;
        rel:hasComponent  ata:ata-57-40 ;
        rel:hasComponent  ata:ata-57-90 ;
        rel:hasComponent  ata:ata-57-30 ;
        rel:hasComponent  ata:ata-57-80 ;
        rel:hasComponent  ata:ata-57-70 ;
        ata:has-id        "57" .

ata:ata-51-10  rdf:type  owl:Class ;
        rdfs:comment     "Definition of damage classifications. Cleanup of dents, cracks, scratches, corrosion, etc. Aerodynamic smoothness requirements for the airplane, and permissible contour variations, gaps, and mismatch data." ;
        rdfs:label       "INVESTIGATION, CLEANUP AND AERODYNAMIC SMOOTHNESS" ;
        rdfs:subClassOf  rel:Component ;
        ata:has-id       "5110" .

ata:ata-56-30  rdf:type  owl:Class ;
        rdfs:comment     "Doors used for entrance and exit of the passengers, flight crew and service personnel to and from the airplane. Includes items such as transparent material, its frame, etc. Does not include emergency exit windows." ;
        rdfs:label       "DOOR" ;
        rdfs:subClassOf  rel:Component ;
        ata:has-id       "5630" .

ata:ata-25  rdf:type     owl:Class ;
        rdfs:comment     "Those removable items of equipment and furnishings externally mounted on the aircraft or contained in the flight, passenger, cargo, and accessory compartments. Includes emergency, buffet, and lavatory equipment. Does not include structures of equipment assigned specifically to other chapters." ;
        rdfs:label       "EQUIPMENT / FURNISHINGS" ;
        rdfs:subClassOf  rel:Component .

_:b31   rdf:type            owl:Restriction ;
        owl:onProperty      rel:hasComponent ;
        owl:someValuesFrom  ata:ata-25-30 .

ata:ata-25  rdfs:subClassOf  _:b31 .

_:b32   rdf:type            owl:Restriction ;
        owl:onProperty      rel:hasComponent ;
        owl:someValuesFrom  ata:ata-25-50 .

ata:ata-25  rdfs:subClassOf  _:b32 .

_:b33   rdf:type            owl:Restriction ;
        owl:onProperty      rel:hasComponent ;
        owl:someValuesFrom  ata:ata-25-40 .

ata:ata-25  rdfs:subClassOf  _:b33 .

_:b34   rdf:type            owl:Restriction ;
        owl:onProperty      rel:hasComponent ;
        owl:someValuesFrom  ata:ata-25-60 .

ata:ata-25  rdfs:subClassOf  _:b34 .

_:b35   rdf:type            owl:Restriction ;
        owl:onProperty      rel:hasComponent ;
        owl:someValuesFrom  ata:ata-25-70 .

ata:ata-25  rdfs:subClassOf  _:b35 .

_:b36   rdf:type            owl:Restriction ;
        owl:onProperty      rel:hasComponent ;
        owl:someValuesFrom  ata:ata-25-20 .

ata:ata-25  rdfs:subClassOf  _:b36 .

_:b37   rdf:type            owl:Restriction ;
        owl:onProperty      rel:hasComponent ;
        owl:someValuesFrom  ata:ata-25-80 .

ata:ata-25  rdfs:subClassOf  _:b37 .

_:b38   rdf:type            owl:Restriction ;
        owl:onProperty      rel:hasComponent ;
        owl:someValuesFrom  ata:ata-25-10 .

ata:ata-25  rdfs:subClassOf  _:b38 ;
        rel:hasComponent  ata:ata-25-80 ;
        rel:hasComponent  ata:ata-25-60 ;
        rel:hasComponent  ata:ata-25-40 ;
        rel:hasComponent  ata:ata-25-10 ;
        rel:hasComponent  ata:ata-25-20 ;
        rel:hasComponent  ata:ata-25-70 ;
        rel:hasComponent  ata:ata-25-50 ;
        rel:hasComponent  ata:ata-25-30 ;
        ata:has-id        "25" .

ata:ata-23-40  rdf:type  owl:Class ;
        rdfs:comment     "That portion of the system which is used by flight and ground personnel to communicate between areas on the aircraft. Includes items such as amplifier, handset, etc. Does not include the interphone system within the flight compartment which is part of the integrating system." ;
        rdfs:label       "INTERPHONE" ;
        rdfs:subClassOf  rel:Component ;
        ata:has-id       "2340" .

ata:ata-71  rdf:type     owl:Class ;
        rdfs:comment     "The overall power package inclusive of engine, air intake, mount, cowling, scoops, cowl flaps." ;
        rdfs:label       "POWER PLANT - GENERAL" ;
        rdfs:subClassOf  rel:Component .

_:b39   rdf:type            owl:Restriction ;
        owl:onProperty      rel:hasComponent ;
        owl:someValuesFrom  ata:ata-71-70 .

ata:ata-71  rdfs:subClassOf  _:b39 .

_:b40   rdf:type            owl:Restriction ;
        owl:onProperty      rel:hasComponent ;
        owl:someValuesFrom  ata:ata-71-20 .

ata:ata-71  rdfs:subClassOf  _:b40 .

_:b41   rdf:type            owl:Restriction ;
        owl:onProperty      rel:hasComponent ;
        owl:someValuesFrom  ata:ata-71-60 .

ata:ata-71  rdfs:subClassOf  _:b41 .

_:b42   rdf:type            owl:Restriction ;
        owl:onProperty      rel:hasComponent ;
        owl:someValuesFrom  ata:ata-71-50 .

ata:ata-71  rdfs:subClassOf  _:b42 .

_:b43   rdf:type            owl:Restriction ;
        owl:onProperty      rel:hasComponent ;
        owl:someValuesFrom  ata:ata-71-10 .

ata:ata-71  rdfs:subClassOf  _:b43 .

_:b44   rdf:type            owl:Restriction ;
        owl:onProperty      rel:hasComponent ;
        owl:someValuesFrom  ata:ata-71-40 .

ata:ata-71  rdfs:subClassOf  _:b44 .

_:b45   rdf:type            owl:Restriction ;
        owl:onProperty      rel:hasComponent ;
        owl:someValuesFrom  ata:ata-71-30 .

ata:ata-71  rdfs:subClassOf  _:b45 ;
        rel:hasComponent  ata:ata-71-30 ;
        rel:hasComponent  ata:ata-71-10 ;
        rel:hasComponent  ata:ata-71-70 ;
        rel:hasComponent  ata:ata-71-60 ;
        rel:hasComponent  ata:ata-71-40 ;
        rel:hasComponent  ata:ata-71-50 ;
        rel:hasComponent  ata:ata-71-20 ;
        ata:has-id        "71" .

ata:ata-36-20  rdf:type  owl:Class ;
        rdfs:comment     "That portion of the system which is used to indicate temperature and pressure of the pneumatic system. Includes temperature and pressure warning systems." ;
        rdfs:label       "INDICATING" ;
        rdfs:subClassOf  rel:Component ;
        ata:has-id       "3620" .

ata:ata-54-30  rdf:type  owl:Class ;
        rdfs:label       "[AS REQUIRED]" ;
        rdfs:subClassOf  rel:Component ;
        ata:has-id       "5430" .

ata:ata-67-10  rdf:type  owl:Class ;
        rdfs:comment     "That portion of the system which controls the attitude by the angle of attack of the rotor blades. Includes items such as collective pitch lever, cyclic pitch stick and corresponding linkage and cable controls, coupling, and mixing units, and artificial feel unit system. Also includes the control position indicating system." ;
        rdfs:label       "ROTOR CONTROL" ;
        rdfs:subClassOf  rel:Component ;
        ata:has-id       "6710" .

ata:ata-21-40  rdf:type  owl:Class ;
        rdfs:comment     "That portion of the system and its controls which supply heated air. Includes items such as heater panels and other units, fuel system and control, ignition, indicating systems related to heater operation, wiring, etc. Does not include temperature control and indicating systems." ;
        rdfs:label       "HEATING" ;
        rdfs:subClassOf  rel:Component ;
        ata:has-id       "2140" .

ata:ata-34-20  rdf:type  owl:Class ;
        rdfs:comment     "The portion of the system which uses magnetic or inertia forces to sense and display the direction or attitude of the aircraft. This includes sensing, computing, indicating and warning devices such as magnetic compasses, vertical and directional references, magnetic heading systems, attitude director systems, symbol generators, turn and bank, rate of turn, amplifiers, indicators, etc. Includes Flight Director when it is not integral with the auto pilot computation." ;
        rdfs:label       "ATTITUDE AND DIRECTION" ;
        rdfs:subClassOf  rel:Component ;
        ata:has-id       "3420" .

ata:ata-39-40  rdf:type  owl:Class ;
        rdfs:label       "MULTIPURPOSE ELECTRONIC COMPONENTS" ;
        rdfs:subClassOf  rel:Component ;
        ata:has-id       "3940" .

<http://onto.fel.cvut.cz/voc/ata-100/ata-72(R)-30>
        rdf:type         owl:Class ;
        rdfs:comment     "The section of the engine which contains the cylinders, valves, pistons, push rods, intake pipes, baffles, etc. Also includes rocker arm assembly, valve springs, etc." ;
        rdfs:label       "CYLINDER SECTION" ;
        rdfs:subClassOf  rel:Component ;
        ata:has-id       "72(R)30" .

ata:ata-52-30  rdf:type  owl:Class ;
        rdfs:comment     "Exterior doors used primarily to gain access to cargo compartments. Includes items such as structure, latching mechanisms, handles, insulation, lining, controls, integral steps, ramps, handrails, attach/attached fittings, etc." ;
        rdfs:label       "CARGO" ;
        rdfs:subClassOf  rel:Component ;
        ata:has-id       "5230" .

ata:ata-57-50  rdf:type  owl:Class ;
        rdfs:comment     "Trailing Edge Devices Skins and structure of the wing and trailing edge and removable edge airfoils such as flaps and attach/attached fittings." ;
        rdfs:label       "TRAILING EDGE AND TRAILING EDGE DEVICES" ;
        rdfs:subClassOf  rel:Component ;
        ata:has-id       "5750" .

ata:ata-65-10  rdf:type  owl:Class ;
        rdfs:comment     "Drive shafts, bearings, flexible couplings." ;
        rdfs:label       "SHAFTS" ;
        rdfs:subClassOf  rel:Component ;
        ata:has-id       "6510" .

ata:ata-24-60  rdf:type  owl:Class ;
        rdfs:comment     "That portion of the system which provides for connection of DC power to using systems. Includes items such as DC main and secondary busses, main system circuit breakers, power system devices, etc." ;
        rdfs:label       "DC ELECTRICAL LOAD DISTRIBUTION" ;
        rdfs:subClassOf  rel:Component ;
        ata:has-id       "2460" .

ata:ata-32-20  rdf:type  owl:Class ;
        rdfs:comment     "That portion of the system which supports the nose of the aircraft while the aircraft is on the ground. Includes items such as shock struts, drag struts, linkages, attach bolts, etc." ;
        rdfs:label       "NOSE GEAR / TAIL GEAR AND DOORS" ;
        rdfs:subClassOf  rel:Component ;
        ata:has-id       "3220" .

ata:ata-38  rdf:type     owl:Class ;
        rdfs:comment     "Those fixed units and components which store and deliver for use, fresh water, and those fixed components which store and furnish a means of removal of water and waste. Includes wash basins, toilet assemblies, tanks, valves, etc." ;
        rdfs:label       "WATER / WASTE" ;
        rdfs:subClassOf  rel:Component .

_:b46   rdf:type            owl:Restriction ;
        owl:onProperty      rel:hasComponent ;
        owl:someValuesFrom  ata:ata-38-40 .

ata:ata-38  rdfs:subClassOf  _:b46 .

_:b47   rdf:type            owl:Restriction ;
        owl:onProperty      rel:hasComponent ;
        owl:someValuesFrom  ata:ata-38-30 .

ata:ata-38  rdfs:subClassOf  _:b47 .

_:b48   rdf:type            owl:Restriction ;
        owl:onProperty      rel:hasComponent ;
        owl:someValuesFrom  ata:ata-38-20 .

ata:ata-38  rdfs:subClassOf  _:b48 .

_:b49   rdf:type            owl:Restriction ;
        owl:onProperty      rel:hasComponent ;
        owl:someValuesFrom  ata:ata-38-10 .

ata:ata-38  rdfs:subClassOf  _:b49 ;
        rel:hasComponent  ata:ata-38-30 ;
        rel:hasComponent  ata:ata-38-40 ;
        rel:hasComponent  ata:ata-38-20 ;
        rel:hasComponent  ata:ata-38-10 ;
        ata:has-id        "38" .

ata:ata-84  rdf:type     owl:Class ;
        rdfs:comment     "Those units and components that, independent of the primary propulsion system, furnish additional thrust of short duration. Includes solid or liquid propellants, controls, indicator, etc." ;
        rdfs:label       "PROPULSION AUGMENTATION" ;
        rdfs:subClassOf  rel:Component .

_:b50   rdf:type            owl:Restriction ;
        owl:onProperty      rel:hasComponent ;
        owl:someValuesFrom  ata:ata-84-10 .

ata:ata-84  rdfs:subClassOf  _:b50 ;
        rel:hasComponent  ata:ata-84-10 ;
        ata:has-id        "84" .

ata:ata-52  rdf:type     owl:Class ;
        rdfs:comment     "Removable units used for entrance or exit, and for enclosing other structure contained within the fuselage. Includes passenger and crew doors, cargo doors, emergency exits, etc. Electrical and hydraulic systems associated with door control are included as appropriate." ;
        rdfs:label       "DOORS" ;
        rdfs:subClassOf  rel:Component .

_:b51   rdf:type            owl:Restriction ;
        owl:onProperty      rel:hasComponent ;
        owl:someValuesFrom  ata:ata-52-80 .

ata:ata-52  rdfs:subClassOf  _:b51 .

_:b52   rdf:type            owl:Restriction ;
        owl:onProperty      rel:hasComponent ;
        owl:someValuesFrom  ata:ata-52-60 .

ata:ata-52  rdfs:subClassOf  _:b52 .

_:b53   rdf:type            owl:Restriction ;
        owl:onProperty      rel:hasComponent ;
        owl:someValuesFrom  ata:ata-52-20 .

ata:ata-52  rdfs:subClassOf  _:b53 .

_:b54   rdf:type            owl:Restriction ;
        owl:onProperty      rel:hasComponent ;
        owl:someValuesFrom  ata:ata-52-40 .

ata:ata-52  rdfs:subClassOf  _:b54 .

_:b55   rdf:type            owl:Restriction ;
        owl:onProperty      rel:hasComponent ;
        owl:someValuesFrom  ata:ata-52-30 .

ata:ata-52  rdfs:subClassOf  _:b55 .

_:b56   rdf:type            owl:Restriction ;
        owl:onProperty      rel:hasComponent ;
        owl:someValuesFrom  ata:ata-52-70 .

ata:ata-52  rdfs:subClassOf  _:b56 .

_:b57   rdf:type            owl:Restriction ;
        owl:onProperty      rel:hasComponent ;
        owl:someValuesFrom  ata:ata-52-10 .

ata:ata-52  rdfs:subClassOf  _:b57 .

_:b58   rdf:type            owl:Restriction ;
        owl:onProperty      rel:hasComponent ;
        owl:someValuesFrom  ata:ata-52-50 .

ata:ata-52  rdfs:subClassOf  _:b58 ;
        rel:hasComponent  ata:ata-52-10 ;
        rel:hasComponent  ata:ata-52-40 ;
        rel:hasComponent  ata:ata-52-50 ;
        rel:hasComponent  ata:ata-52-70 ;
        rel:hasComponent  ata:ata-52-20 ;
        rel:hasComponent  ata:ata-52-80 ;
        rel:hasComponent  ata:ata-52-30 ;
        rel:hasComponent  ata:ata-52-60 ;
        ata:has-id        "52" .

ata:ata-83-20  rdf:type  owl:Class ;
        rdfs:comment     "The case which contains the gear trains and shafts. Includes items such as gears, shafts, seals, oil pumps, coolers, etc." ;
        rdfs:label       "GEAR BOX SECTION" ;
        rdfs:subClassOf  rel:Component ;
        ata:has-id       "8320" .

ata:ata-63-10  rdf:type  owl:Class ;
        rdfs:comment     "Drive shaft(s) between engine(s) and main gear box(es) and, if applicable, clutch and free wheel unit(s)." ;
        rdfs:label       "ENGINE / GEARBOX COUPLINGS" ;
        rdfs:subClassOf  rel:Component ;
        ata:has-id       "6310" .

ata:ata-27-80  rdf:type  owl:Class ;
        rdfs:comment     "That portion of the systems which controls the position and movement of variable opening wings slots, leading edge wing flaps, and other similar auxiliary devices used for increasing aerodynamic lift. Includes items such as control handles, cables, actuators, linkages, warning systems, control surfaces, position indicators, etc. Does not include trailing edge flaps." ;
        rdfs:label       "LIFT AUGMENTING" ;
        rdfs:subClassOf  rel:Component ;
        ata:has-id       "2780" .

ata:ata-30-20  rdf:type  owl:Class ;
        rdfs:comment     "That portion of the system which is used to eliminate or prevent the formation of ice in or around air intakes. Includes power plant cowling anti-icing." ;
        rdfs:label       "AIR INTAKES" ;
        rdfs:subClassOf  rel:Component ;
        ata:has-id       "3020" .

ata:ata-81-20  rdf:type  owl:Class ;
        rdfs:comment     "The turbines which extract energy from the exhaust gases and drive an air compressor." ;
        rdfs:label       "TURBO-SUPERCHARGER" ;
        rdfs:subClassOf  rel:Component ;
        ata:has-id       "8120" .

ata:ata-53-50  rdf:type  owl:Class ;
        rdfs:label       "AERODYNAMIC FAIRINGS" ;
        rdfs:subClassOf  rel:Component ;
        ata:has-id       "5350" .

ata:ata-61-10  rdf:type  owl:Class ;
        rdfs:comment     "That portion of the system which rotates except the engine propeller shaft. Includes items such as blades, dome, hub, spinner, slip ring, deicer boot, distributor valve, etc." ;
        rdfs:label       "PROPELLER ASSEMBLY" ;
        rdfs:subClassOf  rel:Component ;
        ata:has-id       "6110" .

ata:ata-66-30  rdf:type  owl:Class ;
        rdfs:comment     "Part of the system intended for controlling folding/spreading sequences and for indicating the system operation. Includes the control units, caption lights, indicators, wiring, etc." ;
        rdfs:label       "CONTROLS AND INDICATING" ;
        rdfs:subClassOf  rel:Component ;
        ata:has-id       "6630" .

ata:ata-25-80  rdf:type  owl:Class ;
        rdfs:comment     "Those insulation blankets which are used for heat and sound insulation. Includes flight compartments, passenger compartment, cargo and accessory compartment insulation, etc." ;
        rdfs:label       "INSULATION" ;
        rdfs:subClassOf  rel:Component ;
        ata:has-id       "2580" .

ata:ata-79-10  rdf:type  owl:Class ;
        rdfs:comment     "That portion of the system used for storage of oil. Includes items such as tanks, filling systems, internal hoppers, baffles, tank sump and drain, etc. Does not include tanks which are an integral portion of the engine." ;
        rdfs:label       "STORAGE (DRY SUMP)" ;
        rdfs:subClassOf  rel:Component ;
        ata:has-id       "7910" .

ata:ata-33-40  rdf:type  owl:Class ;
        rdfs:comment     "The lighting sub-systems used to provide illumination outside of the aircraft. Includes lights such as landing, navigation, position indicating, wing illumination, rotating, courtesy, taxi, etc." ;
        rdfs:label       "EXTERIOR LIGHTING" ;
        rdfs:subClassOf  rel:Component ;
        ata:has-id       "3340" .

ata:ata-46-20  rdf:type  owl:Class ;
        rdfs:comment     "That portion of the onboard information system that supports the flight deck systems, flight deck crew and flight operations." ;
        rdfs:label       "FLIGHT DECK INFORMATION SYSTEMS" ;
        rdfs:subClassOf  rel:Component ;
        ata:has-id       "4620" .

ata:ata-45-45  rdf:type  owl:Class ;
        rdfs:comment     "Central Maintenance System That portion of the system which interfaces with other airplane systems, flight line mechanics, and radio communications. Includes computers, storage devices, control and display devices." ;
        rdfs:label       "CENTRAL MAINTENANCE SYSTEM" ;
        rdfs:subClassOf  rel:Component ;
        ata:has-id       "4545" .

ata:ata-71-60  rdf:type  owl:Class ;
        rdfs:comment     "That portion of the power plant system which directs and may or may not vary the mass air flow to the engine. Includes items such as nose ring cowls, scoops, compressor fan cowls, buried engine ducts, vortex generators, actuators, control handles, cables, wiring, plumbing, linkages, doors, warning systems, position indicators, etc. Does not include integral structure with the airframe, which shall be included in the applicable Structures chapter." ;
        rdfs:label       "ENGINE AIR INTAKES" ;
        rdfs:subClassOf  rel:Component ;
        ata:has-id       "7160" .

ata:ata-51-50  rdf:type  owl:Class ;
        rdfs:comment     "Procedure for supporting the airplane to relieve loads during repairs. Includes locations for supports and contour dimensions for required ground equipment." ;
        rdfs:label       "SUPPORT OF AIRPLANE FOR REPAIR AND ALIGNMENT CHECK PROCEDURES" ;
        rdfs:subClassOf  rel:Component ;
        ata:has-id       "5150" .

ata:ata-65  rdf:type     owl:Class ;
        rdfs:comment     "Includes all the components transmitting power to the tail rotor: drive shafts, bearings, gearboxes." ;
        rdfs:label       "TAIL ROTOR DRIVE" ;
        rdfs:subClassOf  rel:Component .

_:b59   rdf:type            owl:Restriction ;
        owl:onProperty      rel:hasComponent ;
        owl:someValuesFrom  ata:ata-65-20 .

ata:ata-65  rdfs:subClassOf  _:b59 .

_:b60   rdf:type            owl:Restriction ;
        owl:onProperty      rel:hasComponent ;
        owl:someValuesFrom  ata:ata-65-40 .

ata:ata-65  rdfs:subClassOf  _:b60 .

_:b61   rdf:type            owl:Restriction ;
        owl:onProperty      rel:hasComponent ;
        owl:someValuesFrom  ata:ata-65-30 .

ata:ata-65  rdfs:subClassOf  _:b61 .

_:b62   rdf:type            owl:Restriction ;
        owl:onProperty      rel:hasComponent ;
        owl:someValuesFrom  ata:ata-65-10 .

ata:ata-65  rdfs:subClassOf  _:b62 ;
        rel:hasComponent  ata:ata-65-20 ;
        rel:hasComponent  ata:ata-65-30 ;
        rel:hasComponent  ata:ata-65-10 ;
        rel:hasComponent  ata:ata-65-40 ;
        ata:has-id        "65" .

ata:ata-64-30  rdf:type  owl:Class ;
        rdfs:label       "[AVAILABLE]" ;
        rdfs:subClassOf  rel:Component ;
        ata:has-id       "6430" .

ata:ata-23-80  rdf:type  owl:Class ;
        rdfs:comment     "That portion of the system which maintains integrated control of the operating frequencies of communication and navigation transmitter/receivers after either a manually inserted command or a preprogrammed integrated flight system command. Includes such items as integrated frequency selector panels, digital frequency control computers, integrated frequency display panels, etc." ;
        rdfs:label       "INTEGRATED AUTOMATIC TUNING" ;
        rdfs:subClassOf  rel:Component ;
        ata:has-id       "2380" .

ata:ata-77-10  rdf:type  owl:Class ;
        rdfs:comment     "That portion of the system which directly or indirectly indicates power or thrust. Includes items such as BMEP, pressure-ratio, RPM, etc." ;
        rdfs:label       "POWER" ;
        rdfs:subClassOf  rel:Component ;
        ata:has-id       "7710" .

ata:ata-31-40  rdf:type  owl:Class ;
        rdfs:comment     "Those systems and components used for computing data from a number of different sources without a preponderance of functions in any one system. Includes items such as Digital Core Avionic System (DCAS), stored check list, emergency procedures, company regulations, etc., for call up on a display, integrated instrument systems such as engine, airplane power and central warning indicators when combined into a central display." ;
        rdfs:label       "CENTRAL COMPUTERS" ;
        rdfs:subClassOf  rel:Component ;
        ata:has-id       "3140" .

ata:ata-33  rdf:type     owl:Class ;
        rdfs:comment     "Those units and components (electrically powered) which provide for external and internal illumination such as landing lights, taxi lights, position lights, rotating lights, ice lights, master warning lights, passenger reading and cabin dome lights, etc. Includes light fixtures, switches and wiring. Does not include warning lights for individual systems or self -illuminating signs (see Chapter 11)." ;
        rdfs:label       "LIGHTS" ;
        rdfs:subClassOf  rel:Component .

_:b63   rdf:type            owl:Restriction ;
        owl:onProperty      rel:hasComponent ;
        owl:someValuesFrom  ata:ata-33-20 .

ata:ata-33  rdfs:subClassOf  _:b63 .

_:b64   rdf:type            owl:Restriction ;
        owl:onProperty      rel:hasComponent ;
        owl:someValuesFrom  ata:ata-33-30 .

ata:ata-33  rdfs:subClassOf  _:b64 .

_:b65   rdf:type            owl:Restriction ;
        owl:onProperty      rel:hasComponent ;
        owl:someValuesFrom  ata:ata-33-50 .

ata:ata-33  rdfs:subClassOf  _:b65 .

_:b66   rdf:type            owl:Restriction ;
        owl:onProperty      rel:hasComponent ;
        owl:someValuesFrom  ata:ata-33-40 .

ata:ata-33  rdfs:subClassOf  _:b66 .

_:b67   rdf:type            owl:Restriction ;
        owl:onProperty      rel:hasComponent ;
        owl:someValuesFrom  ata:ata-33-10 .

ata:ata-33  rdfs:subClassOf  _:b67 ;
        rel:hasComponent  ata:ata-33-20 ;
        rel:hasComponent  ata:ata-33-10 ;
        rel:hasComponent  ata:ata-33-40 ;
        rel:hasComponent  ata:ata-33-30 ;
        rel:hasComponent  ata:ata-33-50 ;
        ata:has-id        "33" .

ata:ata-49-40  rdf:type  owl:Class ;
        rdfs:comment     "For definitions see Chapter 74 and 80." ;
        rdfs:label       "IGNITION / STARTING" ;
        rdfs:subClassOf  rel:Component ;
        ata:has-id       "4940" .

ata:ata-82-40  rdf:type  owl:Class ;
        rdfs:comment     "That portion of the system which is used to indicate the quantity, temperature, and pressure of the water mixtures. Includes items such as transmitters, indicators, wiring, etc." ;
        rdfs:label       "INDICATING" ;
        rdfs:subClassOf  rel:Component ;
        ata:has-id       "8240" .

ata:ata-54-70  rdf:type  owl:Class ;
        rdfs:label       "[AS REQUIRED]" ;
        rdfs:subClassOf  rel:Component ;
        ata:has-id       "5470" .

ata:ata-62-30  rdf:type  owl:Class ;
        rdfs:comment     "Rotor shaft(s) / swashplate assembly(ies) not included in -20." ;
        rdfs:label       "ROTOR SHAFT(S) / SWASHPLATE ASSEMBLY(IES)" ;
        rdfs:subClassOf  rel:Component ;
        ata:has-id       "6230" .

ata:ata-75-10  rdf:type  owl:Class ;
        rdfs:comment     "That portion of the system which is used to eliminate and prevent the formation of ice by bleed air in al parts of the engine, excluding power plant cowling which is covered by Chapter 30. Includes items such as valves, plumbing, wiring, regulators, etc. Electrical anti-icing is covered in Chapter 30." ;
        rdfs:label       "ENGINE ANTI-ICING" ;
        rdfs:subClassOf  rel:Component ;
        ata:has-id       "7510" .

ata:ata-34-60  rdf:type  owl:Class ;
        rdfs:comment     "That portion of the system which combines navigational data to compute or manage the aircraft's geographical position or theoretical flight path. Includes items such as course computers, flight management computers, performance data computers, and associated control display units, warning annunciators, etc." ;
        rdfs:label       "FLIGHT MANAGEMENT COMPUTING" ;
        rdfs:subClassOf  rel:Component ;
        ata:has-id       "3460" .

ata:ata-52-70  rdf:type  owl:Class ;
        rdfs:comment     "That portion of the system which is used to indicate whether the doors are closed and properly latched. Includes items such as switches, lights, bells, horns, etc. Does not include landing gear door warning which is covered in Chapter 32." ;
        rdfs:label       "DOOR WARNING" ;
        rdfs:subClassOf  rel:Component ;
        ata:has-id       "5270" .

ata:ata-57-90  rdf:type  owl:Class ;
        rdfs:comment     "System that controls the on-ground movement of any portion of the main wing structure. Includes mechanisms, linkages, actuators, locks, indicating/warning systems, etc." ;
        rdfs:label       "WING FOLDING SYSTEM" ;
        rdfs:subClassOf  rel:Component ;
        ata:has-id       "5790" .

ata:ata-73-10  rdf:type  owl:Class ;
        rdfs:comment     "That portion of the system from the main quick disconnect to the engine, which distributes fuel to the engine burner section and the thrust augmentor. Includes items such as plumbing, pumps, temperature regulator, valves, filters, manifold, nozzles, etc. Does not include main of thrust augmentor control." ;
        rdfs:label       "DISTRIBUTION" ;
        rdfs:subClassOf  rel:Component ;
        ata:has-id       "7310" .

ata:ata-78-30  rdf:type  owl:Class ;
        rdfs:comment     "That portion of the system which is used to change the direction of the exhast gases for reverse thrust. Includes items such as clamshells, linkages, levers, actuator, plumbing, wiring, indicators, warning systems, etc. Use -10 where integral part of nozzle system." ;
        rdfs:label       "THRUST REVERSER" ;
        rdfs:subClassOf  rel:Component ;
        ata:has-id       "7830" .

ata:ata-32-60  rdf:type  owl:Class ;
        rdfs:comment     "That portion of the system which is used to indicate and warn of the position of the landing gear/doors. Includes items such as switches, relays, lights, indicators, horns, wiring, etc." ;
        rdfs:label       "POSITION, WARNING, AND GROUND SAFETY SWITCH" ;
        rdfs:subClassOf  rel:Component ;
        ata:has-id       "3260" .

ata:ata-78  rdf:type     owl:Class ;
        rdfs:comment     "Those units and components which direct the engine exhaust gases overboard. For turbine engines, includes units external to the basic engine such as thrust reverser and noise suppressor. For reciprocating engines, includes augmentors, stacks, clamps, etc. Excludes exhaust-driven turbines." ;
        rdfs:label       "EXHAUST" ;
        rdfs:subClassOf  rel:Component .

_:b68   rdf:type            owl:Restriction ;
        owl:onProperty      rel:hasComponent ;
        owl:someValuesFrom  ata:ata-78-10 .

ata:ata-78  rdfs:subClassOf  _:b68 .

_:b69   rdf:type            owl:Restriction ;
        owl:onProperty      rel:hasComponent ;
        owl:someValuesFrom  ata:ata-78-40 .

ata:ata-78  rdfs:subClassOf  _:b69 .

_:b70   rdf:type            owl:Restriction ;
        owl:onProperty      rel:hasComponent ;
        owl:someValuesFrom  ata:ata-78-30 .

ata:ata-78  rdfs:subClassOf  _:b70 .

_:b71   rdf:type            owl:Restriction ;
        owl:onProperty      rel:hasComponent ;
        owl:someValuesFrom  ata:ata-78-20 .

ata:ata-78  rdfs:subClassOf  _:b71 ;
        rel:hasComponent  ata:ata-78-40 ;
        rel:hasComponent  ata:ata-78-30 ;
        rel:hasComponent  ata:ata-78-10 ;
        rel:hasComponent  ata:ata-78-20 ;
        ata:has-id        "78" .

ata:ata-23-15  rdf:type  owl:Class ;
        rdfs:comment     "That portion of the system which utilizes satellite communication systems (SATCOM)." ;
        rdfs:label       "SATCOM" ;
        rdfs:subClassOf  rel:Component ;
        ata:has-id       "2315" .

ata:ata-29-10  rdf:type  owl:Class ;
        rdfs:comment     "That portion of the system which is used to store and deliver hydraulic fluid to using systems. Includes items such as tanks, accumulators, valves, pumps, levers, switches, cables, plumbing, wiring, external connectors, etc. Does not include the supply valves to the using systems." ;
        rdfs:label       "MAIN" ;
        rdfs:subClassOf  rel:Component ;
        ata:has-id       "2910" .

ata:ata-46  rdf:type     owl:Class ;
        rdfs:comment     "Those units and components which furnish a means of storing, updating, and retrieving digital information traditionally provided on paper, microfilm, or microfiche. Includes units that are dedicated to the information storage and retrieval function such as the Electronic Library mass storage and controller. Does not include units or components installed for other uses and shared with other systems, such as flight deck printer or general use display." ;
        rdfs:label       "INFORMATION SYSTEMS" ;
        rdfs:subClassOf  rel:Component .

_:b72   rdf:type            owl:Restriction ;
        owl:onProperty      rel:hasComponent ;
        owl:someValuesFrom  ata:ata-46-40 .

ata:ata-46  rdfs:subClassOf  _:b72 .

_:b73   rdf:type            owl:Restriction ;
        owl:onProperty      rel:hasComponent ;
        owl:someValuesFrom  ata:ata-46-10 .

ata:ata-46  rdfs:subClassOf  _:b73 .

_:b74   rdf:type            owl:Restriction ;
        owl:onProperty      rel:hasComponent ;
        owl:someValuesFrom  ata:ata-46-20 .

ata:ata-46  rdfs:subClassOf  _:b74 .

_:b75   rdf:type            owl:Restriction ;
        owl:onProperty      rel:hasComponent ;
        owl:someValuesFrom  ata:ata-46-30 .

ata:ata-46  rdfs:subClassOf  _:b75 .

_:b76   rdf:type            owl:Restriction ;
        owl:onProperty      rel:hasComponent ;
        owl:someValuesFrom  ata:ata-46-50 .

ata:ata-46  rdfs:subClassOf  _:b76 ;
        rel:hasComponent  ata:ata-46-30 ;
        rel:hasComponent  ata:ata-46-10 ;
        rel:hasComponent  ata:ata-46-40 ;
        rel:hasComponent  ata:ata-46-20 ;
        rel:hasComponent  ata:ata-46-50 ;
        ata:has-id        "46" .

ata:ata-60  rdf:type     owl:Class ;
        rdfs:label       "STANDARD PRACTICES - PROPELLER / ROTOR" ;
        rdfs:subClassOf  rel:Component ;
        ata:has-id       "60" .

ata:ata-30-60  rdf:type  owl:Class ;
        rdfs:comment     "That portion of the system which is used to eliminate or prevent the formation of ice on propellers or rotors. Includes all components up to but not including rotating assembly." ;
        rdfs:label       "PROPELLERS / ROTORS" ;
        rdfs:subClassOf  rel:Component ;
        ata:has-id       "3060" .

ata:group-power-plant
        rdf:type         owl:Class ;
        rdfs:label       "POWER PLANT" ;
        rdfs:subClassOf  rel:Component .

_:b77   rdf:type            owl:Restriction ;
        owl:onProperty      rel:hasComponent ;
        owl:someValuesFrom  ata:ata-74 .

ata:group-power-plant
        rdfs:subClassOf  _:b77 .

_:b78   rdf:type            owl:Restriction ;
        owl:onProperty      rel:hasComponent ;
        owl:someValuesFrom  ata:ata-81 .

ata:group-power-plant
        rdfs:subClassOf  _:b78 .

_:b79   rdf:type            owl:Restriction ;
        owl:onProperty      rel:hasComponent ;
        owl:someValuesFrom  ata:ata-80 .

ata:group-power-plant
        rdfs:subClassOf  _:b79 .

_:b80   rdf:type            owl:Restriction ;
        owl:onProperty      rel:hasComponent ;
        owl:someValuesFrom  ata:ata-73 .

ata:group-power-plant
        rdfs:subClassOf  _:b80 .

_:b81   rdf:type            owl:Restriction ;
        owl:onProperty      rel:hasComponent ;
        owl:someValuesFrom  ata:ata-77 .

ata:group-power-plant
        rdfs:subClassOf  _:b81 .

_:b82   rdf:type            owl:Restriction ;
        owl:onProperty      rel:hasComponent ;
        owl:someValuesFrom  ata:ata-78 .

ata:group-power-plant
        rdfs:subClassOf  _:b82 .

_:b83   rdf:type            owl:Restriction ;
        owl:onProperty      rel:hasComponent ;
        owl:someValuesFrom  <http://onto.fel.cvut.cz/voc/ata-100/ata-72(R)> .

ata:group-power-plant
        rdfs:subClassOf  _:b83 .

_:b84   rdf:type            owl:Restriction ;
        owl:onProperty      rel:hasComponent ;
        owl:someValuesFrom  ata:ata-83 .

ata:group-power-plant
        rdfs:subClassOf  _:b84 .

_:b85   rdf:type            owl:Restriction ;
        owl:onProperty      rel:hasComponent ;
        owl:someValuesFrom  ata:ata-75 .

ata:group-power-plant
        rdfs:subClassOf  _:b85 .

_:b86   rdf:type            owl:Restriction ;
        owl:onProperty      rel:hasComponent ;
        owl:someValuesFrom  ata:ata-84 .

ata:group-power-plant
        rdfs:subClassOf  _:b86 .

_:b87   rdf:type            owl:Restriction ;
        owl:onProperty      rel:hasComponent ;
        owl:someValuesFrom  ata:ata-79 .

ata:group-power-plant
        rdfs:subClassOf  _:b87 .

_:b88   rdf:type            owl:Restriction ;
        owl:onProperty      rel:hasComponent ;
        owl:someValuesFrom  <http://onto.fel.cvut.cz/voc/ata-100/ata-72(T)> .

ata:group-power-plant
        rdfs:subClassOf  _:b88 .

_:b89   rdf:type            owl:Restriction ;
        owl:onProperty      rel:hasComponent ;
        owl:someValuesFrom  ata:ata-82 .

ata:group-power-plant
        rdfs:subClassOf  _:b89 .

_:b90   rdf:type            owl:Restriction ;
        owl:onProperty      rel:hasComponent ;
        owl:someValuesFrom  ata:ata-71 .

ata:group-power-plant
        rdfs:subClassOf  _:b90 .

_:b91   rdf:type            owl:Restriction ;
        owl:onProperty      rel:hasComponent ;
        owl:someValuesFrom  ata:ata-70 .

ata:group-power-plant
        rdfs:subClassOf  _:b91 .

_:b92   rdf:type            owl:Restriction ;
        owl:onProperty      rel:hasComponent ;
        owl:someValuesFrom  ata:ata-76 .

ata:group-power-plant
        rdfs:subClassOf   _:b92 ;
        rel:hasComponent  ata:ata-74 ;
        rel:hasComponent  ata:ata-83 ;
        rel:hasComponent  ata:ata-78 ;
        rel:hasComponent  <http://onto.fel.cvut.cz/voc/ata-100/ata-72(T)> ;
        rel:hasComponent  <http://onto.fel.cvut.cz/voc/ata-100/ata-72(R)> ;
        rel:hasComponent  ata:ata-77 ;
        rel:hasComponent  ata:ata-81 ;
        rel:hasComponent  ata:ata-80 ;
        rel:hasComponent  ata:ata-75 ;
        rel:hasComponent  ata:ata-84 ;
        rel:hasComponent  ata:ata-79 ;
        rel:hasComponent  ata:ata-70 ;
        rel:hasComponent  ata:ata-73 ;
        rel:hasComponent  ata:ata-82 ;
        rel:hasComponent  ata:ata-71 ;
        rel:hasComponent  ata:ata-76 ;
        ata:has-id        "group-power-plant" .

ata:ata-27-10  rdf:type  owl:Class ;
        rdfs:comment     "That portion of the systems which controls the position and movement of the ailerons/elevons and tabs. Includes items such as the control wheels, cables, boosters, linkages, control surfaces, indicators, etc." ;
        rdfs:label       "AILERON AND TAB" ;
        rdfs:subClassOf  rel:Component ;
        ata:has-id       "2710" .

ata:ata-53-90  rdf:type  owl:Class ;
        rdfs:label       "[AS REQUIRED]" ;
        rdfs:subClassOf  rel:Component ;
        ata:has-id       "5390" .

ata:ata-61-50  rdf:type  owl:Class ;
        rdfs:comment     "The complete duct assembly including vector drive attachment, fairings, stators, gearbox covers, etc." ;
        rdfs:label       "PROPULSOR DUCT" ;
        rdfs:subClassOf  rel:Component ;
        ata:has-id       "6150" .

ata:ata-74-30  rdf:type  owl:Class ;
        rdfs:comment     "That portion of the system which provides a means of rendering the electrical power supply inoperative. Includes items such as ignition switches, wiring, connectors, etc." ;
        rdfs:label       "SWITCHING" ;
        rdfs:subClassOf  rel:Component ;
        ata:has-id       "7430" .

ata:ata-25-10  rdf:type  owl:Class ;
        rdfs:comment     "The compartment above the floor and between the forward passenger partition and the forward pressure dome. Includes items such as flight crew seats, tables, pilot check lists and food containers, wardrobes, curtains, manuals, electronic equipment rack, spare bulbs, fuses, etc. Does not include cargo compartments." ;
        rdfs:label       "FLIGHT COMPARTMENT" ;
        rdfs:subClassOf  rel:Component ;
        ata:has-id       "2510" .

<http://onto.fel.cvut.cz/voc/ata-100/ata-72(T)-30>
        rdf:type         owl:Class ;
        rdfs:comment     "The section of the engine in which the air is compressed. Includes items such as cases, vanes, shrouds, rotors, diffusers, etc. Also includes the maintenance and overhaul of stator blades but not the operation of variable stator blades which is covered under Chapter 75 - 30. Does not include compressor bleed section." ;
        rdfs:label       "COMPRESSOR SECTION" ;
        rdfs:subClassOf  rel:Component ;
        ata:has-id       "72(T)30" .

ata:ata-27  rdf:type     owl:Class ;
        rdfs:comment     "Those units and components which furnish a means of manually controlling the flight attitude characteristics of the aircraft, including items such as hydraulic boost system, rudder pedals, controls, mounting brackets, etc. Also includes the functioning and maintenance aspects of the flaps, spoilers, and other control surfaces, but does not include the structure which is covered in the Structures Chapters. Does not include rotorcraft rotor controls which are covered in the Rotor Chapter 65." ;
        rdfs:label       "FLIGHT CONTROLS" ;
        rdfs:subClassOf  rel:Component .

_:b93   rdf:type            owl:Restriction ;
        owl:onProperty      rel:hasComponent ;
        owl:someValuesFrom  ata:ata-27-70 .

ata:ata-27  rdfs:subClassOf  _:b93 .

_:b94   rdf:type            owl:Restriction ;
        owl:onProperty      rel:hasComponent ;
        owl:someValuesFrom  ata:ata-27-60 .

ata:ata-27  rdfs:subClassOf  _:b94 .

_:b95   rdf:type            owl:Restriction ;
        owl:onProperty      rel:hasComponent ;
        owl:someValuesFrom  ata:ata-27-10 .

ata:ata-27  rdfs:subClassOf  _:b95 .

_:b96   rdf:type            owl:Restriction ;
        owl:onProperty      rel:hasComponent ;
        owl:someValuesFrom  ata:ata-27-50 .

ata:ata-27  rdfs:subClassOf  _:b96 .

_:b97   rdf:type            owl:Restriction ;
        owl:onProperty      rel:hasComponent ;
        owl:someValuesFrom  ata:ata-27-80 .

ata:ata-27  rdfs:subClassOf  _:b97 .

_:b98   rdf:type            owl:Restriction ;
        owl:onProperty      rel:hasComponent ;
        owl:someValuesFrom  ata:ata-27-20 .

ata:ata-27  rdfs:subClassOf  _:b98 .

_:b99   rdf:type            owl:Restriction ;
        owl:onProperty      rel:hasComponent ;
        owl:someValuesFrom  ata:ata-27-40 .

ata:ata-27  rdfs:subClassOf  _:b99 .

_:b100  rdf:type            owl:Restriction ;
        owl:onProperty      rel:hasComponent ;
        owl:someValuesFrom  ata:ata-27-30 .

ata:ata-27  rdfs:subClassOf  _:b100 ;
        rel:hasComponent  ata:ata-27-40 ;
        rel:hasComponent  ata:ata-27-30 ;
        rel:hasComponent  ata:ata-27-20 ;
        rel:hasComponent  ata:ata-27-10 ;
        rel:hasComponent  ata:ata-27-70 ;
        rel:hasComponent  ata:ata-27-60 ;
        rel:hasComponent  ata:ata-27-80 ;
        rel:hasComponent  ata:ata-27-50 ;
        ata:has-id        "27" .

ata:ata-73  rdf:type     owl:Class ;
        rdfs:comment     "For turbine engines, those units and components and associated mechanical systems or electrical circuits which furnish or control fuel to the engine beyond the main fuel quick disconnect; and trust augmentor, fuel flow rate sensing, transmitting and/or indicating units whether the units are before or beyond the quick disconnect.\n\nIncludes coordinator of equivalent, engine driven fuel pump and filter assembly, main and thrust augmentor fuel controls, electronic temperature datum control, temerature datum valve, fuel manifold, fuel nozzles, fuel enrichment system, speed sensitivity switch, relay box assembly, solenoid drip valve, etc.\n\nFor reciprocating engines, those units and components which deliver metered fuel and air to the engine. The fuel portion includes the carburetor/master control from the inlet sideto the discharge nozzle(s), injection pumps, carburetor, injection nozzles, and fuel primer. The air portion includes units from the scoop inlet to the vapor return, and impeller chamber." ;
        rdfs:label       "ENGINE - FUEL AND CONTROL" ;
        rdfs:subClassOf  rel:Component .

_:b101  rdf:type            owl:Restriction ;
        owl:onProperty      rel:hasComponent ;
        owl:someValuesFrom  ata:ata-73-30 .

ata:ata-73  rdfs:subClassOf  _:b101 .

_:b102  rdf:type            owl:Restriction ;
        owl:onProperty      rel:hasComponent ;
        owl:someValuesFrom  ata:ata-73-20 .

ata:ata-73  rdfs:subClassOf  _:b102 .

_:b103  rdf:type            owl:Restriction ;
        owl:onProperty      rel:hasComponent ;
        owl:someValuesFrom  ata:ata-73-10 .

ata:ata-73  rdfs:subClassOf  _:b103 ;
        rel:hasComponent  ata:ata-73-20 ;
        rel:hasComponent  ata:ata-73-30 ;
        rel:hasComponent  ata:ata-73-10 ;
        ata:has-id        "73" .

ata:ata-49-80  rdf:type  owl:Class ;
        rdfs:comment     "For definitions see Chapter 78." ;
        rdfs:label       "EXHAUST" ;
        rdfs:subClassOf  rel:Component ;
        ata:has-id       "4980" .

ata:ata-23-10  rdf:type  owl:Class ;
        rdfs:comment     "That portion of the system which utilizes voice modulated electromagnetic waves to transmit and/or receive messages from air to air, or air to ground installations. Includes H.F., V.H.F., U.H.F, etc., inflight telephone, communication transmitting & receiving equipment." ;
        rdfs:label       "SPEECH COMMUNICATIONS" ;
        rdfs:subClassOf  rel:Component ;
        ata:has-id       "2310" .

ata:ata-28-30  rdf:type  owl:Class ;
        rdfs:comment     "That portion of the system which is used to dump fuel overboard during flight. Includes items such as plumbing, valves, controls, chutes, etc." ;
        rdfs:label       "DUMP" ;
        rdfs:subClassOf  rel:Component ;
        ata:has-id       "2830" .

ata:ata-41  rdf:type     owl:Class ;
        rdfs:comment     "Those units and components provided for the storage, balancing, control, filling, discharge, and dumping of water ballast. Does not include units or components covered in Chapter 38." ;
        rdfs:label       "WATER BALLAST" ;
        rdfs:subClassOf  rel:Component .

_:b104  rdf:type            owl:Restriction ;
        owl:onProperty      rel:hasComponent ;
        owl:someValuesFrom  ata:ata-41-30 .

ata:ata-41  rdfs:subClassOf  _:b104 .

_:b105  rdf:type            owl:Restriction ;
        owl:onProperty      rel:hasComponent ;
        owl:someValuesFrom  ata:ata-41-10 .

ata:ata-41  rdfs:subClassOf  _:b105 .

_:b106  rdf:type            owl:Restriction ;
        owl:onProperty      rel:hasComponent ;
        owl:someValuesFrom  ata:ata-41-20 .

ata:ata-41  rdfs:subClassOf  _:b106 ;
        rel:hasComponent  ata:ata-41-20 ;
        rel:hasComponent  ata:ata-41-10 ;
        rel:hasComponent  ata:ata-41-30 ;
        ata:has-id        "41" .

ata:ata-41-20  rdf:type  owl:Class ;
        rdfs:comment     "That portion of the system used to dump water ballast during flight. Includes valves, remote/direct, manual/automatic controls, etc." ;
        rdfs:label       "DUMP" ;
        rdfs:subClassOf  rel:Component ;
        ata:has-id       "4120" .

ata:group-aircraft  rdf:type  owl:Class ;
        rdfs:comment     "The complete operational unit. Includes dimensions and areas, lifting and shoring, leveling and weighing, towing and taxiing, parking and mooring, required placards, servicing." ;
        rdfs:label       "AIRCRAFT" ;
        rdfs:subClassOf  rel:Component ;
        ata:has-id       "group-aircraft" .

ata:ata-21-10  rdf:type  owl:Class ;
        rdfs:comment     "That portion of the system and its controls which supplies compressed air. Includes items such as controls and indicating systems related to the compressors, wiring, etc. Does not include the pressure control and indicating system for the cabin pressurization." ;
        rdfs:label       "COMPRESSION" ;
        rdfs:subClassOf  rel:Component ;
        ata:has-id       "2110" .

ata:ata-26-30  rdf:type  owl:Class ;
        rdfs:comment     "That portion of the system which is used to sense, indicate and extinguish a flame propagating into the fuel vent or scoop to prevent an explosion in the fuel system." ;
        rdfs:label       "EXPLOSION SUPPRESSION" ;
        rdfs:subClassOf  rel:Component ;
        ata:has-id       "2630" .

ata:ata-39-10  rdf:type  owl:Class ;
        rdfs:label       "INSTRUMENT AND CONTROL PANELS" ;
        rdfs:subClassOf  rel:Component ;
        ata:has-id       "3910" .

ata:ata-57-20  rdf:type  owl:Class ;
        rdfs:comment     "Wing Skins, primary structure, fillets, and fairings of the outer wing, and attach / attached fittings." ;
        rdfs:label       "OUTER" ;
        rdfs:subClassOf  rel:Component ;
        ata:has-id       "5720" .

ata:ata-24-30  rdf:type  owl:Class ;
        rdfs:comment     "That portion of the systems used to generate, regulate, control and indicate DC electrical power. Includes items such as generators/ alternators, transformers, rectifiers, batteries, control and regulating components, indicating systems, etc., all wiring to but not including main busses." ;
        rdfs:label       "DC GENERATION" ;
        rdfs:subClassOf  rel:Component ;
        ata:has-id       "2430" .

ata:ata-37-10  rdf:type  owl:Class ;
        rdfs:comment     "That portion of the system which is used to distribute negative pressure air to using systems." ;
        rdfs:label       "DISTRIBUTION" ;
        rdfs:subClassOf  rel:Component ;
        ata:has-id       "3710" .

ata:ata-54  rdf:type     owl:Class ;
        rdfs:comment     "Structural units and associated components and members which furnish a means of mounting and housing the power plant or rotor assembly. Includes skins, longerons, belt frames, stringers, clamshells, scuppers, doors, nacelle fillets, attach/attached fittings, etc. Also includes the structure of power plant cowling inclusive of the structural portion of the inlet whether or not integral with the aircraft. Structural portions of the exhaust system are excluded where they are not integral with the airframe." ;
        rdfs:label       "NACELLES / PYLONS" ;
        rdfs:subClassOf  rel:Component .

_:b107  rdf:type            owl:Restriction ;
        owl:onProperty      rel:hasComponent ;
        owl:someValuesFrom  ata:ata-54-90 .

ata:ata-54  rdfs:subClassOf  _:b107 .

_:b108  rdf:type            owl:Restriction ;
        owl:onProperty      rel:hasComponent ;
        owl:someValuesFrom  ata:ata-54-20 .

ata:ata-54  rdfs:subClassOf  _:b108 .

_:b109  rdf:type            owl:Restriction ;
        owl:onProperty      rel:hasComponent ;
        owl:someValuesFrom  ata:ata-54-40 .

ata:ata-54  rdfs:subClassOf  _:b109 .

_:b110  rdf:type            owl:Restriction ;
        owl:onProperty      rel:hasComponent ;
        owl:someValuesFrom  ata:ata-54-80 .

ata:ata-54  rdfs:subClassOf  _:b110 .

_:b111  rdf:type            owl:Restriction ;
        owl:onProperty      rel:hasComponent ;
        owl:someValuesFrom  ata:ata-54-70 .

ata:ata-54  rdfs:subClassOf  _:b111 .

_:b112  rdf:type            owl:Restriction ;
        owl:onProperty      rel:hasComponent ;
        owl:someValuesFrom  ata:ata-54-50 .

ata:ata-54  rdfs:subClassOf  _:b112 .

_:b113  rdf:type            owl:Restriction ;
        owl:onProperty      rel:hasComponent ;
        owl:someValuesFrom  ata:ata-54-10 .

ata:ata-54  rdfs:subClassOf  _:b113 .

_:b114  rdf:type            owl:Restriction ;
        owl:onProperty      rel:hasComponent ;
        owl:someValuesFrom  ata:ata-54-60 .

ata:ata-54  rdfs:subClassOf  _:b114 .

_:b115  rdf:type            owl:Restriction ;
        owl:onProperty      rel:hasComponent ;
        owl:someValuesFrom  ata:ata-54-30 .

ata:ata-54  rdfs:subClassOf  _:b115 ;
        rel:hasComponent  ata:ata-54-40 ;
        rel:hasComponent  ata:ata-54-50 ;
        rel:hasComponent  ata:ata-54-60 ;
        rel:hasComponent  ata:ata-54-20 ;
        rel:hasComponent  ata:ata-54-30 ;
        rel:hasComponent  ata:ata-54-90 ;
        rel:hasComponent  ata:ata-54-70 ;
        rel:hasComponent  ata:ata-54-10 ;
        rel:hasComponent  ata:ata-54-80 ;
        ata:has-id        "54" .

ata:ata-22  rdf:type     owl:Class ;
        rdfs:comment     "Those units and components which furnish a means of automatically controlling the flight of the aircraft. Includes those units and components which control direction, heading, attitude, altitude and speed." ;
        rdfs:label       "AUTO FLIGHT" ;
        rdfs:subClassOf  rel:Component .

_:b116  rdf:type            owl:Restriction ;
        owl:onProperty      rel:hasComponent ;
        owl:someValuesFrom  ata:ata-22-20 .

ata:ata-22  rdfs:subClassOf  _:b116 .

_:b117  rdf:type            owl:Restriction ;
        owl:onProperty      rel:hasComponent ;
        owl:someValuesFrom  ata:ata-22-10 .

ata:ata-22  rdfs:subClassOf  _:b117 .

_:b118  rdf:type            owl:Restriction ;
        owl:onProperty      rel:hasComponent ;
        owl:someValuesFrom  ata:ata-22-40 .

ata:ata-22  rdfs:subClassOf  _:b118 .

_:b119  rdf:type            owl:Restriction ;
        owl:onProperty      rel:hasComponent ;
        owl:someValuesFrom  ata:ata-22-30 .

ata:ata-22  rdfs:subClassOf  _:b119 .

_:b120  rdf:type            owl:Restriction ;
        owl:onProperty      rel:hasComponent ;
        owl:someValuesFrom  ata:ata-22-50 .

ata:ata-22  rdfs:subClassOf  _:b120 ;
        rel:hasComponent  ata:ata-22-50 ;
        rel:hasComponent  ata:ata-22-10 ;
        rel:hasComponent  ata:ata-22-40 ;
        rel:hasComponent  ata:ata-22-30 ;
        rel:hasComponent  ata:ata-22-20 ;
        ata:has-id        "22" .

ata:ata-55-20  rdf:type  owl:Class ;
        rdfs:comment     "Removable airfoil which is attached to the horizontal stabilizer or canard and used for pitch control. Includes items such as spars, ribs, stringers, skins, access covers, tabs, balance devices, attach/ attached fittings, etc." ;
        rdfs:label       "ELEVATOR - ELEVON" ;
        rdfs:subClassOf  rel:Component ;
        ata:has-id       "5520" .

ata:ata-22-30  rdf:type  owl:Class ;
        rdfs:comment     "That portion of the system that automatically controls the position of the throttles to properly manage engine power during all phases of flight/attitude. This includes engaging, sensing, computing, amplifying, controlling, actuating and warning devices such as amplifiers, computers, servos, limit switches, clutches, gear boxes, warning lights, etc." ;
        rdfs:label       "AUTO THROTTLE" ;
        rdfs:subClassOf  rel:Component ;
        ata:has-id       "2230" .

ata:ata-27-50  rdf:type  owl:Class ;
        rdfs:comment     "That portion of the systems which controls the position and movement of the trailing edge flaps. Includes items such as control handles, cables, actuators, warning systems, linkages, control surfaces, position indicators, etc." ;
        rdfs:label       "FLAPS" ;
        rdfs:subClassOf  rel:Component ;
        ata:has-id       "2750" .

ata:ata-35-10  rdf:type  owl:Class ;
        rdfs:comment     "That portion of the system which furnishes oxygen to the crew." ;
        rdfs:label       "CREW" ;
        rdfs:subClassOf  rel:Component ;
        ata:has-id       "3510" .

ata:ata-53-20  rdf:type  owl:Class ;
        rdfs:label       "AUXILIARY STRUCTURE" ;
        rdfs:subClassOf  rel:Component ;
        ata:has-id       "5320" .

ata:ata-25-50  rdf:type  owl:Class ;
        rdfs:comment     "Those compartments for storage of cargo and those components which are or can be mounted on the aircraft and used to load/unload, restrain, guide or service cargo. Includes drive systems, rollers, latches, restraint nets, etc." ;
        rdfs:label       "CARGO COMPARTMENTS" ;
        rdfs:subClassOf  rel:Component ;
        ata:has-id       "2550" .

ata:ata-33-10  rdf:type  owl:Class ;
        rdfs:comment     "The lighting sub-systems in the compartment above the floor and between the forward passenger partition and the forward pressure dome. Does not include cargo compartment. Includes direct and indirect illumination of work areas, panels, and instruments. Includes master warning light and warning light dimming systems, where not integrated with a central audio or visual system under 31-50." ;
        rdfs:label       "FLIGHT COMPARTMENT AND ANNUNCIATOR PANEL" ;
        rdfs:subClassOf  rel:Component ;
        ata:has-id       "3310" .

ata:ata-38-30  rdf:type  owl:Class ;
        rdfs:comment     "That portion of the system which is used for disposal of water and waste. Includes items such as wash basins, water closets, flushing systems, etc." ;
        rdfs:label       "WASTE DISPOSAL" ;
        rdfs:subClassOf  rel:Component ;
        ata:has-id       "3830" .

<http://onto.fel.cvut.cz/voc/ata-100/ata-72(T)-70>
        rdf:type         owl:Class ;
        rdfs:comment     "The section of the engine which by-passes a portion of the normal engine airflow (either ram or compressed air) for the prime purpose adding to engine trust of reducing specific fuel consumption." ;
        rdfs:label       "BY-PASS SECTION" ;
        rdfs:subClassOf  rel:Component ;
        ata:has-id       "72(T)70" .

ata:ata-71-30  rdf:type  owl:Class ;
        rdfs:comment     "Those fire-resistant partitions and seals mounted on or about the power package for the purpose of isolating areas subject to fire. Does not include those fire-walls which are included in Chapter 54." ;
        rdfs:label       "FIRESEALS AND SHROUDS" ;
        rdfs:subClassOf  rel:Component ;
        ata:has-id       "7130" .

ata:ata-67  rdf:type     owl:Class ;
        rdfs:comment     "The system which provides means of manually controlling the flight attitude of the helicopter. Includes items such as control linkage and control cables for collective pitch, cyclic pitch, directional control, servo-controls and corresponding system. The trim system and the indicating and monitoring system. NOTE: this chapter includes the complete rigging of rotor control including the associated items not described under this system, such as auto -pilot, servo -control unit, automatic trim (Ch. 22), blade pitch change rod (Ch. 63), swashplate." ;
        rdfs:label       "ROTORS FLIGHT CONTROL" ;
        rdfs:subClassOf  rel:Component .

_:b121  rdf:type            owl:Restriction ;
        owl:onProperty      rel:hasComponent ;
        owl:someValuesFrom  ata:ata-67-10 .

ata:ata-67  rdfs:subClassOf  _:b121 .

_:b122  rdf:type            owl:Restriction ;
        owl:onProperty      rel:hasComponent ;
        owl:someValuesFrom  ata:ata-67-20 .

ata:ata-67  rdfs:subClassOf  _:b122 .

_:b123  rdf:type            owl:Restriction ;
        owl:onProperty      rel:hasComponent ;
        owl:someValuesFrom  ata:ata-67-30 .

ata:ata-67  rdfs:subClassOf  _:b123 ;
        rel:hasComponent  ata:ata-67-30 ;
        rel:hasComponent  ata:ata-67-10 ;
        rel:hasComponent  ata:ata-67-20 ;
        ata:has-id        "67" .

ata:ata-84-10  rdf:type  owl:Class ;
        rdfs:comment     "Those units or components dedicated to jet assisted takeoff (JATO) systems." ;
        rdfs:label       "JET ASSISTED TAKEOFF" ;
        rdfs:subClassOf  rel:Component ;
        ata:has-id       "8410" .

ata:ata-51-20  rdf:type  owl:Class ;
        rdfs:comment     "Special processes for use in the repair of the airplane. Will not include general engineering practices unless specific deviations are required. Unique processes such as welding specifications, etc., relative to a single repair shall be incorporated in the repair and only referenced here." ;
        rdfs:label       "PROCESSES" ;
        rdfs:subClassOf  rel:Component ;
        ata:has-id       "5120" .

ata:group-airframe-systems
        rdf:type         owl:Class ;
        rdfs:comment     "All airframe systems except the Power Plant package." ;
        rdfs:label       "AIRFRAME SYSTEMS" ;
        rdfs:subClassOf  rel:Component .

_:b124  rdf:type            owl:Restriction ;
        owl:onProperty      rel:hasComponent ;
        owl:someValuesFrom  ata:ata-33 .

ata:group-airframe-systems
        rdfs:subClassOf  _:b124 .

_:b125  rdf:type            owl:Restriction ;
        owl:onProperty      rel:hasComponent ;
        owl:someValuesFrom  ata:ata-45 .

ata:group-airframe-systems
        rdfs:subClassOf  _:b125 .

_:b126  rdf:type            owl:Restriction ;
        owl:onProperty      rel:hasComponent ;
        owl:someValuesFrom  ata:ata-46 .

ata:group-airframe-systems
        rdfs:subClassOf  _:b126 .

_:b127  rdf:type            owl:Restriction ;
        owl:onProperty      rel:hasComponent ;
        owl:someValuesFrom  ata:ata-37 .

ata:group-airframe-systems
        rdfs:subClassOf  _:b127 .

_:b128  rdf:type            owl:Restriction ;
        owl:onProperty      rel:hasComponent ;
        owl:someValuesFrom  ata:ata-30 .

ata:group-airframe-systems
        rdfs:subClassOf  _:b128 .

_:b129  rdf:type            owl:Restriction ;
        owl:onProperty      rel:hasComponent ;
        owl:someValuesFrom  ata:ata-34 .

ata:group-airframe-systems
        rdfs:subClassOf  _:b129 .

_:b130  rdf:type            owl:Restriction ;
        owl:onProperty      rel:hasComponent ;
        owl:someValuesFrom  ata:ata-24 .

ata:group-airframe-systems
        rdfs:subClassOf  _:b130 .

_:b131  rdf:type            owl:Restriction ;
        owl:onProperty      rel:hasComponent ;
        owl:someValuesFrom  ata:ata-39 .

ata:group-airframe-systems
        rdfs:subClassOf  _:b131 .

_:b132  rdf:type            owl:Restriction ;
        owl:onProperty      rel:hasComponent ;
        owl:someValuesFrom  ata:ata-35 .

ata:group-airframe-systems
        rdfs:subClassOf  _:b132 .

_:b133  rdf:type            owl:Restriction ;
        owl:onProperty      rel:hasComponent ;
        owl:someValuesFrom  ata:ata-36 .

ata:group-airframe-systems
        rdfs:subClassOf  _:b133 .

_:b134  rdf:type            owl:Restriction ;
        owl:onProperty      rel:hasComponent ;
        owl:someValuesFrom  ata:ata-23 .

ata:group-airframe-systems
        rdfs:subClassOf  _:b134 .

_:b135  rdf:type            owl:Restriction ;
        owl:onProperty      rel:hasComponent ;
        owl:someValuesFrom  ata:ata-29 .

ata:group-airframe-systems
        rdfs:subClassOf  _:b135 .

_:b136  rdf:type            owl:Restriction ;
        owl:onProperty      rel:hasComponent ;
        owl:someValuesFrom  ata:ata-21 .

ata:group-airframe-systems
        rdfs:subClassOf  _:b136 .

_:b137  rdf:type            owl:Restriction ;
        owl:onProperty      rel:hasComponent ;
        owl:someValuesFrom  ata:ata-38 .

ata:group-airframe-systems
        rdfs:subClassOf  _:b137 .

_:b138  rdf:type            owl:Restriction ;
        owl:onProperty      rel:hasComponent ;
        owl:someValuesFrom  ata:ata-27 .

ata:group-airframe-systems
        rdfs:subClassOf  _:b138 .

_:b139  rdf:type            owl:Restriction ;
        owl:onProperty      rel:hasComponent ;
        owl:someValuesFrom  ata:ata-28 .

ata:group-airframe-systems
        rdfs:subClassOf  _:b139 .

_:b140  rdf:type            owl:Restriction ;
        owl:onProperty      rel:hasComponent ;
        owl:someValuesFrom  ata:ata-31 .

ata:group-airframe-systems
        rdfs:subClassOf  _:b140 .

_:b141  rdf:type            owl:Restriction ;
        owl:onProperty      rel:hasComponent ;
        owl:someValuesFrom  ata:ata-32 .

ata:group-airframe-systems
        rdfs:subClassOf  _:b141 .

_:b142  rdf:type            owl:Restriction ;
        owl:onProperty      rel:hasComponent ;
        owl:someValuesFrom  ata:ata-26 .

ata:group-airframe-systems
        rdfs:subClassOf  _:b142 .

_:b143  rdf:type            owl:Restriction ;
        owl:onProperty      rel:hasComponent ;
        owl:someValuesFrom  ata:ata-22 .

ata:group-airframe-systems
        rdfs:subClassOf  _:b143 .

_:b144  rdf:type            owl:Restriction ;
        owl:onProperty      rel:hasComponent ;
        owl:someValuesFrom  ata:ata-25 .

ata:group-airframe-systems
        rdfs:subClassOf  _:b144 .

_:b145  rdf:type            owl:Restriction ;
        owl:onProperty      rel:hasComponent ;
        owl:someValuesFrom  ata:ata-49 .

ata:group-airframe-systems
        rdfs:subClassOf  _:b145 .

_:b146  rdf:type            owl:Restriction ;
        owl:onProperty      rel:hasComponent ;
        owl:someValuesFrom  ata:ata-41 .

ata:group-airframe-systems
        rdfs:subClassOf   _:b146 ;
        rel:hasComponent  ata:ata-23 ;
        rel:hasComponent  ata:ata-49 ;
        rel:hasComponent  ata:ata-35 ;
        rel:hasComponent  ata:ata-26 ;
        rel:hasComponent  ata:ata-31 ;
        rel:hasComponent  ata:ata-22 ;
        rel:hasComponent  ata:ata-38 ;
        rel:hasComponent  ata:ata-29 ;
        rel:hasComponent  ata:ata-24 ;
        rel:hasComponent  ata:ata-36 ;
        rel:hasComponent  ata:ata-27 ;
        rel:hasComponent  ata:ata-39 ;
        rel:hasComponent  ata:ata-32 ;
        rel:hasComponent  ata:ata-45 ;
        rel:hasComponent  ata:ata-41 ;
        rel:hasComponent  ata:ata-28 ;
        rel:hasComponent  ata:ata-34 ;
        rel:hasComponent  ata:ata-25 ;
        rel:hasComponent  ata:ata-30 ;
        rel:hasComponent  ata:ata-37 ;
        rel:hasComponent  ata:ata-21 ;
        rel:hasComponent  ata:ata-46 ;
        rel:hasComponent  ata:ata-33 ;
        ata:has-id        "group-airframe-systems" .

ata:ata-56-40  rdf:type  owl:Class ;
        rdfs:comment     "Windows used for examining compartments and equipment in and about the airplane, and astrodomes used for celestial navigation. Includes items such as transparent material, its frame, etc." ;
        rdfs:label       "INSPECTION AND OBSERVATION" ;
        rdfs:subClassOf  rel:Component ;
        ata:has-id       "5640" .

ata:ata-35  rdf:type     owl:Class ;
        rdfs:comment     "Those units and components which store, regulate, and deliver oxygen to the passengers and crew, including bottles, relief valves, shut-off valves, outlets, regulators, masks, walk -around bottles, etc." ;
        rdfs:label       "OXYGEN" ;
        rdfs:subClassOf  rel:Component .

_:b147  rdf:type            owl:Restriction ;
        owl:onProperty      rel:hasComponent ;
        owl:someValuesFrom  ata:ata-35-10 .

ata:ata-35  rdfs:subClassOf  _:b147 .

_:b148  rdf:type            owl:Restriction ;
        owl:onProperty      rel:hasComponent ;
        owl:someValuesFrom  ata:ata-35-20 .

ata:ata-35  rdfs:subClassOf  _:b148 .

_:b149  rdf:type            owl:Restriction ;
        owl:onProperty      rel:hasComponent ;
        owl:someValuesFrom  ata:ata-35-30 .

ata:ata-35  rdfs:subClassOf  _:b149 ;
        rel:hasComponent  ata:ata-35-30 ;
        rel:hasComponent  ata:ata-35-20 ;
        rel:hasComponent  ata:ata-35-10 ;
        ata:has-id        "35" .

ata:ata-23-50  rdf:type  owl:Class ;
        rdfs:comment     "That portion of the system which controls the output of the communications and navigation receivers into the flight crew headphones and speakers and the output of the flight crew microphones into the communications transmitters. Includes items such as audio selector control panel, micro-phones, headphones, cockpit loudspeakers, etc." ;
        rdfs:label       "AUDIO INTEGRATING" ;
        rdfs:subClassOf  rel:Component ;
        ata:has-id       "2350" .

ata:ata-31-10  rdf:type  owl:Class ;
        rdfs:comment     "Coverage of all panels fixed or movable with their replaceable components such as instruments, switches, circuit breakers, fuses, etc. Also includes general coverage of instrument panel vibrators and other panel accessories." ;
        rdfs:label       "INSTRUMENT AND CONTROL PANELS" ;
        rdfs:subClassOf  rel:Component ;
        ata:has-id       "3110" .

ata:ata-81  rdf:type     owl:Class ;
        rdfs:comment     "For reciprocating engines only. Includes power recovery turbine assembly and turbo-supercharger unit when external to the engine." ;
        rdfs:label       "TURBINES (RECIPROCATING ENGINES)" ;
        rdfs:subClassOf  rel:Component .

_:b150  rdf:type            owl:Restriction ;
        owl:onProperty      rel:hasComponent ;
        owl:someValuesFrom  ata:ata-81-20 .

ata:ata-81  rdfs:subClassOf  _:b150 .

_:b151  rdf:type            owl:Restriction ;
        owl:onProperty      rel:hasComponent ;
        owl:someValuesFrom  ata:ata-81-10 .

ata:ata-81  rdfs:subClassOf  _:b151 ;
        rel:hasComponent  ata:ata-81-20 ;
        rel:hasComponent  ata:ata-81-10 ;
        ata:has-id        "81" .

ata:ata-49-10  rdf:type  owl:Class ;
        rdfs:comment     "For definitions see Chapter 71." ;
        rdfs:label       "POWER PLANT" ;
        rdfs:subClassOf  rel:Component ;
        ata:has-id       "4910" .

ata:ata-82-10  rdf:type  owl:Class ;
        rdfs:comment     "That portion of the system which is used to for the storage of water or water mixtures. Includes tank sealing, attachment of bladder type cells, ventilating system, cell and tank interconnects, filling systems, etc." ;
        rdfs:label       "STORAGE" ;
        rdfs:subClassOf  rel:Component ;
        ata:has-id       "8210" .

ata:ata-54-40  rdf:type  owl:Class ;
        rdfs:label       "[AS REQUIRED]" ;
        rdfs:subClassOf  rel:Component ;
        ata:has-id       "5440" .

ata:ata-67-20  rdf:type  owl:Class ;
        rdfs:comment     "That portion of the controls which control the direction of the helicopter (yaw control). Includes items such as tail rotor control pedals, relevant linkage and cable controls, bellcranks constituting the yaw control channel and the control position indicating system." ;
        rdfs:label       "ANTI-TORQUE ROTOR CONTROL (YAW CONTROL)" ;
        rdfs:subClassOf  rel:Component ;
        ata:has-id       "6720" .

ata:ata-21-50  rdf:type  owl:Class ;
        rdfs:comment     "That portion of the system and its controls which supply cooled air. Includes items such as the cooling unit, indicating systems related to the cooler operation, wiring, etc. Does not include temperature control and indicating systems." ;
        rdfs:label       "COOLING" ;
        rdfs:subClassOf  rel:Component ;
        ata:has-id       "2150" .

ata:ata-34-30  rdf:type  owl:Class ;
        rdfs:comment     "That portion of the system which provides guidance during approach, landing and taxiing. Includes items such as localizer, glide slope, ILS, markers, paravisual director ground guidance systems, etc." ;
        rdfs:label       "LANDING AND TAXIING AIDS" ;
        rdfs:subClassOf  rel:Component ;
        ata:has-id       "3430" .

ata:ata-39-50  rdf:type  owl:Class ;
        rdfs:label       "INTEGRATED CIRCUITS" ;
        rdfs:subClassOf  rel:Component ;
        ata:has-id       "3950" .

<http://onto.fel.cvut.cz/voc/ata-100/ata-72(R)-40>
        rdf:type         owl:Class ;
        rdfs:comment     "The section of the engine which contains the cases, shroud plates, PRT coupling and gearing, impeller and drives, accessory drives, bushings, etc." ;
        rdfs:label       "SUPERCHARGER SECTION" ;
        rdfs:subClassOf  rel:Component ;
        ata:has-id       "72(R)40" .

ata:ata-80-10  rdf:type  owl:Class ;
        rdfs:comment     "That portion of the system which is used to perform the cranking portion of the starting operation. Includes items such as plumbing, valves, wiring, starters, switches, relays, etc." ;
        rdfs:label       "CRANKING" ;
        rdfs:subClassOf  rel:Component ;
        ata:has-id       "8010" .

ata:ata-52-40  rdf:type  owl:Class ;
        rdfs:comment     "Exterior doors used primarily to gain access for servicing aircraft systems and equipment. Includes items such as structure, latching mechanisms, handles, insulation, lining, controls, integral steps, handrails, attach/attached fittings, etc." ;
        rdfs:label       "SERVICE" ;
        rdfs:subClassOf  rel:Component ;
        ata:has-id       "5240" .

ata:ata-57-60  rdf:type  owl:Class ;
        rdfs:comment     "Skins and structure of wing-mounted spoilers, airbrakes, lift dumpers, attach/attached fittings, etc." ;
        rdfs:label       "AILERONS AND ELEVONS" ;
        rdfs:subClassOf  rel:Component ;
        ata:has-id       "5760" .

ata:ata-65-20  rdf:type  owl:Class ;
        rdfs:comment     "Intermediate gearbox. Tail gearbox." ;
        rdfs:label       "GEARBOXES" ;
        rdfs:subClassOf  rel:Component ;
        ata:has-id       "6520" .

ata:ata-32-30  rdf:type  owl:Class ;
        rdfs:comment     "That portion of the system which is used to extend and retract the landing gear and open and close the landing gear doors. Includes items such as actuating mechanisms, bogie trim, bungees, up and down latches, operating controls, valves and motors, cables, wiring, plumbing, etc." ;
        rdfs:label       "EXTENSION AND RETRACTION" ;
        rdfs:subClassOf  rel:Component ;
        ata:has-id       "3230" .

<http://onto.fel.cvut.cz/voc/ata-100/ata-72(R)>
        rdf:type         owl:Class ;
        rdfs:label       "ENGINE - RECIPROCATING" ;
        rdfs:subClassOf  rel:Component .

_:b152  rdf:type            owl:Restriction ;
        owl:onProperty      rel:hasComponent ;
        owl:someValuesFrom  <http://onto.fel.cvut.cz/voc/ata-100/ata-72(R)-30> .

<http://onto.fel.cvut.cz/voc/ata-100/ata-72(R)>
        rdfs:subClassOf  _:b152 .

_:b153  rdf:type            owl:Restriction ;
        owl:onProperty      rel:hasComponent ;
        owl:someValuesFrom  <http://onto.fel.cvut.cz/voc/ata-100/ata-72(R)-10> .

<http://onto.fel.cvut.cz/voc/ata-100/ata-72(R)>
        rdfs:subClassOf  _:b153 .

_:b154  rdf:type            owl:Restriction ;
        owl:onProperty      rel:hasComponent ;
        owl:someValuesFrom  <http://onto.fel.cvut.cz/voc/ata-100/ata-72(R)-50> .

<http://onto.fel.cvut.cz/voc/ata-100/ata-72(R)>
        rdfs:subClassOf  _:b154 .

_:b155  rdf:type            owl:Restriction ;
        owl:onProperty      rel:hasComponent ;
        owl:someValuesFrom  <http://onto.fel.cvut.cz/voc/ata-100/ata-72(R)-40> .

<http://onto.fel.cvut.cz/voc/ata-100/ata-72(R)>
        rdfs:subClassOf  _:b155 .

_:b156  rdf:type            owl:Restriction ;
        owl:onProperty      rel:hasComponent ;
        owl:someValuesFrom  <http://onto.fel.cvut.cz/voc/ata-100/ata-72(R)-20> .

<http://onto.fel.cvut.cz/voc/ata-100/ata-72(R)>
        rdfs:subClassOf   _:b156 ;
        rel:hasComponent  <http://onto.fel.cvut.cz/voc/ata-100/ata-72(R)-10> ;
        rel:hasComponent  <http://onto.fel.cvut.cz/voc/ata-100/ata-72(R)-50> ;
        rel:hasComponent  <http://onto.fel.cvut.cz/voc/ata-100/ata-72(R)-40> ;
        rel:hasComponent  <http://onto.fel.cvut.cz/voc/ata-100/ata-72(R)-20> ;
        rel:hasComponent  <http://onto.fel.cvut.cz/voc/ata-100/ata-72(R)-30> ;
        ata:has-id        "72(R)" .

_:b157  rdf:type            owl:Restriction ;
        owl:onProperty      rel:hasComponent ;
        owl:someValuesFrom  ata:ata-72 .

ata:ata-62  rdf:type     owl:Class ;
        rdfs:comment     "Rotor head assembly(ies) and rotor blades, including the swashplate assembly(ies) and the rotor shaft unit(s) if not an integral part of the gear box(es). Does not include the rotor anti-icing system which is dealt with in chapter 30 \"Ice and Rain Protection\"." ;
        rdfs:label       "MAIN ROTOR(S)" ;
        rdfs:subClassOf  rel:Component .

_:b158  rdf:type            owl:Restriction ;
        owl:onProperty      rel:hasComponent ;
        owl:someValuesFrom  ata:ata-62-20 .

ata:ata-62  rdfs:subClassOf  _:b158 .

_:b159  rdf:type            owl:Restriction ;
        owl:onProperty      rel:hasComponent ;
        owl:someValuesFrom  ata:ata-62-10 .

ata:ata-62  rdfs:subClassOf  _:b159 .

_:b160  rdf:type            owl:Restriction ;
        owl:onProperty      rel:hasComponent ;
        owl:someValuesFrom  ata:ata-62-30 .

ata:ata-62  rdfs:subClassOf  _:b160 .

_:b161  rdf:type            owl:Restriction ;
        owl:onProperty      rel:hasComponent ;
        owl:someValuesFrom  ata:ata-62-40 .

ata:ata-62  rdfs:subClassOf  _:b161 ;
        rel:hasComponent  ata:ata-62-40 ;
        rel:hasComponent  ata:ata-62-20 ;
        rel:hasComponent  ata:ata-62-30 ;
        rel:hasComponent  ata:ata-62-10 ;
        ata:has-id        "62" .

ata:ata-30  rdf:type     owl:Class ;
        rdfs:comment     "Those units and components which provide a means of preventing or disposing of formation of ice and rain on various parts of the aircraft. Includes alcohol pump, valves, tanks, propeller / rotor anti-icing system, wing heaters, water line heaters, pitot heaters, scoop heaters, windshield wipers and the electrical and heated air portion of windshield ice control. Does not include the basic windshield panel. For turbine type power plants using air as the anti-icing medium, engine anti-icing is contained under Air System." ;
        rdfs:label       "ICE AND RAIN PROTECTION" ;
        rdfs:subClassOf  rel:Component .

_:b162  rdf:type            owl:Restriction ;
        owl:onProperty      rel:hasComponent ;
        owl:someValuesFrom  ata:ata-30-30 .

ata:ata-30  rdfs:subClassOf  _:b162 .

_:b163  rdf:type            owl:Restriction ;
        owl:onProperty      rel:hasComponent ;
        owl:someValuesFrom  ata:ata-30-80 .

ata:ata-30  rdfs:subClassOf  _:b163 .

_:b164  rdf:type            owl:Restriction ;
        owl:onProperty      rel:hasComponent ;
        owl:someValuesFrom  ata:ata-30-70 .

ata:ata-30  rdfs:subClassOf  _:b164 .

_:b165  rdf:type            owl:Restriction ;
        owl:onProperty      rel:hasComponent ;
        owl:someValuesFrom  ata:ata-30-40 .

ata:ata-30  rdfs:subClassOf  _:b165 .

_:b166  rdf:type            owl:Restriction ;
        owl:onProperty      rel:hasComponent ;
        owl:someValuesFrom  ata:ata-30-20 .

ata:ata-30  rdfs:subClassOf  _:b166 .

_:b167  rdf:type            owl:Restriction ;
        owl:onProperty      rel:hasComponent ;
        owl:someValuesFrom  ata:ata-30-10 .

ata:ata-30  rdfs:subClassOf  _:b167 .

_:b168  rdf:type            owl:Restriction ;
        owl:onProperty      rel:hasComponent ;
        owl:someValuesFrom  ata:ata-30-50 .

ata:ata-30  rdfs:subClassOf  _:b168 .

_:b169  rdf:type            owl:Restriction ;
        owl:onProperty      rel:hasComponent ;
        owl:someValuesFrom  ata:ata-30-60 .

ata:ata-30  rdfs:subClassOf  _:b169 ;
        rel:hasComponent  ata:ata-30-20 ;
        rel:hasComponent  ata:ata-30-60 ;
        rel:hasComponent  ata:ata-30-30 ;
        rel:hasComponent  ata:ata-30-70 ;
        rel:hasComponent  ata:ata-30-40 ;
        rel:hasComponent  ata:ata-30-10 ;
        rel:hasComponent  ata:ata-30-80 ;
        rel:hasComponent  ata:ata-30-50 ;
        ata:has-id        "30" .

ata:ata-63-20  rdf:type  owl:Class ;
        rdfs:comment     "Part of the system driving the rotor(s). Includes the mechanical power take -off(s) and accessory drives but does not include the accessories themselves (alternators, hydraulic pumps, etc.). Includes the G.B. lubricating system(s) and the rotor brake(s) if the latter form(s) part of the G.B.(s)." ;
        rdfs:label       "GEARBOX(ES)" ;
        rdfs:subClassOf  rel:Component ;
        ata:has-id       "6320" .

ata:ata-30-30  rdf:type  owl:Class ;
        rdfs:comment     "That portion of the system which is used to eliminate or prevent the formation of ice on the pitot and static systems." ;
        rdfs:label       "PITOT AND STATIC" ;
        rdfs:subClassOf  rel:Component ;
        ata:has-id       "3030" .

ata:ata-53-60  rdf:type  owl:Class ;
        rdfs:label       "[AS REQUIRED]" ;
        rdfs:subClassOf  rel:Component ;
        ata:has-id       "5360" .

ata:ata-61-20  rdf:type  owl:Class ;
        rdfs:comment     "That portion of the system which controls the pitch of the propeller blades. Includes items such as governor synchronizers, switches, wiring, cables, levers, etc. Does not include any parts which rotate with the propeller assembly. Also includes all those units and components provided for the propulsor vector drive system. Includes flight deck control, drive motors, gearboxes, drive shafts, synchronizing shafts, etc." ;
        rdfs:label       "CONTROLLING" ;
        rdfs:subClassOf  rel:Component ;
        ata:has-id       "6120" .

ata:ata-79-20  rdf:type  owl:Class ;
        rdfs:comment     "That portion of the system which is used to conduct oil to and from the engine. Includes items such as plumbing, valves, temperature regulator, control systems, etc." ;
        rdfs:label       "DISTRIBUTION" ;
        rdfs:subClassOf  rel:Component ;
        ata:has-id       "7920" .

ata:ata-33-50  rdf:type  owl:Class ;
        rdfs:comment     "The separate and independent sub-system used to provide illumination in case of primary electrical power failure. Includes items such as inertia flashlights, lanterns, etc." ;
        rdfs:label       "EMERGENCY LIGHTING" ;
        rdfs:subClassOf  rel:Component ;
        ata:has-id       "3350" .

ata:ata-46-30  rdf:type  owl:Class ;
        rdfs:comment     "That portion of the onboard flight information system that supports all onboard maintenance system functions, maintenance technicians, and any ground based maintenance activity." ;
        rdfs:label       "MAINTENANCE INFORMATION SYSTEMS" ;
        rdfs:subClassOf  rel:Component ;
        ata:has-id       "4630" .

ata:ata-71-70  rdf:type  owl:Class ;
        rdfs:comment     "Those components and manifold assemblies which are used to drain off excess fluids from the power plant and its accessories. Includes drainlines, manifolds, tanks, flame arrestors, vents, and their supporting brackets, etc. Also includes components that are an integral part of, or fitted to the power plant cowling." ;
        rdfs:label       "ENGINE DRAINS" ;
        rdfs:subClassOf  rel:Component ;
        ata:has-id       "7170" .

ata:ata-29  rdf:type     owl:Class ;
        rdfs:comment     "Those units and components which furnish hydraulic fluid under pressure (includes pumps, regulators, lines, valves, etc.) to a common point (manifold) for redistribution to other defined systems." ;
        rdfs:label       "HYDRAULIC POWER" ;
        rdfs:subClassOf  rel:Component .

_:b170  rdf:type            owl:Restriction ;
        owl:onProperty      rel:hasComponent ;
        owl:someValuesFrom  ata:ata-29-20 .

ata:ata-29  rdfs:subClassOf  _:b170 .

_:b171  rdf:type            owl:Restriction ;
        owl:onProperty      rel:hasComponent ;
        owl:someValuesFrom  ata:ata-29-30 .

ata:ata-29  rdfs:subClassOf  _:b171 .

_:b172  rdf:type            owl:Restriction ;
        owl:onProperty      rel:hasComponent ;
        owl:someValuesFrom  ata:ata-29-10 .

ata:ata-29  rdfs:subClassOf  _:b172 ;
        rel:hasComponent  ata:ata-29-20 ;
        rel:hasComponent  ata:ata-29-30 ;
        rel:hasComponent  ata:ata-29-10 ;
        ata:has-id        "29" .

ata:ata-51-60  rdf:type  owl:Class ;
        rdfs:comment     "Procedures for adjusting the mass balance of control surfaces after repair. Where applicable, individual repairs will contain their own balancing instructions." ;
        rdfs:label       "CONTROL-SURFACE BALANCING" ;
        rdfs:subClassOf  rel:Component ;
        ata:has-id       "5160" .

ata:ata-75  rdf:type     owl:Class ;
        rdfs:comment     "For turbine engines, those external units and components and integral basic engine parts which go together to conduct air to the extension shaft and torquemeter, assembly, if any. Includes compressor bleed systems used to control flow of air through the engine, cooling air systems and heated air systems for engine anti-icing. Does not include aircraft anti-icing, engine starting systems, nor exhaust supplementary air systems." ;
        rdfs:label       "BLEED AIR" ;
        rdfs:subClassOf  rel:Component .

_:b173  rdf:type            owl:Restriction ;
        owl:onProperty      rel:hasComponent ;
        owl:someValuesFrom  ata:ata-75-30 .

ata:ata-75  rdfs:subClassOf  _:b173 .

_:b174  rdf:type            owl:Restriction ;
        owl:onProperty      rel:hasComponent ;
        owl:someValuesFrom  ata:ata-75-10 .

ata:ata-75  rdfs:subClassOf  _:b174 .

_:b175  rdf:type            owl:Restriction ;
        owl:onProperty      rel:hasComponent ;
        owl:someValuesFrom  ata:ata-75-20 .

ata:ata-75  rdfs:subClassOf  _:b175 .

_:b176  rdf:type            owl:Restriction ;
        owl:onProperty      rel:hasComponent ;
        owl:someValuesFrom  ata:ata-75-40 .

ata:ata-75  rdfs:subClassOf  _:b176 ;
        rel:hasComponent  ata:ata-75-30 ;
        rel:hasComponent  ata:ata-75-20 ;
        rel:hasComponent  ata:ata-75-10 ;
        rel:hasComponent  ata:ata-75-40 ;
        ata:has-id        "75" .

ata:ata-64-40  rdf:type  owl:Class ;
        rdfs:comment     "That portion of the system which indicates operation or activation of rotor systems. Includes items such as lights, gauges, switches, wiring, etc. Note: For an integral unit, only one section will be used." ;
        rdfs:label       "INDICATING" ;
        rdfs:subClassOf  rel:Component ;
        ata:has-id       "6440" .

ata:ata-77-20  rdf:type  owl:Class ;
        rdfs:comment     "That portion of the system which indicates temperatures in the engine. Includes items such as cylinder head, exhaust (turbine inlet), etc." ;
        rdfs:label       "TEMPERATURE" ;
        rdfs:subClassOf  rel:Component ;
        ata:has-id       "7720" .

ata:ata-31-50  rdf:type  owl:Class ;
        rdfs:comment     "Those systems and components which give audible or visual warning of conditions in unrelated systems. Includes items such as master warning or flight warning systems, central instrument warning, or caution and warning systems, tone generators, annunciators, etc." ;
        rdfs:label       "CENTRAL WARNING SYSTEMS" ;
        rdfs:subClassOf  rel:Component ;
        ata:has-id       "3150" .

_:b177  rdf:type            owl:Restriction ;
        owl:onProperty      rel:hasComponent ;
        owl:someValuesFrom  ata:ata-91 .

ata:ata-49-50  rdf:type  owl:Class ;
        rdfs:comment     "For definitions see Chapter 75." ;
        rdfs:label       "AIR" ;
        rdfs:subClassOf  rel:Component ;
        ata:has-id       "4950" .

ata:ata-54-80  rdf:type  owl:Class ;
        rdfs:label       "[AS REQUIRED]" ;
        rdfs:subClassOf  rel:Component ;
        ata:has-id       "5480" .

ata:ata-62-40  rdf:type  owl:Class ;
        rdfs:comment     "That portion of the system which indicates operation or activation of rotor systems. Includes items such as lights, gauges, switches, wiring, etc." ;
        rdfs:label       "INDICATING" ;
        rdfs:subClassOf  rel:Component ;
        ata:has-id       "6240" .

ata:ata-75-20  rdf:type  owl:Class ;
        rdfs:comment     "That portion of the system which is used to ventilate the engine and accessories. Includes items such as valves, plumbing, wiring, jet pumps, vortex spoilers, etc." ;
        rdfs:label       "ENGINE COOLING" ;
        rdfs:subClassOf  rel:Component ;
        ata:has-id       "7520" .

ata:ata-52-80  rdf:type  owl:Class ;
        rdfs:comment     "Structure of the doors used to enclose the landing gear compartments. Includes items such as structure, latching mechanisms, handles, insulation, lining, controls, attach/attached fittings, etc." ;
        rdfs:label       "LANDING GEAR" ;
        rdfs:subClassOf  rel:Component ;
        ata:has-id       "5280" .

ata:ata-32-70  rdf:type  owl:Class ;
        rdfs:comment     "Devices used to stabilize the aircraft while on the ground and prevent damage by ground contact. Includes items such as shock strut, skid block, wheels, etc." ;
        rdfs:label       "SUPPLEMENTARY GEAR - SKIS, FLOATS" ;
        rdfs:subClassOf  rel:Component ;
        ata:has-id       "3270" .

ata:ata-73-20  rdf:type  owl:Class ;
        rdfs:comment     "The main fuel control which meters fuel to the engine and the thrust augmentor. Includes items such as hydro-mechanical or electronic fuel control, levers, actuators, cables, pulleys, linkages, sensors, valves, etc. which are components of the fuel control units." ;
        rdfs:label       "CONTROLLING - GOVERNING" ;
        rdfs:subClassOf  rel:Component ;
        ata:has-id       "7320" .

ata:ata-78-40  rdf:type  owl:Class ;
        rdfs:comment     "That portion of the system which varies and controls supplementary air flow of the exhaust system. Includes items such as tertiary doors, actuators, linkages, springs, plumbing, wiring, position indicators, warning systems, etc." ;
        rdfs:label       "SUPPLEMENTAL AIR" ;
        rdfs:subClassOf  rel:Component ;
        ata:has-id       "7840" .

ata:ata-45-50  rdf:type  owl:Class ;
        rdfs:comment     "Central Maintenance System interfaces with Structures, and identification of maintenance functions related to Structures." ;
        rdfs:label       "CMS / STRUCTURES" ;
        rdfs:subClassOf  rel:Component ;
        ata:has-id       "4550" .

ata:ata-29-20  rdf:type  owl:Class ;
        rdfs:comment     "That portion of the system which is classified as auxiliary, emergency or standby, and which is used to supplement or take the place of the main hydraulic system. Includes items such as tanks and accumulators which are separate from the main system, hand pumps, auxiliary pumps, valves, plumbing, wiring, etc." ;
        rdfs:label       "AUXILIARY" ;
        rdfs:subClassOf  rel:Component ;
        ata:has-id       "2920" .

ata:ata-56  rdf:type     owl:Class ;
        rdfs:comment     "Fuselage and crew compartment windows inclusive of windshield; also those windows installed in doors." ;
        rdfs:label       "WINDOWS" ;
        rdfs:subClassOf  rel:Component .

_:b178  rdf:type            owl:Restriction ;
        owl:onProperty      rel:hasComponent ;
        owl:someValuesFrom  ata:ata-56-20 .

ata:ata-56  rdfs:subClassOf  _:b178 .

_:b179  rdf:type            owl:Restriction ;
        owl:onProperty      rel:hasComponent ;
        owl:someValuesFrom  ata:ata-56-10 .

ata:ata-56  rdfs:subClassOf  _:b179 .

_:b180  rdf:type            owl:Restriction ;
        owl:onProperty      rel:hasComponent ;
        owl:someValuesFrom  ata:ata-56-30 .

ata:ata-56  rdfs:subClassOf  _:b180 .

_:b181  rdf:type            owl:Restriction ;
        owl:onProperty      rel:hasComponent ;
        owl:someValuesFrom  ata:ata-56-40 .

ata:ata-56  rdfs:subClassOf  _:b181 ;
        rel:hasComponent  ata:ata-56-40 ;
        rel:hasComponent  ata:ata-56-20 ;
        rel:hasComponent  ata:ata-56-30 ;
        rel:hasComponent  ata:ata-56-10 ;
        ata:has-id        "56" .

ata:ata-24  rdf:type     owl:Class ;
        rdfs:comment     "Those electrical units and components which generate, control and supply AC and/or DC electrical power for other systems, including generators and relays, inverters, batteries, etc., through the secondary busses. Also includes common electrical items such as wiring, switches, connectors, etc." ;
        rdfs:label       "ELECTRICAL POWER" ;
        rdfs:subClassOf  rel:Component .

_:b182  rdf:type            owl:Restriction ;
        owl:onProperty      rel:hasComponent ;
        owl:someValuesFrom  ata:ata-24-30 .

ata:ata-24  rdfs:subClassOf  _:b182 .

_:b183  rdf:type            owl:Restriction ;
        owl:onProperty      rel:hasComponent ;
        owl:someValuesFrom  ata:ata-24-60 .

ata:ata-24  rdfs:subClassOf  _:b183 .

_:b184  rdf:type            owl:Restriction ;
        owl:onProperty      rel:hasComponent ;
        owl:someValuesFrom  ata:ata-24-20 .

ata:ata-24  rdfs:subClassOf  _:b184 .

_:b185  rdf:type            owl:Restriction ;
        owl:onProperty      rel:hasComponent ;
        owl:someValuesFrom  ata:ata-24-50 .

ata:ata-24  rdfs:subClassOf  _:b185 .

_:b186  rdf:type            owl:Restriction ;
        owl:onProperty      rel:hasComponent ;
        owl:someValuesFrom  ata:ata-24-40 .

ata:ata-24  rdfs:subClassOf  _:b186 .

_:b187  rdf:type            owl:Restriction ;
        owl:onProperty      rel:hasComponent ;
        owl:someValuesFrom  ata:ata-24-10 .

ata:ata-24  rdfs:subClassOf  _:b187 ;
        rel:hasComponent  ata:ata-24-40 ;
        rel:hasComponent  ata:ata-24-20 ;
        rel:hasComponent  ata:ata-24-60 ;
        rel:hasComponent  ata:ata-24-50 ;
        rel:hasComponent  ata:ata-24-30 ;
        rel:hasComponent  ata:ata-24-10 ;
        ata:has-id        "24" .

ata:ata-70  rdf:type     owl:Class ;
        rdfs:label       "STANDARD PRACTICES - ENGINE" ;
        rdfs:subClassOf  rel:Component ;
        ata:has-id       "70" .

ata:ata-30-70  rdf:type  owl:Class ;
        rdfs:comment     "That portion of the system which is used to prevent the formation of ice in water supply and drain lines." ;
        rdfs:label       "WATER LINES" ;
        rdfs:subClassOf  rel:Component ;
        ata:has-id       "3070" .

ata:ata-27-20  rdf:type  owl:Class ;
        rdfs:comment     "That portion of the systems which controls the position and movement of the rudder / ruddevator and rudder tabs. Includes items such as the rudder pedals, tab control wheel, cables, boosters, linkages, control surfaces, position indicators, etc." ;
        rdfs:label       "RUDDER / RUDDEVATOR AND TAB" ;
        rdfs:subClassOf  rel:Component ;
        ata:has-id       "2720" .

ata:ata-25-20  rdf:type  owl:Class ;
        rdfs:comment     "The areas in which the passengers are seated. Includes lounges but not dressing rooms. Includes items such as seats, berths, overhead storage compartments, curtains, wall coverings, carpets, magazine racks, wardrobes, movable partitions, wall type thermometers, spare bulbs, fuses, etc." ;
        rdfs:label       "PASSENGER COMPARTMENT" ;
        rdfs:subClassOf  rel:Component ;
        ata:has-id       "2520" .

<http://onto.fel.cvut.cz/voc/ata-100/ata-72(T)-40>
        rdf:type         owl:Class ;
        rdfs:comment     "The section of the engine in which the air and fuel are combined and burned. Includes items such as burner cans, cases, etc." ;
        rdfs:label       "COMBUSTION SECTION" ;
        rdfs:subClassOf  rel:Component ;
        ata:has-id       "72(T)40" .

ata:ata-37  rdf:type     owl:Class ;
        rdfs:comment     "Those units and components used to generate, deliver and regulate negative air pressure, including pumps, regulators, lines, etc., through and including the manifold." ;
        rdfs:label       "VACUUM" ;
        rdfs:subClassOf  rel:Component .

_:b188  rdf:type            owl:Restriction ;
        owl:onProperty      rel:hasComponent ;
        owl:someValuesFrom  ata:ata-37-20 .

ata:ata-37  rdfs:subClassOf  _:b188 .

_:b189  rdf:type            owl:Restriction ;
        owl:onProperty      rel:hasComponent ;
        owl:someValuesFrom  ata:ata-37-10 .

ata:ata-37  rdfs:subClassOf  _:b189 ;
        rel:hasComponent  ata:ata-37-20 ;
        rel:hasComponent  ata:ata-37-10 ;
        ata:has-id        "37" .

ata:ata-83  rdf:type     owl:Class ;
        rdfs:comment     "Those units and components which are remotely installed and connected to the engine by a drive shaft and which drive multiple type of accessories. Does not include those accessory drives which are bolted to and are immediately adjacent to the engine. The latter item shall be covered under Chapter 72, ENGINE." ;
        rdfs:label       "ACCESSORY GEAR BOXES (ENGINE DRIVEN)" ;
        rdfs:subClassOf  rel:Component .

_:b190  rdf:type            owl:Restriction ;
        owl:onProperty      rel:hasComponent ;
        owl:someValuesFrom  ata:ata-83-10 .

ata:ata-83  rdfs:subClassOf  _:b190 .

_:b191  rdf:type            owl:Restriction ;
        owl:onProperty      rel:hasComponent ;
        owl:someValuesFrom  ata:ata-83-20 .

ata:ata-83  rdfs:subClassOf  _:b191 ;
        rel:hasComponent  ata:ata-83-10 ;
        rel:hasComponent  ata:ata-83-20 ;
        ata:has-id        "83" .

ata:ata-49-90  rdf:type  owl:Class ;
        rdfs:comment     "For definitions see Chapter 79." ;
        rdfs:label       "OIL" ;
        rdfs:subClassOf  rel:Component ;
        ata:has-id       "4990" .

ata:ata-56-10  rdf:type  owl:Class ;
        rdfs:comment     "Compartment above the floor and between the forward passenger partition and the forward pressure dome. Includes items such as the transparent material and its frame of sliding and fixed windows and windshields, handles, latching mechanisms, etc. Does not include door or inspection/observation windows." ;
        rdfs:label       "FLIGHT COMPARTMENT" ;
        rdfs:subClassOf  rel:Component ;
        ata:has-id       "5610" .

ata:ata-23-20  rdf:type  owl:Class ;
        rdfs:comment     "That portion of the system which presents information derived from pulse coded transmissions. Includes Teleprinter, Selcal, Calsel, ACARS, etc." ;
        rdfs:label       "DATA TRANSMISSION AND AUTOMATIC CALLING" ;
        rdfs:subClassOf  rel:Component ;
        ata:has-id       "2320" .

ata:ata-28-40  rdf:type  owl:Class ;
        rdfs:comment     "That portion of the system which is used to indicate the quantity, temperature, and pressure of the fuel. Includes pressure warning systems for pumping systems within the tank, etc. Does not include engine fuel flow or pressure." ;
        rdfs:label       "INDICATING" ;
        rdfs:subClassOf  rel:Component ;
        ata:has-id       "2840" .

ata:ata-51  rdf:type     owl:Class ;
        rdfs:comment     "GENERAL Standard Practices, General Procedures and typical repairs applicable to more than one chapter and are not specifically covered under Chapters 52 thru 57 Sub-Sys / Sect breakdown." ;
        rdfs:label       "STANDARD PRACTICES AND STRUCTURES - GENERAL" ;
        rdfs:subClassOf  rel:Component .

_:b192  rdf:type            owl:Restriction ;
        owl:onProperty      rel:hasComponent ;
        owl:someValuesFrom  ata:ata-51-80 .

ata:ata-51  rdfs:subClassOf  _:b192 .

_:b193  rdf:type            owl:Restriction ;
        owl:onProperty      rel:hasComponent ;
        owl:someValuesFrom  ata:ata-51-50 .

ata:ata-51  rdfs:subClassOf  _:b193 .

_:b194  rdf:type            owl:Restriction ;
        owl:onProperty      rel:hasComponent ;
        owl:someValuesFrom  ata:ata-51-40 .

ata:ata-51  rdfs:subClassOf  _:b194 .

_:b195  rdf:type            owl:Restriction ;
        owl:onProperty      rel:hasComponent ;
        owl:someValuesFrom  ata:ata-51-10 .

ata:ata-51  rdfs:subClassOf  _:b195 .

_:b196  rdf:type            owl:Restriction ;
        owl:onProperty      rel:hasComponent ;
        owl:someValuesFrom  ata:ata-51-60 .

ata:ata-51  rdfs:subClassOf  _:b196 .

_:b197  rdf:type            owl:Restriction ;
        owl:onProperty      rel:hasComponent ;
        owl:someValuesFrom  ata:ata-51-70 .

ata:ata-51  rdfs:subClassOf  _:b197 .

_:b198  rdf:type            owl:Restriction ;
        owl:onProperty      rel:hasComponent ;
        owl:someValuesFrom  ata:ata-51-20 .

ata:ata-51  rdfs:subClassOf  _:b198 .

_:b199  rdf:type            owl:Restriction ;
        owl:onProperty      rel:hasComponent ;
        owl:someValuesFrom  ata:ata-51-30 .

ata:ata-51  rdfs:subClassOf  _:b199 ;
        rel:hasComponent  ata:ata-51-50 ;
        rel:hasComponent  ata:ata-51-60 ;
        rel:hasComponent  ata:ata-51-10 ;
        rel:hasComponent  ata:ata-51-20 ;
        rel:hasComponent  ata:ata-51-70 ;
        rel:hasComponent  ata:ata-51-80 ;
        rel:hasComponent  ata:ata-51-30 ;
        rel:hasComponent  ata:ata-51-40 ;
        ata:has-id        "51" .

ata:ata-41-30  rdf:type  owl:Class ;
        rdfs:comment     "That portion of the system used to indicate quantity, condition and relative distribution of the water ballast." ;
        rdfs:label       "INDICATION" ;
        rdfs:subClassOf  rel:Component ;
        ata:has-id       "4130" .

ata:ata-54-10  rdf:type  owl:Class ;
        rdfs:comment     "Nacelle Section Skins, primary structure, secondary structure, fillets, and fairings of a complete nacelle with any structural differences grouped together and highlighted by specific nacelle designator. The section locations shall be defined by manufacturing joints or other suitable demarcations in a logical sequence." ;
        rdfs:label       "[AS REQUIRED]" ;
        rdfs:subClassOf  rel:Component ;
        ata:has-id       "5410" .

ata:ata-21-20  rdf:type  owl:Class ;
        rdfs:comment     "That portion of the system used to induct and distribute air. Includes equipment rack cooling systems and items such as blowers, scoops, ducting, inlets, check valves, wiring, etc. Does not include valves which are part of pressurization and temperature control." ;
        rdfs:label       "DISTRIBUTION" ;
        rdfs:subClassOf  rel:Component ;
        ata:has-id       "2120" .

ata:ata-39-20  rdf:type  owl:Class ;
        rdfs:label       "ELECTRICAL AND ELECTRONIC EQUIPMENT RACKS" ;
        rdfs:subClassOf  rel:Component ;
        ata:has-id       "3920" .

<http://onto.fel.cvut.cz/voc/ata-100/ata-72(R)-10>
        rdf:type         owl:Class ;
        rdfs:comment     "The section of the engine which contains the propeller shafts and reduction gears. Includes items such as drives for nose mounted accessories." ;
        rdfs:label       "FRONT SECTION" ;
        rdfs:subClassOf  rel:Component ;
        ata:has-id       "72(R)10" .

ata:ata-52-10  rdf:type  owl:Class ;
        rdfs:comment     "Doors used for entrance and exit of the passengers and crew to and from the aircraft. Includes items such as structure, latching mechanisms, handles, insulation, lining, controls, integral steps, ramps, handrails, attach/attached fittings, etc." ;
        rdfs:label       "PASSENGER / CREW" ;
        rdfs:subClassOf  rel:Component ;
        ata:has-id       "5210" .

ata:ata-57-30  rdf:type  owl:Class ;
        rdfs:comment     "Skins and structure of the wing tip and attached fittings." ;
        rdfs:label       "WING TIP" ;
        rdfs:subClassOf  rel:Component ;
        ata:has-id       "5730" .

ata:ata-24-40  rdf:type  owl:Class ;
        rdfs:comment     "That portion of the system within the aircraft which connects external electrical power to the aircraft's electrical system. Includes items such as receptacles, relays, switches, wiring, warning lights, etc." ;
        rdfs:label       "EXTERNAL POWER" ;
        rdfs:subClassOf  rel:Component ;
        ata:has-id       "2440" .

ata:ata-37-20  rdf:type  owl:Class ;
        rdfs:comment     "That portion of the system which is used to indicate pressure. Includes pressure warning system." ;
        rdfs:label       "INDICATING" ;
        rdfs:subClassOf  rel:Component ;
        ata:has-id       "3720" .

ata:ata-64  rdf:type     owl:Class ;
        rdfs:comment     "Assembly that rotates in a plane nearly parallel to the symmetry plane and delivers a thrust opposing to the main rotor torque thus ensuring yaw control. Includes the rotor blades and rotor head. Does not include the rotor anti-icing system which is dealt with in chapter 30: \"Protection against ice and rain\"." ;
        rdfs:label       "TAIL ROTOR" ;
        rdfs:subClassOf  rel:Component .

_:b200  rdf:type            owl:Restriction ;
        owl:onProperty      rel:hasComponent ;
        owl:someValuesFrom  ata:ata-64-40 .

ata:ata-64  rdfs:subClassOf  _:b200 .

_:b201  rdf:type            owl:Restriction ;
        owl:onProperty      rel:hasComponent ;
        owl:someValuesFrom  ata:ata-64-30 .

ata:ata-64  rdfs:subClassOf  _:b201 .

_:b202  rdf:type            owl:Restriction ;
        owl:onProperty      rel:hasComponent ;
        owl:someValuesFrom  ata:ata-64-20 .

ata:ata-64  rdfs:subClassOf  _:b202 .

_:b203  rdf:type            owl:Restriction ;
        owl:onProperty      rel:hasComponent ;
        owl:someValuesFrom  ata:ata-64-10 .

ata:ata-64  rdfs:subClassOf  _:b203 ;
        rel:hasComponent  ata:ata-64-30 ;
        rel:hasComponent  ata:ata-64-20 ;
        rel:hasComponent  ata:ata-64-10 ;
        rel:hasComponent  ata:ata-64-40 ;
        ata:has-id        "64" .

ata:ata-32  rdf:type     owl:Class ;
        rdfs:comment     "Those units and components which furnish a means of supporting and steering the aircraft on the ground or water, and make it possible to retract and store the landing gear in flight. Includes tail skid assembly, brakes, wheels, floats, skids, skis, doors, shock struts, tires, linkages, position indicating and warning systems. Also includes the functioning and maintenance aspects of the landing gear doors but does not include the structure which is covered in Chapter 52 DOORS." ;
        rdfs:label       "LANDING GEAR" ;
        rdfs:subClassOf  rel:Component .

_:b204  rdf:type            owl:Restriction ;
        owl:onProperty      rel:hasComponent ;
        owl:someValuesFrom  ata:ata-32-70 .

ata:ata-32  rdfs:subClassOf  _:b204 .

_:b205  rdf:type            owl:Restriction ;
        owl:onProperty      rel:hasComponent ;
        owl:someValuesFrom  ata:ata-32-60 .

ata:ata-32  rdfs:subClassOf  _:b205 .

_:b206  rdf:type            owl:Restriction ;
        owl:onProperty      rel:hasComponent ;
        owl:someValuesFrom  ata:ata-32-20 .

ata:ata-32  rdfs:subClassOf  _:b206 .

_:b207  rdf:type            owl:Restriction ;
        owl:onProperty      rel:hasComponent ;
        owl:someValuesFrom  ata:ata-32-10 .

ata:ata-32  rdfs:subClassOf  _:b207 .

_:b208  rdf:type            owl:Restriction ;
        owl:onProperty      rel:hasComponent ;
        owl:someValuesFrom  ata:ata-32-50 .

ata:ata-32  rdfs:subClassOf  _:b208 .

_:b209  rdf:type            owl:Restriction ;
        owl:onProperty      rel:hasComponent ;
        owl:someValuesFrom  ata:ata-32-30 .

ata:ata-32  rdfs:subClassOf  _:b209 .

_:b210  rdf:type            owl:Restriction ;
        owl:onProperty      rel:hasComponent ;
        owl:someValuesFrom  ata:ata-32-40 .

ata:ata-32  rdfs:subClassOf  _:b210 ;
        rel:hasComponent  ata:ata-32-40 ;
        rel:hasComponent  ata:ata-32-60 ;
        rel:hasComponent  ata:ata-32-30 ;
        rel:hasComponent  ata:ata-32-10 ;
        rel:hasComponent  ata:ata-32-50 ;
        rel:hasComponent  ata:ata-32-20 ;
        rel:hasComponent  ata:ata-32-70 ;
        ata:has-id        "32" .

ata:ata-55-30  rdf:type  owl:Class ;
        rdfs:comment     "Vertical airfoil to which the rudder is attached. Includes items such as spars, ribs, stringers, skins, access covers, tips, attach/attached fittings, etc." ;
        rdfs:label       "VERTICAL STABILIZER" ;
        rdfs:subClassOf  rel:Component ;
        ata:has-id       "5530" .

ata:ata-22-40  rdf:type  owl:Class ;
        rdfs:comment     "That which provides separate or external monitoring/remote readout (for maintenance or other purposes) not directly related to the internal system monitoring (for system integrity flight crew warning). This includes sensing, computing, indicating and warning devices, control panels, etc." ;
        rdfs:label       "SYSTEM MONITOR" ;
        rdfs:subClassOf  rel:Component ;
        ata:has-id       "2240" .

ata:ata-27-60  rdf:type  owl:Class ;
        rdfs:comment     "That portion of the systems which controls the position and movement of the spoilers, drag devices and variable aerodynamic fairings. Includes fairings. Includes items such as control handles, cables, warning systems, linkages, spoilers, drag devices, position indicators, etc." ;
        rdfs:label       "SPOILER, DRAG DEVICES AND VARIABLE AERODYNAMIC FAIRINGS" ;
        rdfs:subClassOf  rel:Component ;
        ata:has-id       "2760" .

ata:ata-35-20  rdf:type  owl:Class ;
        rdfs:comment     "That portion of the system which furnishes oxygen to the passengers." ;
        rdfs:label       "PASSENGER" ;
        rdfs:subClassOf  rel:Component ;
        ata:has-id       "3520" .

_:b211  rdf:type            owl:Restriction ;
        owl:onProperty      rel:hasComponent ;
        owl:someValuesFrom  ata:group-structures .

ata:ata-53-30  rdf:type  owl:Class ;
        rdfs:label       "PLATES-SKIN" ;
        rdfs:subClassOf  rel:Component ;
        ata:has-id       "5330" .

ata:ata-66-10  rdf:type  owl:Class ;
        rdfs:comment     "Part of the system ensuring rotor blade folding and spreading; includes the mechanical, hydraulic and electrical means permanently fitted on the aircraft." ;
        rdfs:label       "ROTOR BLADES" ;
        rdfs:subClassOf  rel:Component ;
        ata:has-id       "6610" .

ata:ata-25-60  rdf:type  owl:Class ;
        rdfs:comment     "Those items of equipment carried for use in emergency procedures. Includes items such as evacuation equipment, life rafts, jackets, emergency locator transmitters, underwater locator devices, first aid kit, incubators, oxygen tents, medical stretchers, landing and signal flares, drag parachutes, evacuation signaling systems, etc. Does not include fire extinguishers, oxygen equipment or masks." ;
        rdfs:label       "EMERGENCY" ;
        rdfs:subClassOf  rel:Component ;
        ata:has-id       "2560" .

ata:ata-33-20  rdf:type  owl:Class ;
        rdfs:comment     "The lighting sub-systems in the areas in which the passengers are seated and in buffet / galley, lavatories, lounges and coat rooms. Includes items such as direct and indirect illumination, passenger call system, lighted signs, etc." ;
        rdfs:label       "PASSENGER COMPARTMENT" ;
        rdfs:subClassOf  rel:Component ;
        ata:has-id       "3320" .

ata:ata-38-40  rdf:type  owl:Class ;
        rdfs:comment     "That portion of the system common to more than one sub -system which is used for pressurizing supply tanks to insure fluid flow." ;
        rdfs:label       "AIR SUPPLY" ;
        rdfs:subClassOf  rel:Component ;
        ata:has-id       "3840" .

<http://onto.fel.cvut.cz/voc/ata-100/ata-72(T)-80>
        rdf:type         owl:Class ;
        rdfs:comment     "The section of the engine which contains a propulsor(s) and provides the majority of the energy generated. The propulsor may be turbine-driven or gear-driven. Includes such items as propulsor turbines, propulsor blades, blade actuation, and frames (rotating and/or stationary.)" ;
        rdfs:label       "PROPULSOR SECTION (REAR MOUNTED)" ;
        rdfs:subClassOf  rel:Component ;
        ata:has-id       "72(T)80" .

ata:ata-71-40  rdf:type  owl:Class ;
        rdfs:comment     "Those fittings and brackets which are used for the support of equipment in and about the power package." ;
        rdfs:label       "ATTACH FITTINGS" ;
        rdfs:subClassOf  rel:Component ;
        ata:has-id       "7140" .

ata:ata-77  rdf:type     owl:Class ;
        rdfs:comment     "Those units, components and associated systems which indicate engine operation. Includes indicators, transmitters, analyzers, etc. For turbo-prop engines includes phase detectors. Does not include systems or items which are included in other chapters except when indication is accomplished as part of an integrated engine instrument system (ref. 77-40)." ;
        rdfs:label       "ENGINE INDICATING" ;
        rdfs:subClassOf  rel:Component .

_:b212  rdf:type            owl:Restriction ;
        owl:onProperty      rel:hasComponent ;
        owl:someValuesFrom  ata:ata-77-30 .

ata:ata-77  rdfs:subClassOf  _:b212 .

_:b213  rdf:type            owl:Restriction ;
        owl:onProperty      rel:hasComponent ;
        owl:someValuesFrom  ata:ata-77-10 .

ata:ata-77  rdfs:subClassOf  _:b213 .

_:b214  rdf:type            owl:Restriction ;
        owl:onProperty      rel:hasComponent ;
        owl:someValuesFrom  ata:ata-77-40 .

ata:ata-77  rdfs:subClassOf  _:b214 .

_:b215  rdf:type            owl:Restriction ;
        owl:onProperty      rel:hasComponent ;
        owl:someValuesFrom  ata:ata-77-20 .

ata:ata-77  rdfs:subClassOf  _:b215 ;
        rel:hasComponent  ata:ata-77-20 ;
        rel:hasComponent  ata:ata-77-30 ;
        rel:hasComponent  ata:ata-77-10 ;
        rel:hasComponent  ata:ata-77-40 ;
        ata:has-id        "77" .

ata:ata-51-30  rdf:type  owl:Class ;
        rdfs:comment     "Description of materials (metallic and non-metallic) including extrusions, formed sections, sheet, sealants, adhesives, and special materials used in airplane repair. Where possible, permissible substitutes and sources of supply will be given." ;
        rdfs:label       "MATERIALS" ;
        rdfs:subClassOf  rel:Component ;
        ata:has-id       "5130" .

ata:ata-45  rdf:type     owl:Class ;
        rdfs:comment     "Those units, components and associated system which interfaces with multiple aircraft systems. Contains checkout and fault isolation procedures using a central computer complex and/or standard fault isolation procedures to locate a single system or component malfunction." ;
        rdfs:label       "CENTRAL MAINTENANCE SYSTEM (CMS)" ;
        rdfs:subClassOf  rel:Component .

_:b216  rdf:type            owl:Restriction ;
        owl:onProperty      rel:hasComponent ;
        owl:someValuesFrom  ata:ata-45-20 .

ata:ata-45  rdfs:subClassOf  _:b216 .

_:b217  rdf:type            owl:Restriction ;
        owl:onProperty      rel:hasComponent ;
        owl:someValuesFrom  ata:ata-45-45 .

ata:ata-45  rdfs:subClassOf  _:b217 .

_:b218  rdf:type            owl:Restriction ;
        owl:onProperty      rel:hasComponent ;
        owl:someValuesFrom  ata:ata-45-05 .

ata:ata-45  rdfs:subClassOf  _:b218 .

_:b219  rdf:type            owl:Restriction ;
        owl:onProperty      rel:hasComponent ;
        owl:someValuesFrom  ata:ata-45-46 .

ata:ata-45  rdfs:subClassOf  _:b219 .

_:b220  rdf:type            owl:Restriction ;
        owl:onProperty      rel:hasComponent ;
        owl:someValuesFrom  ata:ata-45-70 .

ata:ata-45  rdfs:subClassOf  _:b220 .

_:b221  rdf:type            owl:Restriction ;
        owl:onProperty      rel:hasComponent ;
        owl:someValuesFrom  ata:ata-45-60 .

ata:ata-45  rdfs:subClassOf  _:b221 .

_:b222  rdf:type            owl:Restriction ;
        owl:onProperty      rel:hasComponent ;
        owl:someValuesFrom  ata:ata-45-50 .

ata:ata-45  rdfs:subClassOf  _:b222 ;
        rel:hasComponent  ata:ata-45-70 ;
        rel:hasComponent  ata:ata-45-05 ;
        rel:hasComponent  ata:ata-45-60 ;
        rel:hasComponent  ata:ata-45-50 ;
        rel:hasComponent  ata:ata-45-45 ;
        rel:hasComponent  ata:ata-45-20 ;
        rel:hasComponent  ata:ata-45-46 ;
        ata:has-id        "45" .

ata:ata-64-10  rdf:type  owl:Class ;
        rdfs:comment     "Blade assemblies, including heating mats (electrical resistors) for anti-icing. For an integral rotor blade/rotor head unit, only one section will be used." ;
        rdfs:label       "ROTOR BLADES" ;
        rdfs:subClassOf  rel:Component ;
        ata:has-id       "6410" .

ata:ata-23-60  rdf:type  owl:Class ;
        rdfs:comment     "That portion of the system which is used to dissipate static electricity." ;
        rdfs:label       "STATIC DISCHARGING" ;
        rdfs:subClassOf  rel:Component ;
        ata:has-id       "2360" .

ata:ata-91  rdf:type     owl:Class ;
        rdfs:comment     "Miscellaneous charts not applicable to any particular system, such as spare wire charts, junction box charts, disconnect plug charts, conduit and wire routing charts, rigid tube charts, flexible hose charts and control cables." ;
        rdfs:label       "CHARTS" ;
        rdfs:subClassOf  rel:Component ;
        ata:has-id       "91" .

ata:ata-31-20  rdf:type  owl:Class ;
        rdfs:comment     "Those instruments, units and components which are not related to specific systems. Includes items such as inclinometers, clocks, etc." ;
        rdfs:label       "INDEPENDENT INSTRUMENTS" ;
        rdfs:subClassOf  rel:Component ;
        ata:has-id       "3120" .

ata:ata-49-20  rdf:type  owl:Class ;
        rdfs:comment     "For definitions see Chapter 72." ;
        rdfs:label       "ENGINE" ;
        rdfs:subClassOf  rel:Component ;
        ata:has-id       "4920" .

ata:group-propeller-rotor
        rdf:type         owl:Class ;
        rdfs:comment     "Complete propeller / rotor system excluding propeller / rotor anti-icing system." ;
        rdfs:label       "GROUP DEFINITION PROPELLER / ROTOR" ;
        rdfs:subClassOf  rel:Component .

_:b223  rdf:type            owl:Restriction ;
        owl:onProperty      rel:hasComponent ;
        owl:someValuesFrom  ata:ata-63 .

ata:group-propeller-rotor
        rdfs:subClassOf  _:b223 .

_:b224  rdf:type            owl:Restriction ;
        owl:onProperty      rel:hasComponent ;
        owl:someValuesFrom  ata:ata-64 .

ata:group-propeller-rotor
        rdfs:subClassOf  _:b224 .

_:b225  rdf:type            owl:Restriction ;
        owl:onProperty      rel:hasComponent ;
        owl:someValuesFrom  ata:ata-67 .

ata:group-propeller-rotor
        rdfs:subClassOf  _:b225 .

_:b226  rdf:type            owl:Restriction ;
        owl:onProperty      rel:hasComponent ;
        owl:someValuesFrom  ata:ata-60 .

ata:group-propeller-rotor
        rdfs:subClassOf  _:b226 .

_:b227  rdf:type            owl:Restriction ;
        owl:onProperty      rel:hasComponent ;
        owl:someValuesFrom  ata:ata-65 .

ata:group-propeller-rotor
        rdfs:subClassOf  _:b227 .

_:b228  rdf:type            owl:Restriction ;
        owl:onProperty      rel:hasComponent ;
        owl:someValuesFrom  ata:ata-62 .

ata:group-propeller-rotor
        rdfs:subClassOf  _:b228 .

_:b229  rdf:type            owl:Restriction ;
        owl:onProperty      rel:hasComponent ;
        owl:someValuesFrom  ata:ata-66 .

ata:group-propeller-rotor
        rdfs:subClassOf  _:b229 .

_:b230  rdf:type            owl:Restriction ;
        owl:onProperty      rel:hasComponent ;
        owl:someValuesFrom  ata:ata-61 .

ata:group-propeller-rotor
        rdfs:subClassOf   _:b230 ;
        rel:hasComponent  ata:ata-60 ;
        rel:hasComponent  ata:ata-66 ;
        rel:hasComponent  ata:ata-65 ;
        rel:hasComponent  ata:ata-64 ;
        rel:hasComponent  ata:ata-63 ;
        rel:hasComponent  ata:ata-62 ;
        rel:hasComponent  ata:ata-61 ;
        rel:hasComponent  ata:ata-67 ;
        ata:has-id        "group-propeller-rotor" .

ata:ata-82-20  rdf:type  owl:Class ;
        rdfs:comment     "That portion of the system which is used to conduct water or water mixtures from the tanks or cells to the engine. Includes items such as plumbing, crossfeed systems, pumps, valves, controls, etc." ;
        rdfs:label       "DISTRUBUTION" ;
        rdfs:subClassOf  rel:Component ;
        ata:has-id       "8220" .

ata:ata-54-50  rdf:type  owl:Class ;
        rdfs:comment     "Pylon Section Skins, primary structure, secondary structure, fillets, and fairings of a complete pylon with any structural differences grouped together and highlighted by specific pylon designator. The section locations shall be defined by manufacturing joints or other suitable demarcations in a logical sequence." ;
        rdfs:label       "[AS REQUIRED]" ;
        rdfs:subClassOf  rel:Component ;
        ata:has-id       "5450" .

ata:ata-62-10  rdf:type  owl:Class ;
        rdfs:comment     "Rotor blade assemblies, including the heating mate (electrical resistors) for anti -icing." ;
        rdfs:label       "ROTOR BLADES" ;
        rdfs:subClassOf  rel:Component ;
        ata:has-id       "6210" .

ata:ata-67-30  rdf:type  owl:Class ;
        rdfs:comment     "That portion of the system which from a power source ensures distribution to the rotor servo-control." ;
        rdfs:label       "SERVO-CONTROL SYSTEM" ;
        rdfs:subClassOf  rel:Component ;
        ata:has-id       "6730" .

ata:ata-21-60  rdf:type  owl:Class ;
        rdfs:comment     "That portion of the system used to control the temperature of the air. Includes items such as control valves, thermal sensing devices, switches, indicators, amplifiers, wiring, etc." ;
        rdfs:label       "TEMPERATURE CONTROL" ;
        rdfs:subClassOf  rel:Component ;
        ata:has-id       "2160" .

ata:ata-34-40  rdf:type  owl:Class ;
        rdfs:comment     "That portion of the system which provides information to determine position and is mainly independent of ground installations or orbital satellites. Includes items such as inertial guidance systems, weather radar, Doppler, proximity warning, collision avoidance, star tracker, etc. Also includes sextants/octants, etc." ;
        rdfs:label       "INDEPENDENT POSITION DETERMINING" ;
        rdfs:subClassOf  rel:Component ;
        ata:has-id       "3440" .

ata:ata-39-60  rdf:type  owl:Class ;
        rdfs:label       "PRINTED CIRCUIT CARD ASSEMBLIES" ;
        rdfs:subClassOf  rel:Component ;
        ata:has-id       "3960" .

<http://onto.fel.cvut.cz/voc/ata-100/ata-72(R)-50>
        rdf:type         owl:Class ;
        rdfs:comment     "Those units and components which are used to distribute oil throughout the engine. Includes front and rear pressure and scavenger pumps, sumps, strainers, valves, etc. Also includes those oil lines not included in chapter 79. Does not include those items which form integral passages within the engine." ;
        rdfs:label       "LUBRICATION" ;
        rdfs:subClassOf  rel:Component ;
        ata:has-id       "72(R)50" .

ata:ata-52-50  rdf:type  owl:Class ;
        rdfs:comment     "Interior Doors inside the fuselage installed in fixed partitions. Includes items such as structure, latching mechanisms, handles, lining, attach/attached fittings, etc. Does not include doors installed in movable partitions which are covered in Chapter 25." ;
        rdfs:label       "FIXED INTERIOR" ;
        rdfs:subClassOf  rel:Component ;
        ata:has-id       "5250" .

ata:ata-57-70  rdf:type  owl:Class ;
        rdfs:comment     "Skins and structure of wing-mounted spoilers, airbrakes, lift dumpers, attach/attached fittings, etc." ;
        rdfs:label       "SPOILERS" ;
        rdfs:subClassOf  rel:Component ;
        ata:has-id       "5770" .

ata:ata-65-30  rdf:type  owl:Class ;
        rdfs:label       "[AVAILABLE]" ;
        rdfs:subClassOf  rel:Component ;
        ata:has-id       "6530" .

ata:ata-32-40  rdf:type  owl:Class ;
        rdfs:comment     "That portion of the system which provides for rolling and stopping the aircraft while on the ground and stopping wheel rotation after retraction. Includes items such as bearings, tires, valves, de -boosters, swivel glands, anti-skid devices, pressure indicators, plumbing, etc." ;
        rdfs:label       "WHEELS AND BRAKES" ;
        rdfs:subClassOf  rel:Component ;
        ata:has-id       "3240" .

ata:ata-78-10  rdf:type  owl:Class ;
        rdfs:comment     "That portion of the system which collects the exhaust gases from the cylinders or turbines and conducts them overboard. Includes items such as collector rings, exhaust and thrust augmentor ducts, variable nozzles, actuators, plumbing, linkages, wiring, position indicators, warning systems, etc. Does not include power recovery turbines, turbo-superchargers, etc., nor noise suppressors or thrust reversers where they are not an integral part of the nozzle system." ;
        rdfs:label       "COLLECTOR - NOZZLE" ;
        rdfs:subClassOf  rel:Component ;
        ata:has-id       "7810" .

ata:ata-45-20  rdf:type  owl:Class ;
        rdfs:comment     "Central Maintenance System interfaces with Airframe Systems, and identification of maintenance functions related to Airframe Systems." ;
        rdfs:label       "CMS / AIRFRAME SYSTEMS" ;
        rdfs:subClassOf  rel:Component ;
        ata:has-id       "4520" .

ata:ata-26  rdf:type     owl:Class ;
        rdfs:comment     "Those fixed and portable units and components which detect and indicate fire or smoke and store and distribute fire extinguishing agent to all protected areas of the aircraft; including bottles, valves, tubing, etc." ;
        rdfs:label       "FIRE PROTECTION" ;
        rdfs:subClassOf  rel:Component .

_:b231  rdf:type            owl:Restriction ;
        owl:onProperty      rel:hasComponent ;
        owl:someValuesFrom  ata:ata-26-10 .

ata:ata-26  rdfs:subClassOf  _:b231 .

_:b232  rdf:type            owl:Restriction ;
        owl:onProperty      rel:hasComponent ;
        owl:someValuesFrom  ata:ata-26-20 .

ata:ata-26  rdfs:subClassOf  _:b232 .

_:b233  rdf:type            owl:Restriction ;
        owl:onProperty      rel:hasComponent ;
        owl:someValuesFrom  ata:ata-26-30 .

ata:ata-26  rdfs:subClassOf  _:b233 ;
        rel:hasComponent  ata:ata-26-20 ;
        rel:hasComponent  ata:ata-26-10 ;
        rel:hasComponent  ata:ata-26-30 ;
        ata:has-id        "26" .

ata:ata-72  rdf:type     owl:Class ;
        rdfs:comment     "Those units and components which are: used to induce and convert fuel-air mixture into power. Includes, for the turbine engine, air inlet, compessor, diffuser, combustion chambers, turbine and exhaust; and for the reciprocating engine, blower and clutch, clutch control valve, cylinder, cylinder baffles, intake pipes, crankshaft assembly, etc.\n\nUsed to transmit power to the propeller shaft, if any, and accessory drives. Includes reduction gearing, gear trains, extension shaft and torque meter.\n\nWithin the profile of the basic engine, used to supplement the functioning of other defined systems external to the engine. Includes items such as accessory drive, mechanical portion of the spark advance mechanism, oil transfer tubes from the propeller governor pad to the propeller shaft, BMEP section, etc.\n\nUsed to control and direct the flow of lubrication through the engine from the inlet fitting to the outlet fitting. Includes engine pumps (pressure and scavenger), pressure relief valves, screens, oil lines (internal and external), etc.\n" ;
        rdfs:label       "ENGINE" ;
        rdfs:subClassOf  rel:Component ;
        ata:has-id       "72" .

ata:ata-63-30  rdf:type  owl:Class ;
        rdfs:comment     "Suspension bars, vibration damping system providing attachment of the G.B.(s) to the airframe." ;
        rdfs:label       "MOUNTS, ATTACHMENTS" ;
        rdfs:subClassOf  rel:Component ;
        ata:has-id       "6330" .

ata:ata-76-10  rdf:type  owl:Class ;
        rdfs:comment     "That portion of the system which furnishes a means of controlling the main fuel control or coordinator. Includes controls to the propeller regulator on turbo-prop engines. Includes items such as linkages, cables, levers, pulleys, switches, wiring, etc. does not include the units themselves." ;
        rdfs:label       "POWER CONTROL" ;
        rdfs:subClassOf  rel:Component ;
        ata:has-id       "7610" .

ata:ata-30-40  rdf:type  owl:Class ;
        rdfs:comment     "That portion of the system which is used to eliminate or prevent the formation of ice, frost or rain on the windows, windshields and doors." ;
        rdfs:label       "WINDOWS, WINDSHIELDS, AND DOORS" ;
        rdfs:subClassOf  rel:Component ;
        ata:has-id       "3040" .

ata:group-structures  rdf:type  owl:Class ;
        rdfs:label       "STRUCTURES" ;
        rdfs:subClassOf  rel:Component .

_:b234  rdf:type            owl:Restriction ;
        owl:onProperty      rel:hasComponent ;
        owl:someValuesFrom  ata:ata-55 .

ata:group-structures  rdfs:subClassOf  _:b234 .

_:b235  rdf:type            owl:Restriction ;
        owl:onProperty      rel:hasComponent ;
        owl:someValuesFrom  ata:ata-51 .

ata:group-structures  rdfs:subClassOf  _:b235 .

_:b236  rdf:type            owl:Restriction ;
        owl:onProperty      rel:hasComponent ;
        owl:someValuesFrom  ata:ata-52 .

ata:group-structures  rdfs:subClassOf  _:b236 .

_:b237  rdf:type            owl:Restriction ;
        owl:onProperty      rel:hasComponent ;
        owl:someValuesFrom  ata:ata-54 .

ata:group-structures  rdfs:subClassOf  _:b237 .

_:b238  rdf:type            owl:Restriction ;
        owl:onProperty      rel:hasComponent ;
        owl:someValuesFrom  ata:ata-56 .

ata:group-structures  rdfs:subClassOf  _:b238 .

_:b239  rdf:type            owl:Restriction ;
        owl:onProperty      rel:hasComponent ;
        owl:someValuesFrom  ata:ata-57 .

ata:group-structures  rdfs:subClassOf  _:b239 .

_:b240  rdf:type            owl:Restriction ;
        owl:onProperty      rel:hasComponent ;
        owl:someValuesFrom  ata:ata-53 .

ata:group-structures  rdfs:subClassOf  _:b240 ;
        rel:hasComponent  ata:ata-53 ;
        rel:hasComponent  ata:ata-52 ;
        rel:hasComponent  ata:ata-51 ;
        rel:hasComponent  ata:ata-57 ;
        rel:hasComponent  ata:ata-55 ;
        rel:hasComponent  ata:ata-56 ;
        rel:hasComponent  ata:ata-54 ;
        ata:has-id        "group-structures" .

ata:ata-53-70  rdf:type  owl:Class ;
        rdfs:label       "[AS REQUIRED]" ;
        rdfs:subClassOf  rel:Component ;
        ata:has-id       "5370" .

ata:ata-61-30  rdf:type  owl:Class ;
        rdfs:comment     "That portion of the system which is used to decrease run -down time or stop propeller rotation during engine power -off conditions. Includes brake mechanisms, levers, pulleys, cables, switches, wiring, plumbing, etc." ;
        rdfs:label       "BRAKING" ;
        rdfs:subClassOf  rel:Component ;
        ata:has-id       "6130" .

ata:ata-74-10  rdf:type  owl:Class ;
        rdfs:comment     "That portion of the system which generates electrical current for the purpose of igniting the fuel mixture in the combustion chambers and thrust augmentors. Includes items such as magnetos, distributors, booster coils, exciters, transformers, storage capacitors, and compositors, etc." ;
        rdfs:label       "ELECTRICAL POWER SUPPLY" ;
        rdfs:subClassOf  rel:Component ;
        ata:has-id       "7410" .

ata:ata-79-30  rdf:type  owl:Class ;
        rdfs:comment     "That portion of the system which is used to indicate oil quantity, temperature, and pressure of the oil. Includes items such as transmitters, indicators, wiring, warning systems, etc. Does not include indication if indication is accomplished as part of an integrated engine instrument system (ref. 77-40)." ;
        rdfs:label       "INDICATING" ;
        rdfs:subClassOf  rel:Component ;
        ata:has-id       "7930" .

ata:ata-46-40  rdf:type  owl:Class ;
        rdfs:comment     "That portion of the onboard information system that supports the passenger cabin, cabin operations, and flight attendants." ;
        rdfs:label       "PASSENGER CABIN INFORMATION SYSTEMS" ;
        rdfs:subClassOf  rel:Component ;
        ata:has-id       "4640" .

ata:ata-39  rdf:type     owl:Class ;
        rdfs:label       "ELECTRICAL - ELECTRONIC PANELS AND MULTIPURPOSE COMPONENTS" ;
        rdfs:subClassOf  rel:Component .

_:b241  rdf:type            owl:Restriction ;
        owl:onProperty      rel:hasComponent ;
        owl:someValuesFrom  ata:ata-39-10 .

ata:ata-39  rdfs:subClassOf  _:b241 .

_:b242  rdf:type            owl:Restriction ;
        owl:onProperty      rel:hasComponent ;
        owl:someValuesFrom  ata:ata-39-30 .

ata:ata-39  rdfs:subClassOf  _:b242 .

_:b243  rdf:type            owl:Restriction ;
        owl:onProperty      rel:hasComponent ;
        owl:someValuesFrom  ata:ata-39-60 .

ata:ata-39  rdfs:subClassOf  _:b243 .

_:b244  rdf:type            owl:Restriction ;
        owl:onProperty      rel:hasComponent ;
        owl:someValuesFrom  ata:ata-39-50 .

ata:ata-39  rdfs:subClassOf  _:b244 .

_:b245  rdf:type            owl:Restriction ;
        owl:onProperty      rel:hasComponent ;
        owl:someValuesFrom  ata:ata-39-20 .

ata:ata-39  rdfs:subClassOf  _:b245 .

_:b246  rdf:type            owl:Restriction ;
        owl:onProperty      rel:hasComponent ;
        owl:someValuesFrom  ata:ata-39-40 .

ata:ata-39  rdfs:subClassOf  _:b246 ;
        rel:hasComponent  ata:ata-39-60 ;
        rel:hasComponent  ata:ata-39-10 ;
        rel:hasComponent  ata:ata-39-50 ;
        rel:hasComponent  ata:ata-39-40 ;
        rel:hasComponent  ata:ata-39-30 ;
        rel:hasComponent  ata:ata-39-20 ;
        ata:has-id        "39" .

ata:ata-51-70  rdf:type  owl:Class ;
        rdfs:comment     "Typical repairs suitable for general use, not limited to one ATA Chapter." ;
        rdfs:label       "REPAIRS" ;
        rdfs:subClassOf  rel:Component ;
        ata:has-id       "5170" .

<http://onto.fel.cvut.cz/voc/ata-100/ata-72(T)-10>
        rdf:type         owl:Class ;
        rdfs:comment     "The section of the engine which contains the propeller shafts and reduction gears. Includes items such as drives for hose mounted accessories, etc. If applicable, the section of the engine which uses mechanical force, through a gear-driven system, to drive front mounted propulsors which provide the majority of the energy generated. Includes items such as Propulsor Blades, Actuation systems, Reduction Gears, Drive-Shafts, etc." ;
        rdfs:label       "REDUCTION GEAR AND SHAFT SECTION (TURBOPROP AND/OR FRONT MOUNTED DRIVEN PROPULSOR)" ;
        rdfs:subClassOf  rel:Component ;
        ata:has-id       "72(T)10" .

ata:ata-77-30  rdf:type  owl:Class ;
        rdfs:comment     "That portion of the system which is used to analyze engine performance or condition by means of instruments or devices such as oscilloscopes, etc. Includes items such as generators, wiring, amplifiers, oscilloscopes, etc." ;
        rdfs:label       "ANALYZERS" ;
        rdfs:subClassOf  rel:Component ;
        ata:has-id       "7730" .

ata:ata-31-60  rdf:type  owl:Class ;
        rdfs:comment     "Those systems and components which give visual display of conditions in unrelated systems." ;
        rdfs:label       "CENTRAL DISPLAY SYSTEMS" ;
        rdfs:subClassOf  rel:Component ;
        ata:has-id       "3160" .

ata:ata-53  rdf:type     owl:Class ;
        rdfs:comment     "Structural units and associated components and members which make up the compartments for equipment, passengers, crew, cargo, plus the structure of the envelope and gondola of airships. Includes skins, belt frames, stringers, floor beams, floor, pressure dome, scuppers, tail cone, fuselage -to-wing and -empennage fillets, attach/attached fittings, load curtains, cables, ballonets, etc." ;
        rdfs:label       "FUSELAGE" ;
        rdfs:subClassOf  rel:Component .

_:b247  rdf:type            owl:Restriction ;
        owl:onProperty      rel:hasComponent ;
        owl:someValuesFrom  ata:ata-53-30 .

ata:ata-53  rdfs:subClassOf  _:b247 .

_:b248  rdf:type            owl:Restriction ;
        owl:onProperty      rel:hasComponent ;
        owl:someValuesFrom  ata:ata-53-50 .

ata:ata-53  rdfs:subClassOf  _:b248 .

_:b249  rdf:type            owl:Restriction ;
        owl:onProperty      rel:hasComponent ;
        owl:someValuesFrom  ata:ata-53-10 .

ata:ata-53  rdfs:subClassOf  _:b249 .

_:b250  rdf:type            owl:Restriction ;
        owl:onProperty      rel:hasComponent ;
        owl:someValuesFrom  ata:ata-53-90 .

ata:ata-53  rdfs:subClassOf  _:b250 .

_:b251  rdf:type            owl:Restriction ;
        owl:onProperty      rel:hasComponent ;
        owl:someValuesFrom  ata:ata-53-80 .

ata:ata-53  rdfs:subClassOf  _:b251 .

_:b252  rdf:type            owl:Restriction ;
        owl:onProperty      rel:hasComponent ;
        owl:someValuesFrom  ata:ata-53-20 .

ata:ata-53  rdfs:subClassOf  _:b252 .

_:b253  rdf:type            owl:Restriction ;
        owl:onProperty      rel:hasComponent ;
        owl:someValuesFrom  ata:ata-53-40 .

ata:ata-53  rdfs:subClassOf  _:b253 .

_:b254  rdf:type            owl:Restriction ;
        owl:onProperty      rel:hasComponent ;
        owl:someValuesFrom  ata:ata-53-60 .

ata:ata-53  rdfs:subClassOf  _:b254 .

_:b255  rdf:type            owl:Restriction ;
        owl:onProperty      rel:hasComponent ;
        owl:someValuesFrom  ata:ata-53-70 .

ata:ata-53  rdfs:subClassOf  _:b255 ;
        rel:hasComponent  ata:ata-53-80 ;
        rel:hasComponent  ata:ata-53-30 ;
        rel:hasComponent  ata:ata-53-20 ;
        rel:hasComponent  ata:ata-53-60 ;
        rel:hasComponent  ata:ata-53-10 ;
        rel:hasComponent  ata:ata-53-40 ;
        rel:hasComponent  ata:ata-53-50 ;
        rel:hasComponent  ata:ata-53-70 ;
        rel:hasComponent  ata:ata-53-90 ;
        ata:has-id        "53" .

ata:ata-49-60  rdf:type  owl:Class ;
        rdfs:comment     "For definitions see Chapter 76." ;
        rdfs:label       "ENGINE CONTROLS" ;
        rdfs:subClassOf  rel:Component ;
        ata:has-id       "4960" .

ata:ata-28-10  rdf:type  owl:Class ;
        rdfs:comment     "That portion of the system which stores fuel. Includes tank sealing, bladder type cells, ventilating system, cell and tank inter -connectors, over wing filler necks and caps, etc. Also includes reservoir feed pumping systems and reservoirs within the tanks which are not part of the distribution system." ;
        rdfs:label       "STORAGE" ;
        rdfs:subClassOf  rel:Component ;
        ata:has-id       "2810" .

ata:ata-21  rdf:type     owl:Class ;
        rdfs:comment     "Those units and components which furnish a means of pressurizing, heating, cooling, moisture controlling, filtering and treating the air used to ventilate the areas of the fuselage within the pressure seals. Includes cabin supercharger, equipment cooling, heater, heater fuel system, expansion turbine, valves, scoops, ducts, etc." ;
        rdfs:label       "AIR CONDITIONING" ;
        rdfs:subClassOf  rel:Component .

_:b256  rdf:type            owl:Restriction ;
        owl:onProperty      rel:hasComponent ;
        owl:someValuesFrom  ata:ata-21-60 .

ata:ata-21  rdfs:subClassOf  _:b256 .

_:b257  rdf:type            owl:Restriction ;
        owl:onProperty      rel:hasComponent ;
        owl:someValuesFrom  ata:ata-21-40 .

ata:ata-21  rdfs:subClassOf  _:b257 .

_:b258  rdf:type            owl:Restriction ;
        owl:onProperty      rel:hasComponent ;
        owl:someValuesFrom  ata:ata-21-20 .

ata:ata-21  rdfs:subClassOf  _:b258 .

_:b259  rdf:type            owl:Restriction ;
        owl:onProperty      rel:hasComponent ;
        owl:someValuesFrom  ata:ata-21-30 .

ata:ata-21  rdfs:subClassOf  _:b259 .

_:b260  rdf:type            owl:Restriction ;
        owl:onProperty      rel:hasComponent ;
        owl:someValuesFrom  ata:ata-21-70 .

ata:ata-21  rdfs:subClassOf  _:b260 .

_:b261  rdf:type            owl:Restriction ;
        owl:onProperty      rel:hasComponent ;
        owl:someValuesFrom  ata:ata-21-10 .

ata:ata-21  rdfs:subClassOf  _:b261 .

_:b262  rdf:type            owl:Restriction ;
        owl:onProperty      rel:hasComponent ;
        owl:someValuesFrom  ata:ata-21-50 .

ata:ata-21  rdfs:subClassOf  _:b262 ;
        rel:hasComponent  ata:ata-21-30 ;
        rel:hasComponent  ata:ata-21-50 ;
        rel:hasComponent  ata:ata-21-20 ;
        rel:hasComponent  ata:ata-21-70 ;
        rel:hasComponent  ata:ata-21-40 ;
        rel:hasComponent  ata:ata-21-60 ;
        rel:hasComponent  ata:ata-21-10 ;
        ata:has-id        "21" .

ata:ata-54-90  rdf:type  owl:Class ;
        rdfs:label       "[AS REQUIRED]" ;
        rdfs:subClassOf  rel:Component ;
        ata:has-id       "5490" .

ata:ata-75-30  rdf:type  owl:Class ;
        rdfs:comment     "That portion of the system which is used to control the flow of air through the engine. Includes items such as governors, valves, actuators, linkages, etc. Also includes the operation of variable stator blades, but not the maintenance and overhaul, which shall be covered under 72-30." ;
        rdfs:label       "COMPRESSOR CONTROL" ;
        rdfs:subClassOf  rel:Component ;
        ata:has-id       "7530" .

ata:ata-26-10  rdf:type  owl:Class ;
        rdfs:comment     "That portion of the system which is used to sense and indicate the presence of overheat, smoke, or fire." ;
        rdfs:label       "DETECTION" ;
        rdfs:subClassOf  rel:Component ;
        ata:has-id       "2610" .

_:b263  rdf:type            owl:Restriction ;
        owl:onProperty      rel:hasComponent ;
        owl:someValuesFrom  ata:group-propeller-rotor .

ata:ata-45-46  rdf:type  owl:Class ;
        rdfs:comment     "Central Maintenance System interfaces with Airframe Systems, and identification of maintenance functions related to Airframe Systems." ;
        rdfs:label       "CMS / AIRFRAME SYSTEMS" ;
        rdfs:subClassOf  rel:Component ;
        ata:has-id       "4546" .

ata:ata-73-30  rdf:type  owl:Class ;
        rdfs:comment     "That portion of the system which is used to indicate the flow rate, temperature, and pressure of the fuel. Includes items such as transmitters, indicators, wiring, etc. Does not include indication, if indication is accomplished as part of an integrated engine instrument system (ref. 77-40)." ;
        rdfs:label       "INDICATING" ;
        rdfs:subClassOf  rel:Component ;
        ata:has-id       "7330" .

ata:ata-45-60  rdf:type  owl:Class ;
        rdfs:comment     "Central Maintenance System interfaces with Propeller, and identification of maintenance functions related to Propellers." ;
        rdfs:label       "CMS / PROPELLERS" ;
        rdfs:subClassOf  rel:Component ;
        ata:has-id       "4560" .

ata:ata-24-10  rdf:type  owl:Class ;
        rdfs:comment     "Mechanical devices that drive the generators at a desired RPM. Includes items such as oil system, connecting devices, indicating and warning systems for the drive, etc." ;
        rdfs:label       "GENERATOR DRIVE" ;
        rdfs:subClassOf  rel:Component ;
        ata:has-id       "2410" .

ata:ata-29-30  rdf:type  owl:Class ;
        rdfs:comment     "That portion of the system which is used to indicate the quantity, temperature and pressure of the hydraulic fluid. Includes items such as transmitters, indicators, wiring, warning systems, etc." ;
        rdfs:label       "INDICATING" ;
        rdfs:subClassOf  rel:Component ;
        ata:has-id       "2930" .

ata:ata-66  rdf:type     owl:Class ;
        rdfs:comment     "The whole of the system ensuring automatic or manual folding and spreading of the rotor blades and/or tail pylon. NOTE: such rigging also affects the components described in other chapters." ;
        rdfs:label       "ROTOR BLADE AND TAIL PYLON FOLDING" ;
        rdfs:subClassOf  rel:Component .

_:b264  rdf:type            owl:Restriction ;
        owl:onProperty      rel:hasComponent ;
        owl:someValuesFrom  ata:ata-66-20 .

ata:ata-66  rdfs:subClassOf  _:b264 .

_:b265  rdf:type            owl:Restriction ;
        owl:onProperty      rel:hasComponent ;
        owl:someValuesFrom  ata:ata-66-30 .

ata:ata-66  rdfs:subClassOf  _:b265 .

_:b266  rdf:type            owl:Restriction ;
        owl:onProperty      rel:hasComponent ;
        owl:someValuesFrom  ata:ata-66-10 .

ata:ata-66  rdfs:subClassOf  _:b266 ;
        rel:hasComponent  ata:ata-66-20 ;
        rel:hasComponent  ata:ata-66-30 ;
        rel:hasComponent  ata:ata-66-10 ;
        ata:has-id        "66" .

ata:ata-34  rdf:type     owl:Class ;
        rdfs:comment     "Those units and components which provide aircraft navigational information. Includes VOR, pitot, static, ILS, flight director, compasses, indicators, etc." ;
        rdfs:label       "NAVIGATION" ;
        rdfs:subClassOf  rel:Component .

_:b267  rdf:type            owl:Restriction ;
        owl:onProperty      rel:hasComponent ;
        owl:someValuesFrom  ata:ata-34-60 .

ata:ata-34  rdfs:subClassOf  _:b267 .

_:b268  rdf:type            owl:Restriction ;
        owl:onProperty      rel:hasComponent ;
        owl:someValuesFrom  ata:ata-34-40 .

ata:ata-34  rdfs:subClassOf  _:b268 .

_:b269  rdf:type            owl:Restriction ;
        owl:onProperty      rel:hasComponent ;
        owl:someValuesFrom  ata:ata-34-50 .

ata:ata-34  rdfs:subClassOf  _:b269 .

_:b270  rdf:type            owl:Restriction ;
        owl:onProperty      rel:hasComponent ;
        owl:someValuesFrom  ata:ata-34-30 .

ata:ata-34  rdfs:subClassOf  _:b270 .

_:b271  rdf:type            owl:Restriction ;
        owl:onProperty      rel:hasComponent ;
        owl:someValuesFrom  ata:ata-34-10 .

ata:ata-34  rdfs:subClassOf  _:b271 .

_:b272  rdf:type            owl:Restriction ;
        owl:onProperty      rel:hasComponent ;
        owl:someValuesFrom  ata:ata-34-20 .

ata:ata-34  rdfs:subClassOf  _:b272 ;
        rel:hasComponent  ata:ata-34-40 ;
        rel:hasComponent  ata:ata-34-20 ;
        rel:hasComponent  ata:ata-34-50 ;
        rel:hasComponent  ata:ata-34-30 ;
        rel:hasComponent  ata:ata-34-60 ;
        rel:hasComponent  ata:ata-34-10 ;
        ata:has-id        "34" .

ata:ata-80  rdf:type     owl:Class ;
        rdfs:comment     "Those units, components and associated systems used for starting the engine. Includes electrical, inertial air or other starter systems. Does not include ignition systems which are covered in chapter 74, IGNITION." ;
        rdfs:label       "STARTING" ;
        rdfs:subClassOf  rel:Component .

_:b273  rdf:type            owl:Restriction ;
        owl:onProperty      rel:hasComponent ;
        owl:someValuesFrom  ata:ata-80-10 .

ata:ata-80  rdfs:subClassOf  _:b273 ;
        rel:hasComponent  ata:ata-80-10 ;
        ata:has-id        "80" .

_:b274  rdf:type            owl:Restriction ;
        owl:onProperty      rel:hasComponent ;
        owl:someValuesFrom  ata:group-airframe-systems .

ata:ata-30-80  rdf:type  owl:Class ;
        rdfs:comment     "That portion of the system which is used to detect and indicate the formation of ice." ;
        rdfs:label       "DETECTION" ;
        rdfs:subClassOf  rel:Component ;
        ata:has-id       "3080" .

ata:ata-22-10  rdf:type  owl:Class ;
        rdfs:comment     "That portion of the system that uses radio/radar signals, directional and vertical references, air data (pitot static), computed flight path data, or manually induced inputs to the system to automatically control the flight path of the aircraft through adjustment to the pitch/roll/yaw axis or wing lift characteristics and provide visual cues for flight path guidance, i.e.: Integrated Flight Director. This includes power source devices, interlocking devices and amplifying, computing, integrating, controlling, actuating, indicating and warning devices such as computers, servos, control panels, indicators, warning lights, etc." ;
        rdfs:label       "AUTOPILOT" ;
        rdfs:subClassOf  rel:Component ;
        ata:has-id       "2210" .

ata:ata-27-30  rdf:type  owl:Class ;
        rdfs:comment     "That portion of the systems which controls the position and movement of the elevator / elevon and tabs. Includes items such as the control column, stickshaker units, automatic stall recovery devices, tab control wheels, cables, boosters, linkages, control surfaces, position indicators, stall warning systems, etc." ;
        rdfs:label       "ELEVATOR AND TAB" ;
        rdfs:subClassOf  rel:Component ;
        ata:has-id       "2730" .

ata:ata-25-30  rdf:type  owl:Class ;
        rdfs:comment     "The areas in which food and beverages are stored and prepared. Includes items such as removable and fixed cabinets, ovens, refrigerators, garbage containers, dish racks, coffee maker and dispensers, containers, electrical outlets, wiring, etc." ;
        rdfs:label       "BUFFET / GALLEY" ;
        rdfs:subClassOf  rel:Component ;
        ata:has-id       "2530" .

ata:ata-38-10  rdf:type  owl:Class ;
        rdfs:comment     "That portion of the system which is used to store and deliver fresh drinking water. Includes wash water system if the potable water is also used for washing." ;
        rdfs:label       "POTABLE" ;
        rdfs:subClassOf  rel:Component ;
        ata:has-id       "3810" .

ata:ata-79  rdf:type     owl:Class ;
        rdfs:comment     "Those units and components external to the engine concerned with storing and delivering lubricating oil to and from the engine. Covers all units and components from the lubricating oil engine outlet to the inlet, including the inlet and outlet fittings, tank, radiator, by-pass valve, etc., and auxiliary oil systems." ;
        rdfs:label       "OIL" ;
        rdfs:subClassOf  rel:Component .

_:b275  rdf:type            owl:Restriction ;
        owl:onProperty      rel:hasComponent ;
        owl:someValuesFrom  ata:ata-79-30 .

ata:ata-79  rdfs:subClassOf  _:b275 .

_:b276  rdf:type            owl:Restriction ;
        owl:onProperty      rel:hasComponent ;
        owl:someValuesFrom  ata:ata-79-20 .

ata:ata-79  rdfs:subClassOf  _:b276 .

_:b277  rdf:type            owl:Restriction ;
        owl:onProperty      rel:hasComponent ;
        owl:someValuesFrom  ata:ata-79-10 .

ata:ata-79  rdfs:subClassOf  _:b277 ;
        rel:hasComponent  ata:ata-79-20 ;
        rel:hasComponent  ata:ata-79-10 ;
        rel:hasComponent  ata:ata-79-30 ;
        ata:has-id        "79" .

<http://onto.fel.cvut.cz/voc/ata-100/ata-72(T)-50>
        rdf:type         owl:Class ;
        rdfs:comment     "The section of the engine containing the turbines. Includes items such as turbine nozzles, turbine rotors, cases, etc." ;
        rdfs:label       "TURBINE SECTION" ;
        rdfs:subClassOf  rel:Component ;
        ata:has-id       "72(T)50" .

ata:ata-71-10  rdf:type  owl:Class ;
        rdfs:comment     "Those removable coverings which extend over and around the power plant assembly. Includes the functioning and maintenance aspects of items such as accessory section cowls, cowl flaps, cowling supports, and attach and locking mechanisms, etc. Does not include the structure integral with the airframe which shall be covered in the applicable Structures chapter." ;
        rdfs:label       "COWLING" ;
        rdfs:subClassOf  rel:Component ;
        ata:has-id       "7110" .

_:b278  rdf:type            owl:Restriction ;
        owl:onProperty      rel:hasComponent ;
        owl:someValuesFrom  ata:group-aircraft .

ata:ata-56-20  rdf:type  owl:Class ;
        rdfs:comment     "Area in which the passengers are seated. Includes lounges, lavatories, buffets / galleys and coatrooms. Includes items such as transparent material, its frame, frost shield, etc." ;
        rdfs:label       "PASSENGER COMPARTMENT" ;
        rdfs:subClassOf  rel:Component ;
        ata:has-id       "5620" .

ata:ata-23-30  rdf:type  owl:Class ;
        rdfs:comment     "That portion of the system used to address and entertain the passengers including installations for increased cabin comfort, such as active noise control systems. Includes items such as amplifiers, speakers, handsets, reproducers, control panels, control -units, etc. Also includes items of audio, video, and film equipment." ;
        rdfs:label       "PASSENGER ADDRESS, ENTERTAINMENT, AND COMFORT" ;
        rdfs:subClassOf  rel:Component ;
        ata:has-id       "2330" .

ata:ata-61  rdf:type     owl:Class ;
        rdfs:comment     "The complete mechanical or electrical propeller, pumps, motors, governor, alternators, and those units and components external to or integral with the engine used to control the propeller blade angle. Includes propeller spinner synchronizers. Also includes propulsor duct assemblies, including aerodynamic fairing of mechanical components, stators, vectoring systems, etc." ;
        rdfs:label       "PROPELLERS / PROPULSORS" ;
        rdfs:subClassOf  rel:Component .

_:b279  rdf:type            owl:Restriction ;
        owl:onProperty      rel:hasComponent ;
        owl:someValuesFrom  ata:ata-61-10 .

ata:ata-61  rdfs:subClassOf  _:b279 .

_:b280  rdf:type            owl:Restriction ;
        owl:onProperty      rel:hasComponent ;
        owl:someValuesFrom  ata:ata-61-20 .

ata:ata-61  rdfs:subClassOf  _:b280 .

_:b281  rdf:type            owl:Restriction ;
        owl:onProperty      rel:hasComponent ;
        owl:someValuesFrom  ata:ata-61-30 .

ata:ata-61  rdfs:subClassOf  _:b281 .

_:b282  rdf:type            owl:Restriction ;
        owl:onProperty      rel:hasComponent ;
        owl:someValuesFrom  ata:ata-61-50 .

ata:ata-61  rdfs:subClassOf  _:b282 .

_:b283  rdf:type            owl:Restriction ;
        owl:onProperty      rel:hasComponent ;
        owl:someValuesFrom  ata:ata-61-40 .

ata:ata-61  rdfs:subClassOf  _:b283 ;
        rel:hasComponent  ata:ata-61-20 ;
        rel:hasComponent  ata:ata-61-50 ;
        rel:hasComponent  ata:ata-61-10 ;
        rel:hasComponent  ata:ata-61-30 ;
        rel:hasComponent  ata:ata-61-40 ;
        ata:has-id        "61" .

ata:ata-36-10  rdf:type  owl:Class ;
        rdfs:comment     "That portion of the system which is used to distribute high or low pressure air to using systems. Includes items such as ducts, valves, actuators, heat exchangers, controls, etc. Does not include the supply valves to the using systems." ;
        rdfs:label       "DISTRIBUTION" ;
        rdfs:subClassOf  rel:Component ;
        ata:has-id       "3610" .

ata:ata-54-20  rdf:type  owl:Class ;
        rdfs:label       "[AS REQUIRED]" ;
        rdfs:subClassOf  rel:Component ;
        ata:has-id       "5420" .

ata:ata-21-30  rdf:type  owl:Class ;
        rdfs:comment     "That portion of the system used to control the pressure within the fuselage. Includes items such as control valves, relief valves, indicators, switches, amplifiers, wiring, etc." ;
        rdfs:label       "PRESSURIZATION CONTROL" ;
        rdfs:subClassOf  rel:Component ;
        ata:has-id       "2130" .

ata:ata-34-10  rdf:type  owl:Class ;
        rdfs:comment     "That portion of the system which senses environmental conditions and uses the data to influence navigation. Includes such items as Central Air Data Computers, pitot/static systems, air temperature, rate -of-climb, airspeed, high speed warning, altitude, altitude reporting, altimeter correction system, air disturbance detection system, etc." ;
        rdfs:label       "FLIGHT ENVIRONMENT DATA" ;
        rdfs:subClassOf  rel:Component ;
        ata:has-id       "3410" .

ata:ata-39-30  rdf:type  owl:Class ;
        rdfs:label       "ELECTRICAL AND ELECTRONIC JUNCTION BOXES" ;
        rdfs:subClassOf  rel:Component ;
        ata:has-id       "3930" .

<http://onto.fel.cvut.cz/voc/ata-100/ata-72(R)-20>
        rdf:type         owl:Class ;
        rdfs:comment     "The section of the engine which contains the crankshaft, master and link rod assemblies, cams, cam drives gears, tappet guides, roller, carriers, etc." ;
        rdfs:label       "POWER SECTION" ;
        rdfs:subClassOf  rel:Component ;
        ata:has-id       "72(R)20" .

ata:ata-52-20  rdf:type  owl:Class ;
        rdfs:comment     "Exit doors used to facilitate evacuation that are not normally used for exit. Includes items such as structure, latching mechanisms, handles, insulation, lining, controls, attach / attached fittings, etc." ;
        rdfs:label       "EMERGENCY EXIT" ;
        rdfs:subClassOf  rel:Component ;
        ata:has-id       "5220" .

ata:ata-57-40  rdf:type  owl:Class ;
        rdfs:comment     "Skins and structure of the wing leading edge and removable leading edge airfoils such as flaps, slats, attach/attached fittings, etc." ;
        rdfs:label       "LEADING EDGE AND LEADING EDGE DEVICES" ;
        rdfs:subClassOf  rel:Component ;
        ata:has-id       "5740" .

ata:ata-24-50  rdf:type  owl:Class ;
        rdfs:comment     "That portion of the system which provides for connection of AC power to using systems. Includes items such as AC main and secondary busses, main system circuit breakers, power system devices, etc." ;
        rdfs:label       "AC ELECTRICAL LOAD DISTRIBUTION" ;
        rdfs:subClassOf  rel:Component ;
        ata:has-id       "2450" .

ata:ata-32-10  rdf:type  owl:Class ;
        rdfs:comment     "That portion of the system which provides the major support for the aircraft while on the ground. Includes items such as shock struts, bogie axles, drag struts, linkages, attach bolts, etc." ;
        rdfs:label       "MAIN GEAR AND DOORS" ;
        rdfs:subClassOf  rel:Component ;
        ata:has-id       "3210" .

ata:ata-28  rdf:type     owl:Class ;
        rdfs:comment     "Those units and components which store and deliver fuel to the engine. Includes engine driven fuel pumps for reciprocating engines, includes tanks (bladder), valves, boost pumps, etc., and those components which furnish a means of dumping fuel overboard. Includes integral and tip fuel tank leak detection and sealing. Does not include the structure of integral or tip fuel tanks and the fuel cell backing boards which are covered in the Structures Chapters, and does not include fuel flow rate sensing, transmitting and / or indicating, which are covered in Chapter 73." ;
        rdfs:label       "FUEL" ;
        rdfs:subClassOf  rel:Component .

_:b284  rdf:type            owl:Restriction ;
        owl:onProperty      rel:hasComponent ;
        owl:someValuesFrom  ata:ata-28-20 .

ata:ata-28  rdfs:subClassOf  _:b284 .

_:b285  rdf:type            owl:Restriction ;
        owl:onProperty      rel:hasComponent ;
        owl:someValuesFrom  ata:ata-28-30 .

ata:ata-28  rdfs:subClassOf  _:b285 .

_:b286  rdf:type            owl:Restriction ;
        owl:onProperty      rel:hasComponent ;
        owl:someValuesFrom  ata:ata-28-40 .

ata:ata-28  rdfs:subClassOf  _:b286 .

_:b287  rdf:type            owl:Restriction ;
        owl:onProperty      rel:hasComponent ;
        owl:someValuesFrom  ata:ata-28-10 .

ata:ata-28  rdfs:subClassOf  _:b287 ;
        rel:hasComponent  ata:ata-28-30 ;
        rel:hasComponent  ata:ata-28-10 ;
        rel:hasComponent  ata:ata-28-40 ;
        rel:hasComponent  ata:ata-28-20 ;
        ata:has-id        "28" .

ata:ata-74  rdf:type     owl:Class ;
        rdfs:comment     "Those units and components which generate, control, furnish, or distribute an electrical current to ignite the fuel air mixture in the cylinders of reciprocating engines or in the combustion chambers or thrust augmentor of turbine engines. Includes induction vibrators, magnetos, switches, lead filters, distributors, harnesses, plugs, ignition relays, exciters, and the electrical portion of spark advance." ;
        rdfs:label       "IGNITION" ;
        rdfs:subClassOf  rel:Component .

_:b288  rdf:type            owl:Restriction ;
        owl:onProperty      rel:hasComponent ;
        owl:someValuesFrom  ata:ata-74-30 .

ata:ata-74  rdfs:subClassOf  _:b288 .

_:b289  rdf:type            owl:Restriction ;
        owl:onProperty      rel:hasComponent ;
        owl:someValuesFrom  ata:ata-74-10 .

ata:ata-74  rdfs:subClassOf  _:b289 .

_:b290  rdf:type            owl:Restriction ;
        owl:onProperty      rel:hasComponent ;
        owl:someValuesFrom  ata:ata-74-20 .

ata:ata-74  rdfs:subClassOf  _:b290 ;
        rel:hasComponent  ata:ata-74-20 ;
        rel:hasComponent  ata:ata-74-10 ;
        rel:hasComponent  ata:ata-74-30 ;
        ata:has-id        "74" .

ata:ata-83-10  rdf:type  owl:Class ;
        rdfs:comment     "That portion of the system which is used to conduct power from the engine to the gearbox. Includes items such as drive shaft, adapters, seals, etc." ;
        rdfs:label       "DRIVE SHAFT SECTION" ;
        rdfs:subClassOf  rel:Component ;
        ata:has-id       "8310" .

ata:ata-55-40  rdf:type  owl:Class ;
        rdfs:comment     "Removable airfoil which is attached to the vertical stabilizer and used for yaw control. Includes items such as spars, ribs, stringers, skins, access covers, tabs, balance devices, attach/attached fittings, etc." ;
        rdfs:label       "RUDDER - RUDDEVATOR" ;
        rdfs:subClassOf  rel:Component ;
        ata:has-id       "5540" .

ata:ata-22-50  rdf:type  owl:Class ;
        rdfs:comment     "The system or portion of the system that automatically corrects/provides for gust loading / upset, aerodynamic augmentation/alleviation/suppression, ride control, etc. This includes sensing, computing, actuating, indicating internal monitoring, warning devices, etc." ;
        rdfs:label       "AERODYNAMIC LOAD ALLEVIATING" ;
        rdfs:subClassOf  rel:Component ;
        ata:has-id       "2250" .

ata:ata-35-30  rdf:type  owl:Class ;
        rdfs:comment     "That portion of the system which has an independent oxygen supply and which can be transported about the airplane." ;
        rdfs:label       "PORTABLE" ;
        rdfs:subClassOf  rel:Component ;
        ata:has-id       "3530" .

ata:ata-27-70  rdf:type  owl:Class ;
        rdfs:comment     "That portion of the systems which protects the control surfaces from movement by wind while the aircraft is on the ground. Does not include locking the control by means of flight control boost system." ;
        rdfs:label       "GUST LOCK AND DAMPER" ;
        rdfs:subClassOf  rel:Component ;
        ata:has-id       "2770" .

ata:ata-30-10  rdf:type  owl:Class ;
        rdfs:comment     "That portion of the system which is used to eliminate or prevent the formation of ice on all airfoil surfaces. Includes wings, airfoil sections of the empennage, and pylons." ;
        rdfs:label       "AIRFOIL" ;
        rdfs:subClassOf  rel:Component ;
        ata:has-id       "3010" .

_:b291  rdf:type            owl:Restriction ;
        owl:onProperty      rel:hasComponent ;
        owl:someValuesFrom  ata:group-power-plant .

ata:ata-81-10  rdf:type  owl:Class ;
        rdfs:comment     "The turbines which extract energy from the exhaust gases and are coupled to the crankshaft." ;
        rdfs:label       "POWER RECOVERY" ;
        rdfs:subClassOf  rel:Component ;
        ata:has-id       "8110" .

ata:ata-53-40  rdf:type  owl:Class ;
        rdfs:label       "ATTACH FITTINGS" ;
        rdfs:subClassOf  rel:Component ;
        ata:has-id       "5340" .

ata:ata-66-20  rdf:type  owl:Class ;
        rdfs:comment     "Part of system ensuring tail pylon folding and spreading; includes mechanical, hydraulic and electrical means permanently fitted on the aircraft." ;
        rdfs:label       "TAIL PYLON" ;
        rdfs:subClassOf  rel:Component ;
        ata:has-id       "6620" .

ata:ata-25-70  rdf:type  owl:Class ;
        rdfs:comment     "Those compartments used for the housing of various components or accessories. Includes wheel wells, tail-hydraulic-electrical/ electronic equipment racks, main battery structure, etc." ;
        rdfs:label       "ACCESSORY COMPARTMENTS" ;
        rdfs:subClassOf  rel:Component ;
        ata:has-id       "2570" .

ata:ata-33-30  rdf:type  owl:Class ;
        rdfs:comment     "The lighting sub-systems in the compartments for stowage of cargo and the housing of various components of accessories." ;
        rdfs:label       "CARGO AND SERVICE COMPARTMENTS" ;
        rdfs:subClassOf  rel:Component ;
        ata:has-id       "3330" .

ata:ata-46-10  rdf:type  owl:Class ;
        rdfs:label       "AIRPLANE GENERAL INFORMATION SYSTEMS" ;
        rdfs:subClassOf  rel:Component ;
        ata:has-id       "4610" .

ata:ata-71-50  rdf:type  owl:Class ;
        rdfs:comment     "Those electrical cables, conduits, plugs, sockets, etc., which serve several power plant systems, but which are banded together to facilitate removal and installation of the power plant. Does not include the wiring which is specifically covered under another system." ;
        rdfs:label       "ELECTRICAL HARNESS" ;
        rdfs:subClassOf  rel:Component ;
        ata:has-id       "7150" .

ata:ata-51-40  rdf:type  owl:Class ;
        rdfs:comment     "Description of fastener types, materials, and sizes. Procedures for fastener installation and removal including hole preparation. Fastener strength values and substitution data." ;
        rdfs:label       "FASTENERS" ;
        rdfs:subClassOf  rel:Component ;
        ata:has-id       "5140" .

ata:ata-55  rdf:type     owl:Class ;
        rdfs:comment     "Horizontal and vertical stabilizers include the structure of the elevator and rudder." ;
        rdfs:label       "STABILIZERS" ;
        rdfs:subClassOf  rel:Component .

_:b292  rdf:type            owl:Restriction ;
        owl:onProperty      rel:hasComponent ;
        owl:someValuesFrom  ata:ata-55-30 .

ata:ata-55  rdfs:subClassOf  _:b292 .

_:b293  rdf:type            owl:Restriction ;
        owl:onProperty      rel:hasComponent ;
        owl:someValuesFrom  ata:ata-55-10 .

ata:ata-55  rdfs:subClassOf  _:b293 .

_:b294  rdf:type            owl:Restriction ;
        owl:onProperty      rel:hasComponent ;
        owl:someValuesFrom  ata:ata-55-40 .

ata:ata-55  rdfs:subClassOf  _:b294 .

_:b295  rdf:type            owl:Restriction ;
        owl:onProperty      rel:hasComponent ;
        owl:someValuesFrom  ata:ata-55-20 .

ata:ata-55  rdfs:subClassOf  _:b295 ;
        rel:hasComponent  ata:ata-55-40 ;
        rel:hasComponent  ata:ata-55-10 ;
        rel:hasComponent  ata:ata-55-20 ;
        rel:hasComponent  ata:ata-55-30 ;
        ata:has-id        "55" .

ata:ata-64-20  rdf:type  owl:Class ;
        rdfs:comment     "Tail rotor head. For an integral rotor blade/rotor head unit, only one section will be used." ;
        rdfs:label       "ROTOR HEAD" ;
        rdfs:subClassOf  rel:Component ;
        ata:has-id       "6420" .

ata:ata-23-70  rdf:type  owl:Class ;
        rdfs:comment     "Those installations that record, or monitor crew or passenger conversation or movement for security or safety purposes. Includes voice recorders, television, monitors, externally mounted camera, etc." ;
        rdfs:label       "AUDIO & VIDEO MONITORING" ;
        rdfs:subClassOf  rel:Component ;
        ata:has-id       "2370" .

ata:ata-31-30  rdf:type  owl:Class ;
        rdfs:comment     "Those systems and components used for recording data not related to specific systems. Includes items such as flight recorders, performance or maintenance recorders, VG recorders, etc." ;
        rdfs:label       "RECORDERS" ;
        rdfs:subClassOf  rel:Component ;
        ata:has-id       "3130" .

ata:ata-23  rdf:type     owl:Class ;
        rdfs:comment     "Those units and components which furnish a means of communicating from one part of the aircraft to another and between the aircraft or ground stations, includes voice, data, C -W communicating components, PA system, inter -com and tape reproducers - record player." ;
        rdfs:label       "COMMUNICATIONS" ;
        rdfs:subClassOf  rel:Component .

_:b296  rdf:type            owl:Restriction ;
        owl:onProperty      rel:hasComponent ;
        owl:someValuesFrom  ata:ata-23-10 .

ata:ata-23  rdfs:subClassOf  _:b296 .

_:b297  rdf:type            owl:Restriction ;
        owl:onProperty      rel:hasComponent ;
        owl:someValuesFrom  ata:ata-23-80 .

ata:ata-23  rdfs:subClassOf  _:b297 .

_:b298  rdf:type            owl:Restriction ;
        owl:onProperty      rel:hasComponent ;
        owl:someValuesFrom  ata:ata-23-30 .

ata:ata-23  rdfs:subClassOf  _:b298 .

_:b299  rdf:type            owl:Restriction ;
        owl:onProperty      rel:hasComponent ;
        owl:someValuesFrom  ata:ata-23-70 .

ata:ata-23  rdfs:subClassOf  _:b299 .

_:b300  rdf:type            owl:Restriction ;
        owl:onProperty      rel:hasComponent ;
        owl:someValuesFrom  ata:ata-23-15 .

ata:ata-23  rdfs:subClassOf  _:b300 .

_:b301  rdf:type            owl:Restriction ;
        owl:onProperty      rel:hasComponent ;
        owl:someValuesFrom  ata:ata-23-20 .

ata:ata-23  rdfs:subClassOf  _:b301 .

_:b302  rdf:type            owl:Restriction ;
        owl:onProperty      rel:hasComponent ;
        owl:someValuesFrom  ata:ata-23-60 .

ata:ata-23  rdfs:subClassOf  _:b302 .

_:b303  rdf:type            owl:Restriction ;
        owl:onProperty      rel:hasComponent ;
        owl:someValuesFrom  ata:ata-23-40 .

ata:ata-23  rdfs:subClassOf  _:b303 .

_:b304  rdf:type            owl:Restriction ;
        owl:onProperty      rel:hasComponent ;
        owl:someValuesFrom  ata:ata-23-50 .

ata:ata-23  rdfs:subClassOf  _:b304 ;
        rel:hasComponent  ata:ata-23-70 ;
        rel:hasComponent  ata:ata-23-15 ;
        rel:hasComponent  ata:ata-23-20 ;
        rel:hasComponent  ata:ata-23-50 ;
        rel:hasComponent  ata:ata-23-30 ;
        rel:hasComponent  ata:ata-23-80 ;
        rel:hasComponent  ata:ata-23-60 ;
        rel:hasComponent  ata:ata-23-10 ;
        rel:hasComponent  ata:ata-23-40 ;
        ata:has-id        "23" .

ata:ata-49-30  rdf:type  owl:Class ;
        rdfs:comment     "For definitions see Chapter 73." ;
        rdfs:label       "ENGINE FUEL AND CONTROL" ;
        rdfs:subClassOf  rel:Component ;
        ata:has-id       "4930" .

ata:ata-82-30  rdf:type  owl:Class ;
        rdfs:comment     "That portion of the system which is used to dump injection water and to purge the system. Includes items such as plumbing, valves, controls, etc." ;
        rdfs:label       "DUMPING AND PURGING" ;
        rdfs:subClassOf  rel:Component ;
        ata:has-id       "8230" .

ata:ata-54-60  rdf:type  owl:Class ;
        rdfs:label       "[AS REQUIRED]" ;
        rdfs:subClassOf  rel:Component ;
        ata:has-id       "5460" .

ata:ata-62-20  rdf:type  owl:Class ;
        rdfs:comment     "Complete rotor head(s), including blade folding system(s). Includes sleeves, spindles, dampers, rotor head fairing(s) as well as rotor shaft(s) and swashplate(s) if the rotor head and shaft constitute a non-dissociable assembly." ;
        rdfs:label       "ROTOR HEAD(S)" ;
        rdfs:subClassOf  rel:Component ;
        ata:has-id       "6220" .

ata:ata-21-70  rdf:type  owl:Class ;
        rdfs:comment     "That portion of the system used to control moisture in the air, to control ozone concentrations, to filter radioactive debris from conditioned air, and to treat the air with deodorizers, insecticides, etc." ;
        rdfs:label       "MOISTURE / AIR CONTAMINANT CONTROL" ;
        rdfs:subClassOf  rel:Component ;
        ata:has-id       "2170" .

ata:ata-34-50  rdf:type  owl:Class ;
        rdfs:comment     "That portion of the system which provides information to determine position and is mainly dependent on ground installations or orbital satellites. Includes items such as DME, transponders, radio compass, LORAN, VOR, ADF, OMEGA, GLOBAL POSITIONING, etc." ;
        rdfs:label       "DEPENDENT POSITION DETERMINING" ;
        rdfs:subClassOf  rel:Component ;
        ata:has-id       "3450" .

ata:ata-52-60  rdf:type  owl:Class ;
        rdfs:comment     "Stairs which operate in conjunction with but are not an integral part of entrance doors. Stairs whose primary structure is a door shall be covered under the appropriate topic. Includes items such as structure, actuating mechanisms and controls, handrails, attach/attached fittings, etc." ;
        rdfs:label       "ENTRANCE STAIRS" ;
        rdfs:subClassOf  rel:Component ;
        ata:has-id       "5260" .

ata:ata-57-80  rdf:type  owl:Class ;
        rdfs:label       "[AS REQUIRED]" ;
        rdfs:subClassOf  rel:Component ;
        ata:has-id       "5780" .

ata:ata-65-40  rdf:type  owl:Class ;
        rdfs:comment     "That portion of the system which indicates operation or activation of rotor systems. Includes items such as lights, gauges, switches, wiring, etc." ;
        rdfs:label       "INDICATING" ;
        rdfs:subClassOf  rel:Component ;
        ata:has-id       "6540" .

ata:ata-78-20  rdf:type  owl:Class ;
        rdfs:comment     "That portion of the system which reduces the noise generated by the exhaust gases. Includes items such as pipes, baffles, shields, actuators, plumbing linkages, wiring, position indicators, warning systems, etc. Use -10 where integral part of nozzle system." ;
        rdfs:label       "NOISE SUPPRESSOR" ;
        rdfs:subClassOf  rel:Component ;
        ata:has-id       "7820" .

ata:ata-32-50  rdf:type  owl:Class ;
        rdfs:comment     "That portion of the system which is used to control the direction of movement of the aircraft on the ground. Includes items such as actuating cylinders, controls, bogie swivel unlock, etc." ;
        rdfs:label       "STEERING" ;
        rdfs:subClassOf  rel:Component ;
        ata:has-id       "3250" .

<http://onto.fel.cvut.cz/voc/ata-100/ata-72(T)>
        rdf:type         owl:Class ;
        rdfs:label       "ENGINE - TURBINE / TURBOPROP, DUCTED FAN / UNDUCTED FAN" ;
        rdfs:subClassOf  rel:Component .

_:b305  rdf:type            owl:Restriction ;
        owl:onProperty      rel:hasComponent ;
        owl:someValuesFrom  <http://onto.fel.cvut.cz/voc/ata-100/ata-72(T)-80> .

<http://onto.fel.cvut.cz/voc/ata-100/ata-72(T)>
        rdfs:subClassOf  _:b305 .

_:b306  rdf:type            owl:Restriction ;
        owl:onProperty      rel:hasComponent ;
        owl:someValuesFrom  <http://onto.fel.cvut.cz/voc/ata-100/ata-72(T)-70> .

<http://onto.fel.cvut.cz/voc/ata-100/ata-72(T)>
        rdfs:subClassOf  _:b306 .

_:b307  rdf:type            owl:Restriction ;
        owl:onProperty      rel:hasComponent ;
        owl:someValuesFrom  <http://onto.fel.cvut.cz/voc/ata-100/ata-72(T)-30> .

<http://onto.fel.cvut.cz/voc/ata-100/ata-72(T)>
        rdfs:subClassOf  _:b307 .

_:b308  rdf:type            owl:Restriction ;
        owl:onProperty      rel:hasComponent ;
        owl:someValuesFrom  <http://onto.fel.cvut.cz/voc/ata-100/ata-72(T)-50> .

<http://onto.fel.cvut.cz/voc/ata-100/ata-72(T)>
        rdfs:subClassOf  _:b308 .

_:b309  rdf:type            owl:Restriction ;
        owl:onProperty      rel:hasComponent ;
        owl:someValuesFrom  <http://onto.fel.cvut.cz/voc/ata-100/ata-72(T)-40> .

<http://onto.fel.cvut.cz/voc/ata-100/ata-72(T)>
        rdfs:subClassOf  _:b309 .

_:b310  rdf:type            owl:Restriction ;
        owl:onProperty      rel:hasComponent ;
        owl:someValuesFrom  <http://onto.fel.cvut.cz/voc/ata-100/ata-72(T)-10> .

<http://onto.fel.cvut.cz/voc/ata-100/ata-72(T)>
        rdfs:subClassOf  _:b310 .

_:b311  rdf:type            owl:Restriction ;
        owl:onProperty      rel:hasComponent ;
        owl:someValuesFrom  <http://onto.fel.cvut.cz/voc/ata-100/ata-72(T)-60> .

<http://onto.fel.cvut.cz/voc/ata-100/ata-72(T)>
        rdfs:subClassOf  _:b311 .

_:b312  rdf:type            owl:Restriction ;
        owl:onProperty      rel:hasComponent ;
        owl:someValuesFrom  <http://onto.fel.cvut.cz/voc/ata-100/ata-72(T)-20> .

<http://onto.fel.cvut.cz/voc/ata-100/ata-72(T)>
        rdfs:subClassOf   _:b312 ;
        rel:hasComponent  <http://onto.fel.cvut.cz/voc/ata-100/ata-72(T)-30> ;
        rel:hasComponent  <http://onto.fel.cvut.cz/voc/ata-100/ata-72(T)-40> ;
        rel:hasComponent  <http://onto.fel.cvut.cz/voc/ata-100/ata-72(T)-50> ;
        rel:hasComponent  <http://onto.fel.cvut.cz/voc/ata-100/ata-72(T)-60> ;
        rel:hasComponent  <http://onto.fel.cvut.cz/voc/ata-100/ata-72(T)-80> ;
        rel:hasComponent  <http://onto.fel.cvut.cz/voc/ata-100/ata-72(T)-10> ;
        rel:hasComponent  <http://onto.fel.cvut.cz/voc/ata-100/ata-72(T)-70> ;
        rel:hasComponent  <http://onto.fel.cvut.cz/voc/ata-100/ata-72(T)-20> ;
        ata:has-id        "72(T)" .

ata:ata-36  rdf:type     owl:Class ;
        rdfs:comment     "Those units and components (Ducts and Valves) which deliver large volumes of compressed air from a power source to connecting points for such other systems as air conditioning, pressurization, deicing, etc." ;
        rdfs:label       "PNEUMATIC" ;
        rdfs:subClassOf  rel:Component .

_:b313  rdf:type            owl:Restriction ;
        owl:onProperty      rel:hasComponent ;
        owl:someValuesFrom  ata:ata-36-20 .

ata:ata-36  rdfs:subClassOf  _:b313 .

_:b314  rdf:type            owl:Restriction ;
        owl:onProperty      rel:hasComponent ;
        owl:someValuesFrom  ata:ata-36-10 .

ata:ata-36  rdfs:subClassOf  _:b314 ;
        rel:hasComponent  ata:ata-36-20 ;
        rel:hasComponent  ata:ata-36-10 ;
        ata:has-id        "36" .

ata:ata-82  rdf:type     owl:Class ;
        rdfs:comment     "Those units and components which furnish, meter, and inject water or water mixtures into the induction system; includes tanks, pumps, regulators, etc." ;
        rdfs:label       "WATER INJECTION" ;
        rdfs:subClassOf  rel:Component .

_:b315  rdf:type            owl:Restriction ;
        owl:onProperty      rel:hasComponent ;
        owl:someValuesFrom  ata:ata-82-20 .

ata:ata-82  rdfs:subClassOf  _:b315 .

_:b316  rdf:type            owl:Restriction ;
        owl:onProperty      rel:hasComponent ;
        owl:someValuesFrom  ata:ata-82-10 .

ata:ata-82  rdfs:subClassOf  _:b316 .

_:b317  rdf:type            owl:Restriction ;
        owl:onProperty      rel:hasComponent ;
        owl:someValuesFrom  ata:ata-82-40 .

ata:ata-82  rdfs:subClassOf  _:b317 .

_:b318  rdf:type            owl:Restriction ;
        owl:onProperty      rel:hasComponent ;
        owl:someValuesFrom  ata:ata-82-30 .

ata:ata-82  rdfs:subClassOf  _:b318 ;
        rel:hasComponent  ata:ata-82-20 ;
        rel:hasComponent  ata:ata-82-40 ;
        rel:hasComponent  ata:ata-82-10 ;
        rel:hasComponent  ata:ata-82-30 ;
        ata:has-id        "82" .

ata:ata-63-40  rdf:type  owl:Class ;
        rdfs:comment     "That portion of the system which indicates operation or activation of rotor systems. Includes items such as lights, gauges, switches, wiring, etc." ;
        rdfs:label       "INDICATING" ;
        rdfs:subClassOf  rel:Component ;
        ata:has-id       "6340" .

ata:ata-30-50  rdf:type  owl:Class ;
        rdfs:comment     "That portion of the system which is used to eliminate or prevent the formation of ice on antennas and radomes." ;
        rdfs:label       "ANTENNAS AND RADOMES" ;
        rdfs:subClassOf  rel:Component ;
        ata:has-id       "3050" .

ata:ata-76-20  rdf:type  owl:Class ;
        rdfs:comment     "That portion of the system which furnishes a means of controlling the flow of fluids to and from the engine during emergency procedures. Includes items such as levers, cables, pulleys, linkages, switches, wiring, etc. Does not include the units themselves." ;
        rdfs:label       "EMERGENCY SHUTDOWN" ;
        rdfs:subClassOf  rel:Component ;
        ata:has-id       "7620" .
